Checking stuff in to allow others to work.  Still much to fix.

x86model/RockSalt/DFACorrectness.v
@@ -28,9 +28,9 @@ Require ExtrOcamlNatBigInt.
 Require ExtrOcamlNatInt.
 Import X86_PARSER_ARG.
 Import X86_PARSER.
-Import X86_BASE_PARSER.
+(* Import X86_BASE_PARSER. *)
 Import X86Syntax.
-Hint Constructors in_parser.
+Hint Constructors in_grammar.
 
 Ltac t := repeat
   match goal with 
@@ -41,58 +41,49 @@ Ltac t := repeat
       generalize (inj_pairT2 _ _ _ _ _ H) ; clear H ; intros ; subst
   end.
 
-(** Inversion lemmas for parsers -- needed because of the dependencies
-    (i.e., inversion will fail as a tactic on most of these because it
-    can't solve a unification problem.)  These really belong in the 
-    Parser library. *)
-Lemma inv_any_pi : forall cs v, in_parser Any_p cs v -> cs = v::nil.
-  intros. inversion H. t. subst.  auto.
-Qed.
-
-Lemma inv_char_pi : forall c cs v, in_parser (Char_p c) cs v -> v = c /\ cs = c::nil.
-  intros. inversion H. t. subst. auto.
-Qed.
-
-Lemma inv_eps_pi : forall cs v, in_parser Eps_p cs v -> cs = nil /\ v = tt.
-  intros. inversion H. t. subst. auto.
-Qed.
-
-Lemma inv_zero_pi : forall t cs v, in_parser (Zero_p t) cs v -> False.
-  intros. inversion H.
-Qed.
-
-Lemma inv_alt_pi : forall t (p1 p2:parser t) cs v, in_parser (Alt_p p1 p2) cs v -> 
-  in_parser p1 cs v \/ in_parser p2 cs v.
-  intros. inversion H ; t ; auto.
-Qed.
-
-Lemma inv_cat_pi : forall t1 t2 (p1:parser t1) (p2:parser t2) cs v, 
-  in_parser (Cat_p p1 p2) cs v -> 
-  exists cs1, exists cs2, exists v1 : result_m t1, exists v2 : result_m t2,
-    cs = cs1 ++ cs2 /\ v = (v1,v2) /\ in_parser p1 cs1 v1 /\ in_parser p2 cs2 v2.
+Lemma inv_alt : forall t (p1 p2:grammar t) cs v, in_grammar (alt p1 p2) cs v -> 
+  in_grammar p1 cs v \/ in_grammar p2 cs v.                                                
 Proof.
-  intros. inversion H ; t. exists cs1. exists cs2. exists v1. exists v2. auto.
+  unfold alt. intros. generalize (MapInv H). intro. destruct H0 as [v' [H0 H1]].
+  generalize (AltInv H0). intros. destruct H2. destruct H2 as [v1 [H2 H3]]. 
+  left. rewrite H1. rewrite H3. auto. destruct H2 as [v1 [H2 H3]]. right.
+  rewrite H1. rewrite H3. auto.
 Qed.
 
-Lemma inv_map_pi : forall t1 t2 (p:parser t1) (f:result_m t1 -> result_m t2) cs v,
-  in_parser (Map_p _ f p) cs v -> exists v1 : result_m t1, 
-    v = f v1 /\ in_parser p cs v1.
+Lemma inv_never : forall t cs v, in_grammar (never t) cs v -> False.
 Proof.
-  intros. inversion H. t. exists v1. auto.
+  unfold never. intros. apply (ZeroInv H).
 Qed.
 
+Lemma in_alt_r : forall t (p1 p2:grammar t) cs v, in_grammar p2 cs v -> 
+                        in_grammar (alt p1 p2) cs v.
+Proof.
+  intros. econstructor ; eauto.
+Qed.
+Hint Resolve in_alt_r.
+
+Lemma in_alt_l : forall t (p1 p2:grammar t) cs v, in_grammar p1 cs v -> 
+                                                  in_grammar (alt p1 p2) cs v.
+Proof.
+  intros ; econstructor ; eauto.
+Qed.
+Hint Resolve in_alt_l.
+   
 (** A tactic to apply the inversion principles for the parser denotational semantis. *)
 Ltac pinv := 
   match goal with
-    | [ H : in_parser Any_p _ _ |- _ ] => generalize (inv_any_pi H) ; clear H 
-    | [ H : in_parser (Char_p _) _ _ |- _ ] => generalize (inv_char_pi H) ; clear H 
-    | [ H : in_parser Eps_p _ _ |- _ ] => generalize (inv_eps_pi H) ; clear H
-    | [ H : in_parser (Cat_p _ _) _ _ |- _ ] => generalize (inv_cat_pi H) ; clear H
-    | [ H : in_parser (_ $ _) _ _ |- _ ] => generalize (inv_cat_pi H) ; clear H
-    | [ H : in_parser (_ |+| _) _ _ |- _ ] => generalize (inv_alt_pi H) ; clear H
-    | [ H : in_parser (Zero_p _) _ _ |- _ ] => contradiction (inv_zero_pi H)
-    | [ H : in_parser (_ @ _) _ _ |- _ ] => generalize (inv_map_pi H) ; clear H    
-    | [ H : in_parser (Map_p _ _ _) _ _ |- _ ] => generalize (inv_map_pi H) ; clear H    
+    | [ H : in_grammar (alt _ _) _ _ |- _ ] => generalize (inv_alt H) ; clear H
+    | [ H : in_grammar Eps _ _ |- _ ] => generalize (EpsInv H) ; clear H
+    | [ H : in_grammar Any _ _ |- _ ] => generalize (AnyInv H) ; clear H
+    | [ H : in_grammar (Char _) _ _ |- _ ] => generalize (CharInv H) ; clear H
+    | [ H : in_grammar (Alt _ _) _ _ |- _ ] => generalize (AltInv H) ; clear H
+    | [ H : in_grammar (seq _ _) _ _ |- _ ] => generalize (CatInv H) ; clear H
+    | [ H : in_grammar (Cat _ _) _ _ |- _ ] => generalize (CatInv H) ; clear H
+    | [ H : in_grammar (never _) _ _ |- _ ] => contradiction (inv_never H)
+    | [ H : in_grammar (Zero _) _ _ |- _ ] => contradiction (ZeroInv H)
+    | [ H : in_grammar (_ @ _) _ _ |- _ ] => generalize (MapInv H) ; clear H
+    | [ H : in_grammar (Map _ _ _) _ _ |- _ ] => generalize (MapInv H) ; clear H
+    | [ H : in_grammar (Xform _ _) _ _ |- _ ] => generalize (XformInv H) ; clear H
     | [ H : _::_ = _::_ |- _] => injection H ; clear H
     | [ H : true = true |- _ ] => clear H
     | [ H : true = _ |- _ ] => generalize (eq_sym H) ; clear H ; intro H
@@ -102,18 +93,90 @@ Ltac pinv :=
           destruct x1 ; destruct x2 ; simpl in H ; try congruence
     | [ H : ?x = ?x -> _ |- _ ] => specialize (H (eq_refl x))
     | [ H : _ \/ _ |- _ ] => destruct H
-    | [ IH : forall _ _ _ _, in_parser ?p1 _ _ -> in_parser ?p2 _ _ -> _, 
-      H1 : in_parser ?p1 _ _, H2 : in_parser ?p2 _ _ |- _ ] => 
+    | [ IH : forall _ _ _ _, in_grammar ?p1 _ _ -> in_grammar ?p2 _ _ -> _, 
+      H1 : in_grammar ?p1 _ _, H2 : in_grammar ?p2 _ _ |- _ ] => 
     specialize (IH _ _ _ _ H1 H2)
   end ; t ; subst.
 
-Lemma in_alts_app : forall t (ps qs:list (parser t)) s v,
-  in_parser (alts ps) s v \/ in_parser (alts qs) s v ->
-  in_parser (alts (ps ++ qs)) s v.
+Lemma in_alts0_simp : 
+  forall t (ps: list (grammar t)) s v, 
+    in_grammar (alts0 ps) s v <-> in_grammar (List.fold_right (@alt t) (@never t) ps) s v.
+Proof. 
+  induction ps ; simpl ; intros. tauto. destruct ps. simpl.
+  split. intro. econstructor. econstructor. eauto. eauto. auto.
+  intro ; repeat pinv ; auto. 
+  split ; intro. pinv. pinv. eauto. eapply in_alt_r. eapply IHps. auto.
+  pinv. pinv. eauto. eapply in_alt_r. eapply IHps. auto.
+Qed.
+
+Lemma half_app : forall A (xs ys zs a b: list A), 
+  half xs ys zs = (a,b) -> 
+  (forall x, (In x xs \/ In x ys \/ In x zs) <-> (In x a) \/ (In x b)).
 Proof.
-  induction ps ; simpl ; intros ; unfold never in * ; repeat pinv ; auto.
-  econstructor. auto. eapply Alt_right_pi. eauto. 
-  eapply Alt_right_pi. eauto.
+  induction xs. simpl. intros. injection H. intros ; subst. tauto.
+  simpl. intros. specialize (IHxs _ _ _ _ H x). simpl in *. tauto.
+Qed. 
+
+Lemma in_simp_alts t (ps:list (grammar t)) cs v : 
+  in_grammar (List.fold_right (@alt t) (@never t) ps) cs v <-> 
+  exists p, In p ps /\ in_grammar p cs v.
+Proof.
+  induction ps. simpl. intros ; split ; intro. pinv. destruct H as [_ [H _]]. contradiction.
+  simpl. intros. split. intro ; repeat pinv. exists a. auto.
+  specialize (IHps cs v). destruct IHps. specialize (H0 H). clear H1 H. 
+  destruct H0 as [p [H0 H]]. eauto. intro. mysimp ; subst. eauto.
+  eapply in_alt_r. specialize (IHps cs v). destruct IHps. eauto.
+Qed.
+
+Lemma in_alts' n t (ps:list (grammar t)) cs v : 
+  in_grammar (alts' n ps) cs v <-> 
+  in_grammar (List.fold_right (@alt t) (@never t) ps) cs v.
+Proof.
+  induction n. apply in_alts0_simp.
+  destruct ps. simpl. tauto. destruct ps. simpl.
+  intros. split ; eauto. intros ; repeat pinv ; auto. intros.
+  simpl. remember (half ps (g::nil) (g0::nil)) as p. destruct p as [ps1 ps2].
+  generalize (IHn _ ps1 cs v) (IHn _ ps2 cs v). intros.
+  generalize (half_app _ _ _ (eq_sym Heqp)). intros.
+  split. intro. repeat pinv. destruct H as [H _]. specialize (H H2). clear H0 H2.
+  assert (exists p, In p ps1 /\ in_grammar p cs v). apply in_simp_alts ; auto.
+  destruct H0 as [p [H0 H2]]. specialize (H1 p). destruct H1 as [_ H1].
+  specialize (H1 (or_introl H0)). 
+  repeat pinv. eapply in_alt_r. eapply in_alt_r. eapply in_simp_alts. eauto.
+  simpl in *. repeat pinv ; try contradiction ; eauto.
+  simpl in * ; repeat pinv ; try contradiction ; eauto.
+  destruct H0 as [H0 _]. specialize (H0 H2). clear H H2.
+  assert (exists p, In p ps2 /\ in_grammar p cs v). apply in_simp_alts. auto.
+  destruct H as [p [H H2]]. specialize (H1 p). destruct H1 as [_ H1].
+  specialize (H1 (or_intror H)). 
+  repeat pinv. eapply in_alt_r. eapply in_alt_r. eapply in_simp_alts ; eauto.
+  simpl in *. repeat pinv ; try contradiction ; eauto.
+  simpl in * ; repeat pinv ; try contradiction ; eauto.
+  intro. repeat pinv. assert (In g ps1 \/ In g ps2). apply H1. 
+  right. left ; auto. simpl. auto. clear H1. destruct H3.
+  apply in_alt_l. apply H. apply in_simp_alts. exists g. auto.
+  apply in_alt_r. apply H0. apply in_simp_alts. exists g ; auto.
+  assert (In g0 ps1 \/ In g0 ps2). apply H1. right. right ; simpl ; auto.
+  clear H1. destruct H3. apply in_alt_l. apply H. apply in_simp_alts. eauto.
+  apply in_alt_r. apply H0. apply in_simp_alts. eauto.
+  generalize (in_simp_alts ps cs v). intros. destruct H3 as [H3 _].
+  specialize (H3 H2). destruct H3. destruct H3. assert (In x ps1 \/ In x ps2).
+  apply H1. auto. destruct H5. eapply in_alt_l. apply H. apply in_simp_alts ; eauto.
+  eapply in_alt_r. apply H0. eapply in_simp_alts ; eauto.
+Qed.
+
+Lemma in_alts t (ps:list (grammar t)) cs v : 
+  in_grammar (alts ps) cs v <-> in_grammar (List.fold_right (@alt t) (@never t) ps) cs v.
+Proof.
+  intros. apply in_alts'.
+Qed.
+
+Lemma in_alts_app : forall t (ps qs:list (grammar t)) s v,
+  in_grammar (alts ps) s v \/ in_grammar (alts qs) s v ->
+  in_grammar (alts (ps ++ qs)) s v.
+Proof.
+  intros. rewrite in_alts in *. rewrite in_alts in H.
+  induction ps ; simpl in *; repeat pinv ; auto.
 Qed.
 
 Lemma app_cons_nil A (x:A) (ys:list A) (y:A) (zs:list A) : 
@@ -123,29 +186,31 @@ Proof.
   simpl in *. intros. specialize (IHys y zs). discriminate H.
 Qed.
 
-(** These next few lemmas are used to invert parsers so that we can
+(** These next few lemmas are used to invert grammars so that we can
     figure out what kinds of values they build. *)
-Lemma in_app_alts : forall t (ps1 ps2:list (parser t)) s v,
-  in_parser (alts (ps1 ++ ps2)) s v -> 
-  in_parser (alts ps1) s v \/ in_parser (alts ps2) s v.
+Lemma in_app_alts : forall t (ps1 ps2:list (grammar t)) s v,
+  in_grammar (alts (ps1 ++ ps2)) s v -> 
+  in_grammar (alts ps1) s v \/ in_grammar (alts ps2) s v.
 Proof.
+  intros. rewrite in_alts in *. rewrite in_alts. generalize ps2 s v H ; clear ps2 s v H.
   induction ps1 ; simpl ; intros. right. auto. repeat pinv. left. econstructor ; eauto.
-  specialize (IHps1 _ _ _ H). pinv. left. eapply Alt_right_pi. auto. right. auto.
+  specialize (IHps1 _ _ _ H). pinv. left. eauto. right. eauto.
 Qed.
 
-Lemma in_alts_map : forall t1 t2 (p1:parser t1) (ps:list (parser t2)) s v,
-  in_parser (alts (List.map (fun p2 => Cat_p p1 p2) ps)) s v -> 
-  in_parser (Cat_p p1 (alts ps)) s v.
+Lemma in_alts_map : forall t1 t2 (p1:grammar t1) (ps:list (grammar t2)) s v,
+  in_grammar (alts (List.map (fun p2 => Cat p1 p2) ps)) s v -> 
+  in_grammar (Cat p1 (alts ps)) s v.
 Proof.
-  induction ps ; simpl ; unfold never ; intros ; repeat pinv. 
-  econstructor. eauto. econstructor. eauto. auto. auto.
-  specialize (IHps _ _ H). pinv. econstructor. eauto. eapply Alt_right_pi.
-  eauto. auto. auto.
+  induction ps ; simpl ; intros ; rewrite in_alts in * ; simpl in * ; repeat pinv.
+  econstructor. eauto. rewrite in_alts. simpl. econstructor. eauto. auto. auto. auto.
+  specialize (IHps s v). rewrite in_alts in IHps. specialize (IHps H).
+  pinv. econstructor. eauto. rewrite in_alts ; simpl. eapply in_alt_r.
+  rewrite in_alts in H1. eauto. eauto. auto. 
 Qed.
 
-Lemma inv_bitsleft bs t (p:parser t) s v : 
-  in_parser (bs $$ p) s v -> 
-  exists s1, exists s2, s = s1 ++ s2 /\ in_parser p s2 v.
+Lemma inv_bitsleft bs t (p:grammar t) s v : 
+  in_grammar (bs $$ p) s v -> 
+  exists s1, exists s2, s = s1 ++ s2 /\ in_grammar p s2 v.
 Proof.
   unfold bitsleft. induction bs ; simpl ; intros ; repeat pinv ; simpl.
   exists nil. exists x1. auto.
@@ -154,51 +219,53 @@ Proof.
 Qed.
 
 Lemma inv_modrm : forall s p,
-  in_parser modrm s p -> 
+  in_grammar modrm s p -> 
   match p with | (_, Imm_op _) => False | (Reg_op r, op) => True | _ => False end.
 Proof.
-  unfold modrm. intros. repeat pinv ; auto. unfold rm00 in *. repeat pinv ; auto.
-  unfold rm01 in *. repeat pinv ; auto. destruct x9 ; auto. unfold rm10 in * ; 
-  repeat pinv ; auto. destruct x9 ; auto. unfold rm11 in * ; repeat pinv ; auto.
+  unfold modrm. unfold modrm_gen. simpl. intros.
+  repeat pinv ; auto. unfold rm00, bitsleft, reg_op, reg in * ;
+  repeat pinv ; auto ; simpl ; auto. 
+  unfold rm01, bitsleft, reg_op, reg in *. repeat pinv ; simpl ; auto. 
+  unfold rm10, bitsleft, reg_op, reg in *. repeat pinv ; simpl ; auto.
+  unfold reg_op, bitsleft, reg in *. repeat pinv ; simpl ; auto.
 Qed.
 
 Lemma inv_ext_modrm : forall bs s v,
-  in_parser (ext_op_modrm bs) s v -> match v with | Imm_op _ => False | _ => True end.
+  in_grammar (ext_op_modrm bs) s v -> match v with | Imm_op _ => False | _ => True end.
 Proof.
-  unfold ext_op_modrm. intros. repeat pinv. unfold rm00 in *. repeat pinv ; auto.
-  unfold rm01 in *. repeat pinv ; auto. destruct x9. auto. 
-  unfold rm10 in *. repeat pinv ; auto. destruct x9. auto.
+  unfold ext_op_modrm. unfold ext_op_modrm_gen. simpl. 
+  intros. repeat pinv ; auto. 
 Qed.
 
 Lemma inv_ext_modrm2 : forall bs s v,
-  in_parser (ext_op_modrm2 bs) s v -> match v with | Imm_op _ => False | _ => True end.
+  in_grammar (ext_op_modrm2 bs) s v -> match v with | Imm_op _ => False | _ => True end.
 Proof.
-  unfold ext_op_modrm2. intros. repeat pinv. unfold rm00 in *. repeat pinv ; auto.
-  unfold rm01 in *. repeat pinv ; auto. destruct x9 ; auto.
-  unfold rm10 in *. repeat pinv ; auto. destruct x9 ; auto.
-  unfold rm11 in *. repeat pinv ; auto.
+  unfold ext_op_modrm2. unfold ext_op_modrm2_gen ; simpl. intros. 
+  repeat pinv ; auto. unfold bitsleft, reg_op in *. repeat pinv ; simpl ; auto.
 Qed.
 
-(** A tactic for applying these inversion properties on parsers to simplify
+(** A tactic for applying these inversion properties on grammars to simplify
     them down to the cases we want to consider. *)
 Ltac psimp := 
   simpl in * ;
   match goal with 
     | [ H : prod _ _ |- _ ] => destruct H
     | [ H : (_,_) = (_,_) |- _ ] => injection H ; clear H ; intros ; subst
-    | [ H : in_parser (_ $$ _) _ _ |- _ ] => 
+    | [ H : in_grammar (_ $$ _) _ _ |- _ ] => 
       generalize (inv_bitsleft H) ; clear H ; t ; subst
-    | [ H : in_parser modrm _ _ |- _ ] => generalize (inv_modrm H) ; clear H ; t
-    | [ H : in_parser (ext_op_modrm ?bs) _ _ |- _ ] => 
+    | [ H : in_grammar modrm _ _ |- _ ] => generalize (inv_modrm H) ; clear H ; t
+    | [ H : in_grammar (ext_op_modrm ?bs) _ _ |- _ ] => 
       generalize (@inv_ext_modrm bs _ _ H) ; clear H ; t
-    | [ H : in_parser (ext_op_modrm2 ?bs) _ _ |- _ ] => 
+    | [ H : in_grammar (ext_op_modrm2 ?bs) _ _ |- _ ] => 
       generalize (@inv_ext_modrm2 bs _ _ H) ; clear H ; t
   end.
 
 (** Main connecton between non_cflow_dfa and semantics -- this is hopefully
-    close enough to the actual parser used in the semantics that proving
+    close enough to the actual grammar used in the semantics that proving
     a relationship is easy to do.  We will see... *)
-Fixpoint simple_parse' (ps:X86_PARSER.instParserState) (bytes:list int8) : 
+Require Import X86Semantics.
+
+Fixpoint simple_parse' (ps:ParseState_t) (bytes:list int8) : 
   option ((prefix * instr) * list int8) := 
   match bytes with 
     | nil => None
@@ -208,366 +275,412 @@ Fixpoint simple_parse' (ps:X86_PARSER.instParserState) (bytes:list int8) :
                end
   end.
 
-Definition simple_parse (bytes:list int8) : option ((prefix * instr) * list int8) := 
-  simple_parse' X86_PARSER.initial_parser_state bytes.
+Section CONFUSE_COQ_FROM_EXPANDING.
+Variable init_p_state : option ParseState_t.
+Definition simple_parse'' (bytes:list int8) : option ((prefix * instr) * list int8) := 
+  match init_p_state with
+      | None => None
+      | Some s => simple_parse' s bytes
+  end.
+End CONFUSE_COQ_FROM_EXPANDING.
+Definition simple_parse := simple_parse'' initial_parser_state.
 
 Definition byte2token (b: int8) : token_id := Zabs_nat (Word.unsigned b).
 
-(** The [valid_prefix_parser_nooveride] parser only builds a [prefix] that satisfies
-   [only_gs_seg_override]. *)
-Lemma pfx_nooverride : forall s v, 
-  in_parser valid_prefix_parser_nooverride s v -> only_gs_seg_override v = true.
-Proof.
-  unfold only_gs_seg_override, valid_prefix_parser_nooverride. intros. repeat pinv ;
-  simpl ; auto. 
-Qed.
-
-(** The [only_op_override] satisfies [either_prefix]. *)
-Lemma pfx_nooverride_imp_either : forall pfx,
-  only_op_override pfx = true -> either_prefix pfx = true.
-Proof.
-  destruct pfx ; unfold only_op_override, either_prefix ; simpl ; intros ; 
-  unfold only_op_override, only_gs_seg_override ; simpl. 
-  destruct lock_rep ; try congruence. destruct seg_override ; try congruence.
-  rewrite H. auto.
-Qed.
-
-(** [only_gs_segoverride] implies [either_prefix] *)
-Lemma pfx_gs_seg_imp_either : forall pfx,
-  only_gs_seg_override pfx = true -> either_prefix pfx = true.
-Proof.
-  destruct pfx ; unfold only_gs_seg_override, either_prefix ; simpl ; intros ; 
-  unfold only_op_override, only_gs_seg_override ; simpl. 
-  destruct lock_rep ; try congruence. destruct seg_override ; try congruence.
-  rewrite H. auto. rewrite H. destruct addr_override ; auto.
-Qed.
-
-(** The [valid_prefix_parser_rep] only builds a [prefix] that satisfies
-    [only_lock_or_rep]. *)
-Lemma pfx_rep : forall s v,
-  in_parser valid_prefix_parser_rep s v -> only_lock_or_rep v = true.
-Proof.
-  unfold valid_prefix_parser_rep, only_lock_or_rep ; intros ; repeat pinv ; auto.
-Qed.
-
-(** This lemma shows that any instruction returned by the [non_cflow_parser]
+(** This lemma shows that any instruction returned by the [non_cflow_grammar]
     satisfies the boolean predicate [non_cflow_instr].  We should probably
     break this up into a lot of little lemmas to make it a little easier
     to adapt. *)
-Lemma non_cflow_instr_inv (pre:prefix) (ins:instr) (s:list char_p) :
-  in_parser VerifierDFA.non_cflow_parser s (pre,ins) -> 
+
+Lemma valid_prefix_grammar_rep_non_cflow pre s : 
+  in_grammar valid_prefix_grammar_rep s pre -> 
+  rep_or_gs_or_op_prefix pre = true.
+Proof.
+  intros pre s. unfold valid_prefix_grammar_rep, option_perm3, rep_or_gs_or_op_prefix.
+  intro. repeat pinv ; simpl ; auto. unfold rep_p, bitsleft in *. repeat pinv. auto.
+  unfold gs_segment_override_p, bitsleft in H. repeat pinv. auto.
+  unfold perm2, rep_p, gs_segment_override_p, bitsleft in H. repeat pinv ; auto.
+  unfold perm2, rep_p, op_override_p, bitsleft in H. repeat pinv ; auto.
+  unfold perm2, gs_segment_override_p, op_override_p, bitsleft in H. repeat pinv ; auto.
+  unfold perm3, rep_p, gs_segment_override_p, op_override_p, bitsleft in H.
+  repeat pinv ; auto. unfold perm2 in * ; repeat pinv ; auto.
+  unfold perm2 in * ; repeat pinv ; auto. unfold perm2 in * ; repeat pinv ; auto.
+Qed.                                  
+
+Lemma valid_instr_grammars_rep_non_cflow pre ins s : 
+  in_grammar (alts (List.map (fun p => valid_prefix_grammar_rep $ p)
+                             valid_instr_grammars_rep)) s (pre, ins) -> 
   non_cflow_instr pre ins = true.
 Proof.
-  unfold VerifierDFA.non_cflow_parser, VerifierDFA.non_cflow_parser_list, 
-    VerifierDFA.non_cflow_instrs_rep_pre.
-  intros. generalize (in_app_alts _ _ H). clear H. intros.
-  destruct H ;
-    [idtac | generalize (in_app_alts _ _ H) ; clear H ; intro H ; destruct H] ;
-  generalize (in_alts_map _ _ H) ; clear H ; intros ; pinv ;
-    injection H0 ; intros ; clear H0 ; subst.
-  generalize (pfx_nooverride H1). clear H1. intros.
-  generalize (pfx_gs_seg_imp_either _ H). intros.
+  unfold valid_instr_grammars_rep. simpl. intros pre ins s.
+  rewrite in_alts. simpl. intros. 
+  repeat pinv ; injection H2 ; clear H2 ; intros ; subst ; 
+  unfold MOVS_p, STOS_p in * ; unfold bitsleft in * ; repeat pinv ; simpl in * ; 
+  eapply valid_prefix_grammar_rep_non_cflow ; eauto.
+Qed.
 
-  unfold non_cflow_instrs_nosize_pre in *. simpl in *. repeat pinv.
-  (* simple instructions *)
-  Ltac punf c := unfold c in *; simpl in * ; pinv ; auto.
-  (* logic or arithmetic instructions *)
-  (* bit-test instructions *)
-  Lemma bit_test : forall pfx I x1 x2 s i,
-    only_gs_seg_override pfx = true -> 
-    in_parser (bit_test_p x1 x2 I) s i -> 
-    (forall op1 op2, no_imm_op op1 = true -> non_cflow_instr pfx (I op1 op2) = true) -> 
-    non_cflow_instr pfx i = true.
-  Proof.
-    unfold bit_test_p. intros. repeat pinv ; repeat psimp ; repeat pinv ; 
-    repeat psimp. eauto. destruct x8 ; try contradiction . eauto. eauto.
-    eauto. destruct o. destruct o0 ; auto. destruct o0 ; auto. destruct o0 ; auto.
-    destruct o0 ; auto.
-  Qed.
-  Ltac btest c := unfold c in * ; eapply bit_test ; simpl ; eauto ; intros ; auto.
-  (* unary operations and a bunch of others *)
-  Ltac unop c := 
-    punf c ; repeat pinv ; repeat psimp ; auto ; repeat pinv ; repeat psimp ; 
-      match goal with 
-        | [ H : match ?x with | Imm_op _ => _ | Reg_op _ => _ | Address_op _ => _ | Offset_op _ => _ end |- _ ] => destruct x ; try contradiction ; auto
-      end.
-  (* rotate and shift instructions *)
-  Lemma rotate : forall pfx x I s i, in_parser (rotate_p x I) s i -> 
-    only_gs_seg_override pfx = true ->
-    (forall b op ri, no_imm_op op = true -> non_cflow_instr pfx (I b op ri) = true) -> 
-    non_cflow_instr pfx i = true.
-  Proof.
-    unfold rotate_p. intros. repeat pinv ; repeat psimp ; repeat pinv ; 
-    repeat psimp ; eauto ; try (destruct x6 ; try contradiction ; eauto).
-    destruct x8 ; try contradiction ; eauto.
-  Qed.
-  Ltac rot c := unfold c in * ; eapply rotate ; eauto ; simpl ; intros ; auto.
-  Lemma shiftdouble : forall pfx x I s i, 
-    only_gs_seg_override pfx = true ->
-    in_parser (shiftdouble_p x I) s i -> 
-    (forall op r ri, no_imm_op op = true -> non_cflow_instr pfx (I op r ri) = true) -> 
-    non_cflow_instr pfx i = true.
-  Proof.
-    unfold shiftdouble_p, modrm_noreg. intros ; repeat pinv ; repeat psimp ; 
-    repeat pinv ; repeat psimp ; eauto ; repeat pinv ; repeat psimp ; 
-    unfold rm01, rm00, rm10 in * ; repeat pinv ; auto ; 
-    try (destruct x16 ; auto) ; try (destruct x14 ; auto).
-  Qed.
-  Ltac shdouble c := unfold c in * ; eapply shiftdouble ; eauto ; intros ; simpl ; auto.
-  Lemma logic_or_arith : forall pfx I b x1 x2 s i, 
-    either_prefix pfx = true ->
-    in_parser (logic_or_arith_p b x1 x2 I) s i -> 
-    (forall b op1 op2, no_imm_op op1 = true -> 
-        non_cflow_instr pfx (I b op1 op2) = true) ->
-    non_cflow_instr pfx i = true.
-  Proof.
-    intros. unfold logic_or_arith_p in * ; repeat pinv ; repeat psimp ; 
-    repeat pinv ; repeat psimp ;try (destruct o1 ; destruct o2 ; try 
-      contradiction ; eauto ; destruct x6 ; eauto) ; eauto ;
-    destruct x6 ; try contradiction ; eauto.
-  Qed.
-  Lemma simple_andb : forall x y, x = true -> y = true -> x && y = true.
-    intros. subst. auto.
-  Qed.
-  Hint Resolve simple_andb.
-  Ltac log_or_arith c := 
-    unfold c in *; eapply logic_or_arith ; eauto ; intros ; simpl ; eauto.
-  (* AAA_p *)
-  punf AAA_p.
-  (* AAD_p *)
-  punf AAD_p.
-  (* AAM_p *)
-  punf AAM_p.
-  (* AAS_p *)
-  punf AAS_p.
-  (* ADC_p *)
-  log_or_arith ADC_p.
-  (* ADD_p *)
-  log_or_arith ADD_p.
-  (* AND_p *)
-  log_or_arith AND_p.
-  (* CMP_p *)
-  log_or_arith CMP_p.
-  (* OR_p *)
-  log_or_arith OR_p.
-  (* SBB_p *)
-  log_or_arith SBB_p.
-  (* SUB_p *)
-  log_or_arith SUB_p.
-  (* XOR_p *)
-  log_or_arith XOR_p.
-  (* BSF_p *)
-  unfold BSF_p in *. repeat pinv ; repeat psimp. 
-  rewrite H. destruct o ; try contradiction ; auto. 
-  destruct o0 ; contradiction. 
-  (* BSR_p *)
-  unfold BSR_p in *. repeat pinv ; repeat psimp. 
-  rewrite H.
-  destruct o ; try contradiction ; auto.
-  destruct o0 ; contradiction.
-  (* BSWAP_p *)
-  punf BSWAP_p.
-  (* BT_p *)
-  btest BT_p. simpl. auto.
-  (* BTC_p *)
-  btest BTC_p. simpl. auto.
-  (* BTR_p *)
-  btest BTR_p. simpl. eauto.
-  (* BTS_p *)
-  btest BTS_p. simpl. auto.
-  (* CDQ_p *)
-  punf CDQ_p. 
-  (* CLC_p *)
-  punf CLC_p.
-  (* CLD_p *)
-  (* FIX:  why does NACL accept CLD? *)
-  punf CLD_p.
-  (* CMOVcc_p *)
-  punf CMOVcc_p ; repeat psimp ; repeat pinv ; repeat psimp ; destruct o1 ; 
-    try contradiction ; auto ; destruct o2 ; try contradiction ; eauto.
-  (* CMC_p *)
-  punf CMC_p.
-  (* CMPXCHG_p *)
-  punf CMPXCHG_p ; repeat psimp ; repeat pinv ; repeat psimp ; destruct o1 ; 
-    try contradiction ; auto ; destruct o2 ; auto.
-  (* CWDE_p *)
-  punf CWDE_p.
-  (* DAA_p *)
-  punf DAA_p.
-  (* DAS_p *)
-  punf DAS_p.
-  (* DEC_p *)
-  unop DEC_p.
-  (* DIV_p *)
-  unop DIV_p.
-  (* FIX: why does NACL accept HLT? *)
-  (* HLT_p *)
-  punf HLT_p.
-  (* IDIV_p *)
-  unop IDIV_p.
-  (* IMUL_p *)
-  unop IMUL_p ; try (destruct o0 ; contradiction) ; try (destruct o2 ; contradiction).
-  (* INC_p *)
-  unop INC_p.
-  (* LAHF_p *)
-  punf LAHF_p.
-  (* LEA_p *)
-  punf LEA_p. repeat psimp. unfold modrm_noreg, rm00, rm01, rm10 in *. 
-  repeat pinv ; repeat psimp ; repeat pinv ; repeat psimp ; auto.
-  (* LEAVE_p *)
-  punf LEAVE_p.
-  (* MOV_p *)
-  unop MOV_p ; destruct o2 ; auto.
-  (* MOVSX_p *)
-  unop MOVSX_p ; destruct o2 ; auto. 
-  (* MOVZX_p *)
-  unop MOVZX_p ; destruct o2 ; auto.
-  (* MUL_p *)
-  unop MUL_p.
-  (* NEG_p *)
-  unop NEG_p.
-  (* NOT_p *)
-  unop NOT_p.
-  (* POP_p *)
-  unop POP_p.
-  (* POPA_p *)
-  punf POPA_p.
-  (* PUSH_p *)
-  unop PUSH_p.
-  (* PUSHA_p *)
-  unop PUSHA_p.
-  (* RCL_p *)
-  rot RCL_p.
-  (* RCR_p *)
-  rot RCR_p.
-  (* ROL_p *)
-  rot ROL_p.
-  (* ROR_p *)
-  rot ROR_p.
-  (* SAHF_p *)
-  punf SAHF_p.
-  (* SAR_p *)
-  rot SAR_p.
-  (* SETcc_p *)
-  unop SETcc_p ; destruct o2 ; auto.
-  (* SHL_p *)
-  rot SHL_p.
-  (* SHLD_p *)
-  shdouble SHLD_p.
-  (* SHR_p *)
-  rot SHR_p.
-  (* SHRD_p *)
-  shdouble SHRD_p.
-  (* STC_p *)
-  punf STC_p.
-  (* STD_p *)
-  punf STD_p. 
-  (* TEST_p *)
-  unop TEST_p.
-  (* XADD_p *)
-  unop XADD_p ; destruct o2 ; auto.
-  (* XCHG_p *)
-  unop XCHG_p ; destruct o2 ; auto. 
-  (* never *)
-  unfold never in * ; pinv.
-  (****************************************************************)
-  (* now to do the opsize_pre *)
-  Lemma opsize_prefix : forall s v,
-    in_parser valid_prefix_parser_opsize s v -> only_op_override v = true /\ 
-    either_prefix v = true.
-  Proof.
+Lemma valid_prefix_grammar_rep_or_repn_non_cflow pre s : 
+  in_grammar valid_prefix_grammar_rep_or_repn s pre -> 
+  rep_or_repn_or_gs_or_op_prefix pre = true.
+Proof.
+  unfold valid_prefix_grammar_rep_or_repn, rep_or_repn_or_gs_or_op_prefix, 
+  option_perm3, rep_or_repn_p, gs_segment_override_p, op_override_p, bitsleft.
+  intros. repeat pinv ; auto ; unfold perm3 in * ; repeat pinv ; auto ; 
+          unfold perm2 in * ; repeat pinv ; auto.
+Qed.
+
+Lemma valid_instr_grammars_rep_or_repn_non_cflow pre ins s : 
+  in_grammar (alts (List.map (fun p => valid_prefix_grammar_rep_or_repn $ p)
+                             valid_instr_grammars_rep_or_repn)) s (pre, ins) -> 
+  non_cflow_instr pre ins = true.
+Proof.
+  unfold valid_instr_grammars_rep_or_repn. unfold instr_grammars_rep_or_repn.
+  simpl ; intros pre ins s. rewrite in_alts. simpl ; intros.
+  unfold CMPS_p, SCAS_p, bitsleft in *. 
+  repeat pinv ; injection H2 ; clear H2 ; intros ; subst ; simpl ; 
+  eapply valid_prefix_grammar_rep_or_repn_non_cflow ; eauto.
+Qed.
+
+Lemma valid_prefix_grammar_lock_with_op_override_non_cflow pre s : 
+  in_grammar valid_prefix_grammar_lock_with_op_override s pre -> 
+  lock_or_gs_with_op pre = true.
+Proof.
+  unfold valid_prefix_grammar_lock_with_op_override.
+  unfold option_perm3_variation, lock_p, gs_segment_override_p, op_override_p, 
+  perm3, perm2. intros. repeat (repeat pinv ; repeat psimp) ; auto.
+Qed.
+
+Lemma valid_prefix_grammar_lock_no_op_override_non_cflow pre s : 
+  in_grammar valid_prefix_grammar_lock_no_op_override s pre -> 
+  lock_or_gs_without_op pre = true.
+Proof.
+  unfold valid_prefix_grammar_lock_no_op_override.
+  unfold option_perm3_variation, option_perm2, 
+  lock_p, gs_segment_override_p, op_override_p, 
+  perm3, perm2. 
+  intros. repeat (repeat pinv ; repeat psimp) ; unfold lock_or_gs_without_op ; auto.
+Qed.
+
+Lemma valid_instr_grammars_lock_with_op_override_non_cflow pre ins s : 
+  in_grammar (alts (List.map (fun p => valid_prefix_grammar_lock_with_op_override $ p)
+                             valid_instr_grammars_lock_with_op_override)) s (pre,ins) ->
+  non_cflow_instr pre ins = true.
+Proof.
+  unfold valid_instr_grammars_lock_with_op_override.
+  unfold instr_grammars_lock_with_op_override.
+  simpl. intros pre ins s. rewrite in_alts. simpl ; intros.
+  Ltac unf1 := 
+  unfold ADD_p, ADC_p, AND_p, NEG_p, NOT_p, OR_p, SBB_p, SUB_p, XOR_p, XCHG_p,
+    logic_or_arith_p in *.
+  repeat pinv ; injection H2 ; clear H2 ; intros ; subst ; simpl ;
+  unf1 ; repeat (repeat pinv ; repeat psimp) ; 
+  repeat 
+    (simpl ; 
+     match goal with 
+       | [ H : match ?x with | Imm_op _ => _ | Reg_op _ => _ | Address_op _ => _ | Offset_op _ => _ end |- _ ] => destruct x ; try contradiction
+       | [ |- context[if ?x then _ else _]] => destruct x
+       | [ H : in_grammar valid_prefix_grammar_lock_with_op_override _ _ |- _ ] => 
+         rewrite (valid_prefix_grammar_lock_with_op_override_non_cflow H) ; auto
+       | _ => idtac
+  end).
+Qed.
+
+Lemma valid_instr_grammars_lock_no_op_override_non_cflow pre ins s : 
+  in_grammar (alts (List.map (fun (p:grammar instruction_t) => 
+                                valid_prefix_grammar_lock_no_op_override $ p)
+                             valid_instr_grammars_lock_no_op_override)) s (pre,ins) ->
+  non_cflow_instr pre ins = true.
+Proof.
+  unfold valid_instr_grammars_lock_no_op_override.
+  unfold instr_grammars_lock_no_op_override.
+  simpl ; intros pre ins s ; rewrite in_alts ; simpl ; intros.
+  repeat pinv ; injection H2 ; clear H2 ; intros ; subst ; simpl ; 
+  unfold ADD_p, ADC_p, AND_p, BTC_p, BTR_p, BTS_p, CMPXCHG_p, DEC_p, INC_p, NEG_p, 
+  NOT_p, OR_p, SBB_p, SUB_p, XOR_p, XADD_p, XCHG_p, logic_or_arith_p, bit_test_p in * ; 
+  repeat (repeat pinv ; repeat psimp) ; 
+  repeat 
+    (simpl ; 
+     match goal with 
+       | [ H : match ?x with | Imm_op _ => _ | Reg_op _ => _ | Address_op _ => _ | Offset_op _ => _ end |- _ ] => destruct x ; try contradiction
+       | [ |- context[if ?x then _ else _]] => destruct x
+       | [ H : in_grammar valid_prefix_grammar_lock_no_op_override _ _ |- _ ] => 
+         rewrite (valid_prefix_grammar_lock_no_op_override_non_cflow H) ; auto
+       | [ |- _ || true = true ] => apply orb_true_r 
+       | _ => idtac
+  end).
+Qed.
+
+Lemma valid_prefix_grammar_seg_with_op_override_non_cflow pre s : 
+  in_grammar valid_prefix_grammar_seg_with_op_override s pre -> 
+  only_seg_or_op pre = true.
+Proof.
+  unfold valid_prefix_grammar_seg_with_op_override.
+  unfold option_perm2_variation, gs_segment_override_p, op_override_p, perm2.
+  intros. repeat pinv ; repeat psimp ; unfold only_seg_or_op ; auto.
+Qed.
+
+Lemma valid_instr_grammars_seg_with_op_override_non_cflow pre ins s : 
+  in_grammar (alts (List.map (fun (p:grammar instruction_t) => 
+                                valid_prefix_grammar_seg_with_op_override $ p)
+                             valid_instr_grammars_seg_with_op_override)) s (pre,ins) ->
+  non_cflow_instr pre ins = true.
+Proof.
+  unfold valid_instr_grammars_seg_with_op_override.
+  unfold instr_grammars_seg_with_op_override.
+  simpl ; intros pre ins s ; rewrite in_alts ; simpl ; intros.
+  repeat pinv ; injection H2 ; clear H2 ; intros ; subst ; simpl ; 
+  unfold CMP_p, IMUL_p, MOV_p, TEST_p, logic_or_arith_p in * ; 
+  repeat (repeat pinv ; repeat psimp) ;
+  repeat 
+    (simpl ; 
+     match goal with 
+       | [ H : match ?x with | Imm_op _ => _ | Reg_op _ => _ | Address_op _ => _ | Offset_op _ => _ end |- _ ] => destruct x ; try contradiction
+       | [ |- context[if ?x then _ else _]] => destruct x
+       | [ H : in_grammar  valid_prefix_grammar_seg_with_op_override _ _ |- _ ] => 
+         rewrite (valid_prefix_grammar_seg_with_op_override_non_cflow H) ; auto
+       | [ |- _ || true = true ] => apply orb_true_r 
+       | _ => idtac
+  end).
+Qed.
+
+Lemma valid_prefix_grammar_seg_op_override_non_cflow pre s : 
+  in_grammar valid_prefix_grammar_seg_op_override s pre -> 
+  only_seg_or_op pre = true.
+Proof.
+  unfold valid_prefix_grammar_seg_op_override, only_seg_or_op, option_perm2,
+  perm2, gs_segment_override_p, op_override_p ; intros ;
+  repeat (repeat pinv ; repeat psimp) ; auto.
+Qed.
+
+Lemma valid_instr_grammars_seg_op_override_non_cflow pre ins s : 
+  in_grammar (alts (List.map
+                      (fun p => valid_prefix_grammar_seg_op_override $ p)
+                      valid_instr_grammars_seg_op_override)) s (pre, ins) ->
+   non_cflow_instr pre ins = true.
+Proof.
+  unfold valid_instr_grammars_seg_op_override.
+  unfold instr_grammars_seg_op_override.
+  simpl ; intros pre ins s ; rewrite in_alts ; simpl ; intros.
+  repeat pinv ; injection H2 ; clear H2 ; intros ; subst ; simpl ; 
+  unfold CDQ_p, CMOVcc_p, CWDE_p, DIV_p, IDIV_p, MOVSX_p, MOVZX_p, MUL_p, 
+  NOP_p, ROL_p, ROR_p, SAR_p, SHL_p, SHLD_p, SHR_p, SHRD_p, rotate_p, 
+  shiftdouble_p, modrm_noreg, modrm_gen_noreg in * ; 
+  repeat (repeat pinv ; repeat psimp) ;
+  repeat match goal with 
+    | [ H : match ?x with | Imm_op _ => _ | Reg_op _ => _ | Address_op _ => _ | Offset_op _ => _ end |- _ ] => destruct x ; try contradiction
+    | [ |- context[if ?x then _ else _]] => destruct x
+    | [ H : in_grammar _ _ _ |- _ ] => 
+      rewrite (valid_prefix_grammar_seg_op_override_non_cflow H) ; auto
+    | _ => idtac
+  end.
+Qed.
+
+Lemma valid_prefix_grammar_seg_override_non_cflow pre s : 
+  in_grammar valid_prefix_grammar_seg_override s pre -> 
+  only_gs_seg_override pre = true.
+Proof.
+  unfold valid_prefix_grammar_seg_override. 
+  unfold option_perm, gs_segment_override_p.
+  intros. repeat pinv ; auto.
+Qed.
+
+Lemma only_gs_seg_override_imp_only_seg_or_op pre : 
+  only_gs_seg_override pre = true -> 
+  only_seg_or_op pre = true.
+Proof.
+  unfold only_gs_seg_override, only_seg_or_op. destruct pre.
+  simpl. destruct lock_rep ; auto. destruct seg_override ; auto.
+  destruct s ; auto. destruct op_override ; auto ; intros.
+  discriminate H. destruct op_override ; auto. intros ; discriminate H.
+Qed.
+
+Lemma modrm_mx_inv_left x y z : 
+  in_grammar modrm_mmx x (y,z) -> no_mmx_imm_op y = true.
+Proof.
+  unfold modrm_mmx. unfold modrm_gen, mmx_reg_op. intros. 
+  repeat (repeat pinv ; repeat psimp ; auto).
+Qed.
+
+Lemma modrm_mx_inv_right x y z : 
+  in_grammar modrm_mmx x (y,z) -> no_mmx_imm_op z = true.
+Proof.
+  unfold modrm_mmx. unfold modrm_gen, mmx_reg_op. intros. 
+  repeat (repeat pinv ; repeat psimp ; auto).
+Qed.
+
+Lemma modrm_xmm_inv_left x y z : 
+  in_grammar modrm_xmm x (y,z) -> no_sse_imm_op y = true.
+Proof.
+  unfold modrm_xmm. unfold modrm_gen, sse_reg_op. intros.
+  repeat (repeat pinv ; repeat psimp ; auto).
+Qed.
+
+Lemma modrm_xmm_inv_right x y z : 
+  in_grammar modrm_xmm x (y,z) -> no_sse_imm_op z = true.
+Proof.
+  unfold modrm_xmm. unfold modrm_gen, sse_reg_op. intros.
+  repeat (repeat pinv ; repeat psimp ; auto).
+Qed.
+
+Lemma modrm_xmm_noreg_inv_left x s s0 : 
+  in_grammar modrm_xmm_noreg x (s,s0) -> no_sse_imm_op s = true.
+Proof.
+  unfold modrm_xmm_noreg. unfold modrm_gen_noreg, sse_reg_op. intros.
+  repeat (repeat pinv ; repeat psimp) ; auto.
+Qed.
+
+Lemma modrm_xmm_noreg_inv_right x s s0 : 
+  in_grammar modrm_xmm_noreg x (s,s0) -> no_sse_imm_op s0 = true.
+Proof.
+  unfold modrm_xmm_noreg. unfold modrm_gen_noreg, sse_reg_op. intros.
+  repeat (repeat pinv ; repeat psimp) ; auto.
+Qed.
+
+Lemma modrm_xmm_gp_noreg_inv x s s0 : 
+  in_grammar modrm_xmm_gp_noreg x (s,s0) -> no_sse_imm_op s = true.
+Proof.
+  unfold modrm_xmm_gp_noreg. unfold modrm_gen_noreg. intros.
+  repeat (repeat pinv ; repeat psimp) ; auto.
+Qed.
+
+Lemma modrm_mm_inv_left x s s0 : 
+  in_grammar modrm_mm x (s,s0) -> no_sse_imm_op s = true.
+Proof.
+  unfold modrm_mm. unfold modrm_gen. intros.
+  repeat (repeat pinv ; repeat psimp) ; auto.
+Qed.
+
+Lemma modrm_mm_inv_right x s s0 : 
+  in_grammar modrm_mm x (s,s0) -> no_sse_imm_op s0 = true.
+Proof.
+  unfold modrm_mm. unfold modrm_gen. intros.
+  repeat (repeat pinv ; repeat psimp) ; auto.
+Qed.
+
+Lemma modrm_mm_noreg_inv_left x s1 s2 : 
+  in_grammar modrm_mm_noreg x (s1,s2) -> no_sse_imm_op s1 = true.
+Proof.
+  unfold modrm_mm_noreg. unfold modrm_gen_noreg. intros.
+  repeat (repeat pinv ; repeat psimp) ; auto.
+Qed.
+
+Lemma modrm_mm_noreg_inv_right x s1 s2 : 
+  in_grammar modrm_mm_noreg x (s1,s2) -> no_sse_imm_op s2 = true.
+Proof.
+  unfold modrm_mm_noreg. unfold modrm_gen_noreg. intros.
+  repeat (repeat pinv ; repeat psimp) ; auto.
+Qed.
+
+Lemma valid_instr_grammars_seg_override_non_cflow pre ins s : 
+  in_grammar (alts (List.map
+                      (fun p => valid_prefix_grammar_seg_override $ p)
+                      valid_instr_grammars_seg_override)) s (pre, ins) -> 
+  non_cflow_instr pre ins = true.
+Proof.
+  unfold valid_instr_grammars_seg_override.
+  simpl ; intros pre ins s ; rewrite in_alts ; simpl ; intros.
+  Ltac unf2 := unfold AAA_p, AAD_p, AAM_p, AAS_p, CMP_p, BOUND_p, BSF_p, 
+               BSR_p, BSWAP_p, BT_p, CLC_p, CLD_p, CLI_p, CLTS_p, CMC_p, 
+               CPUID_p, DAA_p, DAS_p, HLT_p, IMUL_p, LAHF_p, LAR_p, LEA_p,
+               LEAVE_p, LGS_p, MOV_p, MOVCR_p, MOVDR_p, MOVSR_p, MOVBE_p,
+               POP_p, POPA_p, POPF_p, PUSH_p, PUSHSR_p, PUSHA_p, PUSHF_p,
+               RCL_p, RCR_p, RDPMC_p, RDTSC_p, RDTSCP_p, SAHF_p, SETcc_p,
+               SLDT_p, SMSW_p, STC_p, STD_p, STR_p, TEST_p, WBINVD_p, F2XM1_p,
+               FABS_p, FADD_p, FADDP_p, FBLD_p, FBSTP_p, FCHS_p, FCMOVcc_p, 
+               FCOM_p, FCOMP_p, FCOMPP_p, FCOMIP_p, FCOS_p, FDECSTP_p,
+               FDIV_p, FDIVP_p, FDIVR_p, FDIVRP_p, FFREE_p, FIADD_p, FICOM_p, 
+               FICOMP_p, FIDIV_p, FIDIVR_p, FILD_p, FIMUL_p, FINCSTP_p, 
+               FIST_p, FISTP_p, FISUB_p, FISUBR_p, FLD_p, FLD1_p, FLDCW_p, 
+               FLDENV_p, FLDL2E_p, FLDL2T_p, FLDLG2_p, FLDLN2_p, FLDPI_p, 
+               FLDZ_p, FMUL_p, FMULP_p, FNCLEX_p, FNINIT_p, FNOP_p, FNSAVE_p, 
+               FNSTCW_p, FNSTSW_p, FPATAN_p, FPREM_p, FPREM1_p, FPTAN_p, 
+               FRNDINT_p, FRSTOR_p, FSCALE_p, FSIN_p, FSINCOS_p, FSQRT_p, 
+               FST_p, FSTENV_p, FSTP_p, FSUB_p, FSUBP_p, FSUBR_p, FSUBRP_p,
+               FTST_p, FUCOM_p, FUCOMP_p, FUCOMPP_p, FUCOMI_p, FUCOMIP_p, 
+               FXAM_p, FXCH_p, FXTRACT_p, FYL2X_p, FYL2XP1_p, FWAIT_p, 
+               EMMS_p, MOVD_p, MOVQ_p, PACKSSDW_p, PACKSSWB_p, PACKUSWB_p, 
+               PADD_p, PADDS_p, PADDUS_p, PAND_p, PANDN_p, PCMPEQ_p, PCMPGT_p, 
+               PMADDWD_p, PMULHUW_p, PMULHW_p, PMULLW_p, POR_p, PSLL_p, PSRA_p, 
+               PSRL_p, PSUB_p, PSUBS_p, PSUBUS_p, PUNPCKH_p, PUNPCKL_p, PXOR_p, 
+               ADDPS_p, ADDSS_p, ANDNPS_p, ANDPS_p, CMPPS_p, CMPSS_p, COMISS_p, 
+               CVTPI2PS_p, CVTPS2PI_p, CVTSI2SS_p, CVTSS2SI_p, CVTTPS2PI_p, CVTTSS2SI_p,
+               DIVPS_p, DIVSS_p, LDMXCSR_p, MAXPS_p, MAXSS_p, MINPS_p, MINSS_p, 
+               MOVAPS_p, MOVHLPS_p, MOVLPS_p, MOVMSKPS_p, MOVSS_p, MOVUPS_p, MULPS_p,
+               MULSS_p, ORPS_p, RCPPS_p, RCPSS_p, RSQRTPS_p, RSQRTSS_p, SHUFPS_p, 
+               SQRTPS_p, SQRTSS_p, STMXCSR_p, SUBPS_p, SUBSS_p, UCOMISS_p, UNPCKHPS_p,
+               UNPCKLPS_p, XORPS_p, PAVGB_p, PEXTRW_p, PINSRW_p, PMAXSW_p, PMAXUB_p, 
+               PMINSW_p, PMINUB_p, PMOVMSKB_p, PSADBW_p, PSHUFW_p, MASKMOVQ_p,
+               MOVNTPS_p, MOVNTQ_p, PREFETCHT0_p, PREFETCHT1_p, PREFETCHT2_p, 
+               PREFETCHNTA_p, SFENCE_p,
+               logic_or_arith_p, bit_test_p, rotate_p in *.
+  Ltac m3 := 
+  try (repeat (simpl ; repeat psimp ; repeat pinv ; 
+    match goal with 
+    | [ H : match ?x with | Imm_op _ => _ | Reg_op _ => _ | Address_op _ => _ | Offset_op _ => _ end |- _ ] => destruct x ; try contradiction
+    | [ |- context[if ?x then _ else _]] => destruct x
+    | [ |- context[only_seg_or_op _]] => 
+      rewrite only_gs_seg_override_imp_only_seg_or_op ; auto
+    | [ H : in_grammar _ _ _ |- _ ] => 
+      rewrite (valid_prefix_grammar_seg_override_non_cflow H) ; auto
+    | [ H : in_grammar modrm_mmx _ _ |- context[no_mmx_imm_op _]] => 
+      rewrite (modrm_mx_inv_left H)
+    | [ H : in_grammar modrm_mmx _ _ |- context[no_mmx_imm_op _]] => 
+      rewrite (modrm_mx_inv_right H)
+    | [ H : in_grammar modrm_xmm _ _ |- _ ] => 
+      rewrite (modrm_xmm_inv_left H)
+    | [ H : in_grammar modrm_xmm _ _ |- _ ] => 
+      rewrite (modrm_xmm_inv_right H)
+    | [ H : in_grammar modrm_xmm_noreg _ _ |- _ ] => 
+      rewrite (modrm_xmm_noreg_inv_left H)
+    | [ H : in_grammar modrm_xmm_noreg _ _ |- _ ] => 
+      rewrite (modrm_xmm_noreg_inv_right H)
+    | [ H : in_grammar modrm_xmm_gp_noreg _ _ |- _ ] => 
+      rewrite (modrm_xmm_gp_noreg_inv H)
+    | [ H : in_grammar modrm_mm _ _ |- _ ] => 
+      rewrite (modrm_mm_inv_left H)
+    | [ H : in_grammar modrm_mm _ _ |- _ ] => 
+      rewrite (modrm_mm_inv_right H)
+    | [ H : in_grammar modrm_mm_noreg _ _ |- _ ] => 
+      rewrite (modrm_mm_noreg_inv_left H)
+    | [ H : in_grammar modrm_mm_noreg _ _ |- _ ] => 
+      rewrite (modrm_mm_noreg_inv_right H)
+    | _ => idtac ; auto
+  end)).
+  Ltac m2 := 
+    pinv ; pinv ; [ unf2 ; repeat pinv ; 
+                    match goal with 
+                      | [ H : (_,_) = (_,_) |- _ ] => 
+                        injection H ; clear H ; intros ; subst
+                    end ; m3 | idtac ].
+  repeat m2.
+  unfold modrm_gen_noreg, mmx_reg_op, mmx_reg in H1.  
+  repeat (repeat pinv ; repeat psimp) ; auto.
+  unfold modrm_gen_noreg, mmx_reg_op, mmx_reg in H1.
+  repeat (repeat pinv ; repeat psimp) ; auto. 
+  pinv.
+Qed.
+
+Lemma non_cflow_instr_inv (pre:prefix) (ins:instr) (s:list char_p) :
+  in_grammar non_cflow_grammar s (pre,ins) -> 
+  non_cflow_instr pre ins = true.
+Proof.
+    unfold non_cflow_grammar.  unfold non_cflow_grammar_list.
     intros. 
-    unfold valid_prefix_parser_opsize, only_op_override, op_override_p in *.
-    repeat pinv. simpl. unfold either_prefix. simpl. auto.
-  Qed.
-  generalize (opsize_prefix H1) ; clear H1 ; intros. destruct H.
-  unfold non_cflow_instrs_opsize_pre in *. simpl in *. repeat pinv.
-  (* ADC_p *)
-  log_or_arith ADC_p.
-  (* ADD_p *)
-  log_or_arith ADD_p.
-  (* AND_p *)
-  log_or_arith AND_p.
-  (* CMP_p *)
-  log_or_arith CMP_p.
-  (* OR_p *)
-  log_or_arith OR_p.
-  (* SBB_p *)
-  log_or_arith SBB_p.
-  (* SUB_p *)
-  log_or_arith SUB_p.
-  (* SHL_p *)
-  Lemma rotate2 : forall pfx x I s i, in_parser (rotate_p x I) s i -> 
-    only_op_override pfx = true ->
-    (forall b op ri, no_imm_op op = true -> non_cflow_instr pfx (I b op ri) = true) -> 
-    non_cflow_instr pfx i = true.
-  Proof.
-    unfold rotate_p. intros. repeat pinv ; repeat psimp ; repeat pinv ; 
-    repeat psimp ; eauto ; try (destruct x6 ; try contradiction ; eauto).
-    destruct x8 ; try contradiction ; eauto.
-  Qed.
-  Ltac rot2 c := unfold c in * ; eapply rotate2 ; eauto ; simpl ; intros ; auto.
-  rot2 SHL_p.
-  (* SHLD_p *)
-  Lemma shiftdouble2 : forall pfx x I s i, 
-    only_op_override pfx = true ->
-    in_parser (shiftdouble_p x I) s i -> 
-    (forall op r ri, no_imm_op op = true -> non_cflow_instr pfx (I op r ri) = true) -> 
-    non_cflow_instr pfx i = true.
-  Proof.
-    unfold shiftdouble_p, modrm_noreg. intros ; repeat pinv ; repeat psimp ; 
-    repeat pinv ; repeat psimp ; eauto ; repeat pinv ; repeat psimp ; 
-    unfold rm01, rm00, rm10 in * ; repeat pinv ; auto ; 
-    try (destruct x16 ; auto) ; try (destruct x14 ; auto).
-  Qed.
-  Ltac shdouble2 c := unfold c in * ; eapply shiftdouble2 ; eauto ; intros ; simpl ; auto.
-  shdouble2 SHLD_p.
-  (* SHR_p *)
-  rot2 SHR_p.
-  (* SAR_p *)
-  rot2 SAR_p.
-  (* SHRD_p *)
-  shdouble2 SHRD_p.
-  (* XOR_p *)
-  log_or_arith XOR_p.
-  (* IMUL_p *)
-  unop IMUL_p. destruct o0 ; auto. destruct o2 ; auto. destruct o2 ; auto.
-  (* MOV_p *)
-  unop MOV_p ; destruct o2 ; auto.
-  (* MOVSX_p *)
-  unop MOVSX_p ; destruct o2 ; auto.
-  (* MOVZX_p *)
-  unop MOVZX_p ; destruct o2 ; auto.
-  (* NEG_p *)
-  unop NEG_p.
-  (* NOT_p *)
-  unop NOT_p. 
-  (* DIV_p *)
-  unop DIV_p.
-  (* IDIV_p *)
-  unop IDIV_p.
-  (* TEST_p *)
-  unop TEST_p.
-  (* CDQ_p *)
-  punf CDQ_p.
-  (* CWDE_p *)
-  punf CWDE_p.
-  (* MUL_p *)
-  unop MUL_p.
-  (* XCHG_p *)
-  unop XCHG_p ; destruct o2 ; auto.
-  (* never *)
-  unfold never in * ; pinv.
-  (* other stuff *)
-  generalize (pfx_rep H1). clear H1.
-  simpl in H2. repeat pinv.
-  (* CMPS_p *)
-  punf CMPS_p.
-  (* MOVS_p *)
-  punf MOVS_p.
-  (* STOS_p *)
-  punf STOS_p.
-  unfold never in *. pinv.
+    Ltac iaa := 
+      match goal with
+        | [ H : in_grammar (alts (?A ++ ?B)) _ _ |- _ ] => 
+          generalize (in_app_alts _ _ H) ; clear H ; 
+          intro H ; destruct H ; [ idtac | iaa ]
+        | _ => idtac
+      end.
+    iaa.
+    eapply valid_instr_grammars_rep_non_cflow ; eauto.
+    eapply valid_instr_grammars_rep_or_repn_non_cflow ; eauto.
+    eapply valid_instr_grammars_lock_with_op_override_non_cflow ; eauto.
+    eapply valid_instr_grammars_lock_no_op_override_non_cflow ; eauto.
+    eapply valid_instr_grammars_seg_with_op_override_non_cflow ; eauto.
+    eapply valid_instr_grammars_seg_op_override_non_cflow ; eauto.
+    eapply valid_instr_grammars_seg_override_non_cflow ; eauto.
 Qed.
 
 Lemma byteLt256 : forall b:int8, (byte2token b < 256)%nat.
@@ -580,97 +693,326 @@ Proof.
 Qed.
 
 Lemma bytesLt256 : forall (bs:list int8), 
-  list_all (fun t => (t < 256)%nat) (List.map byte2token bs).
+  Parser.list_all (fun t => (t < 256)%nat) (List.map byte2token bs).
 Proof.
   induction bs ; auto ; simpl ; auto ; split ; auto. apply byteLt256. 
 Qed.
 
-Lemma in_map_alts t1 t2 (p1:parser t1) (ps:list (parser t2)) s v : 
-  in_parser (p1 $ (alts ps)) s v ->
-  in_parser (alts (List.map (fun p2 => p1 $ p2) ps)) s v .
+Lemma in_map_alts t1 t2 (p1:grammar t1) (ps:list (grammar t2)) s v : 
+  in_grammar (p1 $ (alts ps)) s v <->
+  in_grammar (alts (List.map (fun p2 => p1 $ p2) ps)) s v .
 Proof.
-  induction ps ; simpl ; intros ; repeat pinv. unfold never in *. pinv.
-  eapply Alt_left_pi. econstructor ; eauto. eapply Alt_right_pi. 
-  eapply IHps. econstructor ; eauto.
-Qed.
-
-(** The [valid_prefix_parser_nooverride] parser used in the DFA is a subset of the 
-    [prefix_parser_nooverride] parser used in the semantics. *)
-Lemma prefix_subset : 
-  forall s v, in_parser valid_prefix_parser_nooverride s v -> 
-    in_parser prefix_parser_nooverride s v.
-Proof.
-  unfold valid_prefix_parser_nooverride, prefix_parser_nooverride. intros.
-  repeat pinv. unfold option_perm2. econstructor. econstructor. 
-  econstructor. eauto. eauto. simpl. auto.
-  unfold option_perm2. econstructor.
-  eapply Alt_right_pi. eapply Alt_right_pi. econstructor. 
-  unfold segment_override_p. econstructor. repeat (eapply Alt_right_pi).
-  econstructor. eapply H0. eauto. eauto. simpl. auto.
+  intros. rewrite in_alts in *. split. intros. pinv. rewrite in_alts in H0.
+  generalize x x0 x1 x2 H H0 ; clear x x0 x1 x2 H H0. 
+  induction ps ; simpl in *; intros ; repeat pinv ; eauto. 
+  induction ps ; simpl ; intros ; repeat pinv. econstructor ; eauto.
+  rewrite in_alts. simpl. eauto. specialize (IHps H). pinv.
+  econstructor ; eauto. rewrite in_alts in *. simpl. eauto.
 Qed.
 
 Lemma mem_parser_subset : 
-  forall t (p:parser t) (ps:list (parser t)),
+  forall t (p:grammar t) (ps:list (grammar t)),
     In p ps -> 
-    forall s v, in_parser p s v -> in_parser (alts ps) s v.
+    forall s v, in_grammar p s v -> in_grammar (alts ps) s v.
 Proof.
-  induction ps ; simpl. intros. contradiction. intros.
-  destruct H ; subst. eapply Alt_left_pi ; auto. eapply Alt_right_pi ; auto.
+  induction ps ; simpl. intros. contradiction. intros. 
+  destruct H ; subst. rewrite in_alts. simpl ; eauto. 
+  rewrite in_alts. simpl. eapply in_alt_r. rewrite <- in_alts. eauto.
 Qed.
 
 Lemma alts_subset : 
-  forall t (ps qs:list (parser t)), 
+  forall t (ps qs:list (grammar t)), 
     (forall p, In p ps -> In p qs) -> 
-    forall s v, in_parser (alts ps) s v -> in_parser (alts qs) s v.
+    forall s v, in_grammar (alts ps) s v -> in_grammar (alts qs) s v.
 Proof.
-  induction ps. simpl. intros. unfold never in *. pinv. intros.
+  induction ps. simpl. intros. rewrite in_alts in *. unfold never in *. simpl in *. 
+  pinv. intros. rewrite in_alts in H0. 
   simpl in *. pinv. destruct H0. eapply mem_parser_subset. eapply (H a). auto. auto.
-  apply IHps. intros. eapply H. right. auto. auto.
+  apply IHps. intros. eapply H. right. auto. auto. rewrite in_alts ; auto.
 Qed.
 
-(** All parsers in [non_cflow_instrs_nosize_pre] are also in 
-    [instr_parsers_nosize_pre]. *)
-Lemma ncflow_is_subset : 
-  forall p, In p non_cflow_instrs_nosize_pre -> 
-    In p instr_parsers_nosize_pre.
+Lemma in_alts_exists t1 t2 (pre : grammar t1) s v (ps:list (grammar t2)) :
+  in_grammar (alts (List.map (fun p => pre $ p ) ps)) s v -> 
+  exists p, In p ps /\ in_grammar (pre $ p) s v.
 Proof.
-  Ltac pv H := repeat (try (left ; auto ; fail) ; right).
-  unfold non_cflow_instrs_nosize_pre, instr_parsers_nosize_pre. intros ; simpl in * ; 
-  repeat (destruct H ; [pv H | idtac]). contradiction.
+  intros. rewrite in_alts in H. generalize H ; clear H. 
+  induction ps ; simpl ; intros ; repeat pinv. exists a. eauto.
+  specialize (IHps H). destruct IHps as [p [H1 H2]].  eauto.
+Qed.
+
+Lemma alts_prefix_subset t1 t2 (pre1 pre2 : grammar t1) 
+      (ps qs:list (grammar t2)) :
+  (forall s v, in_grammar pre1 s v -> in_grammar pre2 s v) -> 
+  (forall p, In p ps -> In p qs) -> 
+  forall s v, in_grammar (alts (List.map (fun p => pre1 $ p) ps)) s v -> 
+              in_grammar (alts ((List.map (fun p => pre2 $ p) qs))) s v.
+Proof.
+  intros.  eapply in_map_alts. generalize (in_alts_exists _ _ H1). intros.
+  destruct H2 as [p [H2 H3]]. clear H1. assert (in_grammar (alts ((pre2 $ p)::nil)) s v).
+  pinv. rewrite in_alts. simpl. eauto. clear H3. eapply in_map_alts.
+  eapply alts_subset. Focus 2. eauto. simpl. intros. destruct H3 ; try contradiction.
+  subst. specialize (H0 _ H2). clear H2. generalize qs H0 ; clear qs H0 H s v H1.
+  induction qs ; simpl ; intros ; try contradiction. destruct H0. subst ; auto.
+  specialize (IHqs H). auto.
+Qed.
+
+Lemma in_perm2_1 t1 t2 (p1 p1' : grammar t1) (p2 : grammar t2) s v : 
+  (forall s v, in_grammar p1 s v -> in_grammar p1' s v) ->
+  in_grammar (perm2 p1 p2) s v -> in_grammar (perm2 p1' p2) s v.
+Proof.
+  unfold perm2. intros. repeat pinv. eauto. eapply in_alt_r. 
+  econstructor ; eauto.
+Qed.
+
+Lemma in_perm2_2 t1 t2 (p1: grammar t1) (p2 p2' : grammar t2) s v : 
+  (forall s v, in_grammar p2 s v -> in_grammar p2' s v) ->
+  in_grammar (perm2 p1 p2) s v -> in_grammar (perm2 p1 p2') s v.
+Proof.
+  unfold perm2. intros ; repeat pinv ; eauto. eapply in_alt_r.
+  econstructor ; eauto.
+Qed.
+
+Lemma in_perm3_1 t1 t2 t3 (p1 p1':grammar t1) (p2:grammar t2) (p3 : grammar t3) s v : 
+  (forall s v, in_grammar p1 s v -> in_grammar p1' s v) ->
+  in_grammar (perm3 p1 p2 p3) s v -> in_grammar (perm3 p1' p2 p3) s v.
+Proof.
+  unfold perm3. intros ; repeat pinv ; eauto. eapply in_alt_r.
+  eapply in_alt_l. econstructor ; eauto. econstructor ; eauto.
+  eapply in_perm2_1 ; eauto. eauto. eapply in_alt_r. eapply in_alt_r.
+  econstructor ; eauto. econstructor ; eauto. eapply in_perm2_1 ; eauto. eauto.
+Qed.
+
+Lemma in_perm3_2 t1 t2 t3 (p1:grammar t1) (p2 p2':grammar t2) (p3 : grammar t3) s v : 
+ (forall s v, in_grammar p2 s v -> in_grammar p2' s v) ->
+  in_grammar (perm3 p1 p2 p3) s v -> in_grammar (perm3 p1 p2' p3) s v.
+Proof.
+  unfold perm3. intros ; repeat pinv ; eauto. eapply in_alt_l. econstructor ; eauto.
+  eapply in_perm2_1 ; eauto. eapply in_alt_r.
+  eapply in_alt_l. econstructor ; eauto. 
+  eapply in_alt_r. eapply in_alt_r.
+  econstructor ; eauto. econstructor ; eauto. eapply in_perm2_2 ; eauto. eauto.
+Qed.
+
+Lemma in_perm3_3 t1 t2 t3 (p1:grammar t1) (p2:grammar t2) (p3 p3' : grammar t3) s v : 
+ (forall s v, in_grammar p3 s v -> in_grammar p3' s v) ->
+  in_grammar (perm3 p1 p2 p3) s v -> in_grammar (perm3 p1 p2 p3') s v.
+Proof.
+  unfold perm3. intros ; repeat pinv ; eauto. eapply in_alt_l. econstructor ; eauto.
+  eapply in_perm2_2 ; eauto. eapply in_alt_r.
+  eapply in_alt_l. econstructor ; eauto. econstructor ; eauto. eapply in_perm2_2 ; 
+  eauto. eauto. eapply in_alt_r. eapply in_alt_r.
+  econstructor ; eauto. 
+Qed.
+
+Lemma in_option_perm3_1 t1 t2 t3 (p1 p1':grammar (User_t t1)) (p2:grammar (User_t t2)) (p3 : grammar (User_t t3)) s v: 
+  (forall s v, in_grammar p1 s v -> in_grammar p1' s v) -> 
+  in_grammar (option_perm3 p1 p2 p3) s v -> 
+  in_grammar (option_perm3 p1' p2 p3) s v.
+Proof.
+  unfold option_perm3. intros. repeat 
+  match goal with 
+    | [ H : in_grammar (_ |+| _) _ _ |- in_grammar (_ |+| _) _ _ ] => 
+      pinv ; pinv ; [ eapply in_alt_l | eapply in_alt_r ]
+    | _ => idtac
+  end ; repeat pinv ; econstructor ; eauto. eapply in_perm2_1 ; eauto.
+  eapply in_perm2_1 ; eauto. eapply in_perm3_1 ; eauto.
+Qed.
+
+Lemma in_option_perm3_2 t1 t2 t3 (p1:grammar (User_t t1)) (p2 p2':grammar (User_t t2)) (p3 : grammar (User_t t3)) s v: 
+  (forall s v, in_grammar p2 s v -> in_grammar p2' s v) -> 
+  in_grammar (option_perm3 p1 p2 p3) s v -> 
+  in_grammar (option_perm3 p1 p2' p3) s v.
+Proof.
+  unfold option_perm3. intros. repeat 
+  match goal with 
+    | [ H : in_grammar (_ |+| _) _ _ |- in_grammar (_ |+| _) _ _ ] => 
+      pinv ; pinv ; [ eapply in_alt_l | eapply in_alt_r ]
+    | _ => idtac
+  end ; repeat pinv ; econstructor ; eauto. eapply in_perm2_2 ; eauto.
+  eapply in_perm2_1 ; eauto. eapply in_perm3_2 ; eauto.
+Qed.
+
+Lemma in_option_perm3_3 t1 t2 t3 (p1:grammar (User_t t1)) (p2:grammar (User_t t2)) (p3 p3': grammar (User_t t3)) s v: 
+  (forall s v, in_grammar p3 s v -> in_grammar p3' s v) -> 
+  in_grammar (option_perm3 p1 p2 p3) s v -> 
+  in_grammar (option_perm3 p1 p2 p3') s v.
+Proof.
+  unfold option_perm3. intros. repeat 
+  match goal with 
+    | [ H : in_grammar (_ |+| _) _ _ |- in_grammar (_ |+| _) _ _ ] => 
+      pinv ; pinv ; [ eapply in_alt_l | eapply in_alt_r ]
+    | _ => idtac
+  end ; repeat pinv ; econstructor ; eauto. eapply in_perm2_2 ; eauto.
+  eapply in_perm2_2 ; eauto. eapply in_perm3_3 ; eauto.
+Qed.
+
+Lemma in_option_perm3_variation_2 t1 t2 t3 (p1:grammar (User_t t1)) (p2 p2':grammar (User_t t2)) (p3 : grammar (User_t t3)) s v : 
+  (forall s v, in_grammar p2 s v -> in_grammar p2' s v) -> 
+  in_grammar (option_perm3_variation p1 p2 p3) s v -> 
+  in_grammar (option_perm3_variation p1 p2' p3) s v.
+Proof.
+  unfold option_perm3_variation. intros. 
+  repeat match goal with 
+    | [ H : in_grammar (_ |+| _) _ _ |- in_grammar (_ |+| _) _ _ ] => 
+      pinv ; pinv ; [ eapply in_alt_l | eapply in_alt_r ]
+    | _ => idtac
+  end ; repeat pinv ; econstructor ; eauto. eapply in_perm2_1 ; eauto.
+  eapply in_perm3_2 ; eauto.
+Qed.                                           
+
+Lemma gs_seg_imp_seg s v : in_grammar gs_segment_override_p s v -> 
+                           in_grammar segment_override_p s v.
+Proof.
+  unfold gs_segment_override_p, segment_override_p. intros.
+  pinv. simpl in x. unfold bitsleft in H. pinv. pinv.
+  unfold bits in H. unfold bits in H0. simpl in *. 
+  repeat pinv. simpl. repeat apply in_alt_r. unfold bitsleft, bits.
+  simpl. repeat econstructor ; eauto.
+Qed.
+
+Lemma valid_prefix_grammar_rep_imp s v : 
+  in_grammar valid_prefix_grammar_rep s v -> in_grammar prefix_grammar_rep s v.
+Proof.
+  unfold valid_prefix_grammar_rep, prefix_grammar_rep. intros. pinv.
+  econstructor ; eauto. eapply in_option_perm3_2. Focus 2. eauto.
+  apply gs_seg_imp_seg.
+Qed.
+
+Lemma valid_instr_grammars_imp p :
+  In p valid_instr_grammars_rep -> In p instr_grammars_rep.
+Proof.
+  unfold valid_instr_grammars_rep, instr_grammars_rep. simpl.
+  intros. tauto.
+Qed.
+
+Lemma valid_prefix_grammar_rep_or_repn_imp s v : 
+  in_grammar valid_prefix_grammar_rep_or_repn s v -> 
+  in_grammar prefix_grammar_rep_or_repn s v.
+Proof.
+  unfold valid_prefix_grammar_rep_or_repn, prefix_grammar_rep_or_repn. 
+  intros. pinv. econstructor ; eauto. eapply in_option_perm3_2. Focus 2. eauto.
+  apply gs_seg_imp_seg.
+Qed.
+
+Lemma valid_prefix_grammar_lock_with_op_override_imp s v : 
+  in_grammar valid_prefix_grammar_lock_with_op_override s v -> 
+  in_grammar prefix_grammar_lock_with_op_override s v.
+Proof.
+  unfold valid_prefix_grammar_lock_with_op_override, 
+  prefix_grammar_lock_with_op_override.
+  intros. pinv. econstructor ; eauto. 
+  eapply in_option_perm3_variation_2. Focus 2. eauto.
+  apply gs_seg_imp_seg.
+Qed.
+
+Lemma valid_prefix_grammar_lock_no_op_override_imp s v : 
+  in_grammar valid_prefix_grammar_lock_no_op_override s v ->
+  in_grammar prefix_grammar_lock_no_op_override s v.
+Proof.
+  unfold valid_prefix_grammar_lock_no_op_override, 
+  prefix_grammar_lock_no_op_override. intros. pinv. econstructor ; eauto.
+  unfold option_perm2 in *. 
+  repeat match goal with 
+    | [ H : in_grammar (_ |+| _) _ _ |- in_grammar (_ |+| _) _ _ ] => 
+      pinv ; pinv ; [ eapply in_alt_l | eapply in_alt_r ]
+    | _ => idtac
+  end ; repeat pinv ; econstructor ; eauto. apply gs_seg_imp_seg ; auto.
+  eapply in_perm2_2. Focus 2. eauto. apply gs_seg_imp_seg ; auto.
+Qed.
+
+Lemma valid_prefix_grammar_seg_with_op_override_imp s v : 
+  in_grammar valid_prefix_grammar_seg_with_op_override s v ->
+  in_grammar prefix_grammar_seg_with_op_override s v.
+Proof.
+  unfold valid_prefix_grammar_seg_with_op_override, 
+  prefix_grammar_seg_with_op_override. intros ; pinv. 
+  econstructor ; eauto. unfold option_perm2_variation in *.
+  repeat match goal with 
+    | [ H : in_grammar (_ |+| _) _ _ |- in_grammar (_ |+| _) _ _ ] => 
+      pinv ; pinv ; [ eapply in_alt_l | eapply in_alt_r ]
+    | _ => idtac
+  end ; repeat pinv ; econstructor ; eauto. eapply in_perm2_1.
+  Focus 2. eauto. apply gs_seg_imp_seg ; auto.
+Qed.
+
+Lemma valid_prefix_grammar_seg_override_imp s v : 
+  in_grammar valid_prefix_grammar_seg_override s v -> 
+  in_grammar prefix_grammar_seg_override s v.
+Proof.
+  unfold valid_prefix_grammar_seg_override, 
+  prefix_grammar_seg_override. intros ; pinv ; econstructor ; eauto.
+  unfold option_perm in *. pinv ; pinv ; [apply in_alt_l | apply in_alt_r].
+  auto. pinv. econstructor ; eauto. apply gs_seg_imp_seg ; auto.
+Qed.
+
+Lemma valid_prefix_grammar_seg_op_override_imp s v : 
+  in_grammar valid_prefix_grammar_seg_op_override s v -> 
+  in_grammar prefix_grammar_seg_op_override s v.
+Proof.
+  unfold valid_prefix_grammar_seg_op_override, 
+  prefix_grammar_seg_op_override. intros ; pinv ; econstructor ; eauto.
+  unfold option_perm2 in *.
+  repeat match goal with 
+    | [ H : in_grammar (_ |+| _) _ _ |- in_grammar (_ |+| _) _ _ ] => 
+      pinv ; pinv ; [ eapply in_alt_l | eapply in_alt_r ]
+    | _ => idtac
+  end ; repeat pinv ; econstructor ; eauto. apply gs_seg_imp_seg ; auto.
+  eapply in_perm2_1. Focus 2. eauto. apply gs_seg_imp_seg ; auto.
+Qed.
+
+Lemma in_valid_instr_grammars_seg_override p : 
+  In p valid_instr_grammars_seg_override -> 
+  In p instr_grammars_seg_override.
+Proof.
+  unfold valid_instr_grammars_seg_override, instr_grammars_seg_override.
+  intros.
+  simpl in H. 
+  Ltac m42 := 
+  match goal with 
+    | [ H : ?x = ?p  \/ ?Q |- In ?p (?x :: _) ] => 
+      destruct H ; [left ; auto | right ; m42]
+    | [ H : _ = _ \/ _ |- _ ] => right ; m42
+    | [ H : False |- _ ] => contradiction 
+  end.
+  m42. 
+Qed.
+
+Lemma non_cflow_grammar_list_subset s v : 
+  in_grammar (alts non_cflow_grammar_list) s v -> 
+  in_grammar (alts instruction_grammar_list) s v.
+Proof.
+  unfold non_cflow_grammar_list. unfold instruction_grammar_list. intros.
+  repeat
+  match goal with 
+    | [ H : in_grammar (alts (_ ++ _)) _ _ |- _] => 
+      generalize (in_app_alts _ _ H) ; clear H ; intro H ; eapply in_alts_app ; 
+      destruct H ; [ left | right ]
+    | _ => idtac
+  end ; 
+  match goal with 
+    | [ H : in_grammar (alts (List.map (fun _ => ?pre1 $ _) ?ps1)) _ _
+        |- in_grammar (alts (List.map (fun _ => ?pre2 $ _) ?ps2)) _ _ ] => 
+      apply (@alts_prefix_subset _ _ pre1 pre2 ps1 ps2) ; intros ; auto
+  end.
+  apply valid_prefix_grammar_rep_imp ; auto.
+  apply valid_instr_grammars_imp ; auto.
+  apply valid_prefix_grammar_rep_or_repn_imp ; auto.
+  apply valid_prefix_grammar_lock_with_op_override_imp ; auto.
+  apply valid_prefix_grammar_lock_no_op_override_imp ; auto.
+  apply valid_prefix_grammar_seg_with_op_override_imp ; auto.
+  apply valid_prefix_grammar_seg_op_override_imp ; auto.
+  apply valid_prefix_grammar_seg_override_imp ; auto.
+  apply in_valid_instr_grammars_seg_override ; auto.
 Qed.
 
 (** This shows that if a string matches the [non_cflow_parser], then it 
     will also match the [instruction_parser].  It's half of what we need
     to establish the correctness of the [non_cflow] DFA. *)
 Lemma non_cflow_parser_subset : 
-  forall s v, in_parser non_cflow_parser s v -> 
-    in_parser instruction_parser s v.
+  forall s v, in_grammar non_cflow_grammar s v -> 
+    in_grammar instruction_grammar s v.
 Proof.
-  unfold non_cflow_parser, instruction_parser.
-  unfold non_cflow_parser_list, instruction_parser_list.
-  intros. generalize (in_app_alts _ _ H). clear H. intro. 
-  destruct H ; [idtac | generalize (in_app_alts _ _ H) ; clear H ; intro H ; destruct H];
-  generalize (in_alts_map _ _ H) ; clear H ; intro ; apply in_alts_app.
-  left. pinv. eapply in_map_alts. 
-  eapply (fun H1 H2 => @Cat_pi _ _ _ _ (x ++ x0) (x1,x2) x x0 x1 x2 H1 H2 (eq_refl _)
-    (eq_refl _)). apply prefix_subset. auto. eapply alts_subset. eapply ncflow_is_subset.
-  auto.
-  right. pinv. eapply in_map_alts.
-  eapply (fun H1 H2 => @Cat_pi _ _ _ _ (x ++ x0) (x1,x2) x x0 x1 x2 H1 H2 (eq_refl _)
-    (eq_refl _)) ; auto. clear H2. unfold valid_prefix_parser_opsize in *.
-  pinv. unfold prefix_parser_opsize. econstructor. econstructor. eauto. auto.
-  pinv. left. eapply in_map_alts.
-  eapply (fun H1 H2 => @Cat_pi _ _ _ _ (x ++ x0) (x1,x2) x x0 x1 x2 H1 H2 (eq_refl _)
-    (eq_refl _)). clear H2. unfold valid_prefix_parser_rep, prefix_parser_nooverride
-  in * ; repeat pinv ; unfold option_perm2. repeat econstructor.
-  econstructor. eapply Alt_right_pi. econstructor. unfold lock_or_rep_p.
-  unfold bitsleft in *. econstructor. pinv. pinv. econstructor. econstructor.
-  eauto. repeat eapply Alt_right_pi. econstructor. eauto. eauto. auto. eauto.
-  simpl. eauto. eauto. simpl. auto. apply (alts_subset non_cflow_instrs_rep_pre) ; 
-  auto. clear H1 H2 x1 x0 x x2. unfold non_cflow_instrs_rep_pre in *. 
-  unfold instr_parsers_nosize_pre. simpl. intros. 
-  repeat (destruct H ; [ repeat (try (left ; auto ; fail) ; right) | idtac ]).
-  contradiction.
+  apply non_cflow_grammar_list_subset.
 Qed.
   
 Definition nat_to_byte(n:nat) : int8 := Word.repr (Z_of_nat n).
@@ -693,7 +1035,7 @@ Proof.
 Qed.
 
 Lemma explode_bits xs : 
-  list_all (fun n => (n < 256)%nat) xs -> 
+  Parser.list_all (fun n => (n < 256)%nat) xs -> 
   flat_map byte_explode (List.map nat_to_byte xs) = flat_map nat2bools xs.
 Proof.
   induction xs. auto. intros. simpl in H. destruct H.
@@ -706,25 +1048,33 @@ Proof.
   unfold nat2bools. unfold byte_explode.
   replace (Z_of_nat a) with (Word.unsigned (nat_to_byte a)). auto.
   unfold nat_to_byte. simpl. rewrite Zmod_small ; auto. 
-  assert (Z_of_nat a < Z_of_nat 256). apply inj_lt ; auto.
+  assert (Z_of_nat a < Z_of_nat 256)%Z. apply inj_lt ; auto.
   split.
   apply Zle_0_nat. auto.
 Qed.
 
+Require Import Recognizer.
+
 (** These abstraction shananigans are necessary to keep Coq from
-    trying to actually build the DFA from within Coq. *)
-Module Type ABSTRACT_MAKE_DFA_SIG.
-  Parameter abstract_build_dfa : 
-    nat -> (token_id -> list char_p) -> nat -> regexp unit_t -> option DFA.
-  Parameter build_dfa_eq : abstract_build_dfa = build_dfa.
-End ABSTRACT_MAKE_DFA_SIG.
+    trying to actually build the recognizer from within Coq. *)
+Module Type ABSTRACT_MAKE_RECOGNIZER_SIG.
+  Parameter abstract_make_recognizer : 
+    forall t, grammar t -> option Recognizer.DFA.
+  Parameter make_recognizer_eq : abstract_make_recognizer = make_recognizer.
+End ABSTRACT_MAKE_RECOGNIZER_SIG.
 
-Module ABSTRACT_MAKE_DFA : ABSTRACT_MAKE_DFA_SIG.
-  Definition abstract_build_dfa := build_dfa.
-  Definition build_dfa_eq := eq_refl build_dfa.
-End ABSTRACT_MAKE_DFA.
+Module ABSTRACT_MAKE_RECOGNIZER : ABSTRACT_MAKE_RECOGNIZER_SIG.
+  Definition abstract_make_recognizer := make_recognizer.
+  Definition make_recognizer_eq := eq_refl make_recognizer.
+End ABSTRACT_MAKE_RECOGNIZER.
 
-Import ABSTRACT_MAKE_DFA.
+Import ABSTRACT_MAKE_RECOGNIZER.
+
+Lemma list_all_eq A (xs:list A) (P : A -> Prop) : 
+  list_all P xs <-> Parser.list_all P xs.
+Proof.
+  induction xs ; simpl ; mysimp ; intros ; mysimp ; apply IHxs ; auto.
+Qed.
 
 (** This lemma tells that that the DFA build from the [non_cflow_parser],
     when run on an input string of bytes [bytes] and produces [Some(n,nats2)],
@@ -733,44 +1083,81 @@ Import ABSTRACT_MAKE_DFA.
     [bytes1] and produce the same value.  Furthermore, there is no smaller
     prefix of [bytes] that the [non_cflow_parser] will accept. Also,
 *)
+Opaque non_cflow_grammar.
 Lemma non_cflow_dfa_corr1 :
   forall (d:DFA), 
-    abstract_build_dfa 256 nat2bools 400 (par2rec non_cflow_parser) = Some d -> 
+    abstract_make_recognizer non_cflow_grammar = Some d -> 
     forall (bytes:list int8) (n:nat) (nats2:list nat),
-      dfa_recognize 256 d (List.map byte2token bytes) = Some (n, nats2) -> 
+      dfa_recognize d (List.map byte2token bytes) = Some (n, nats2) -> 
       exists bytes1, exists pfx:prefix, exists ins:instr, 
-        in_parser non_cflow_parser (flat_map byte_explode bytes1) (pfx,ins) /\ 
-        in_parser instruction_parser (flat_map byte_explode bytes1) (pfx,ins) /\ 
+        in_grammar non_cflow_grammar (flat_map byte_explode bytes1) (pfx,ins) /\ 
+        in_grammar instruction_grammar (flat_map byte_explode bytes1) (pfx,ins) /\ 
         n = length bytes1 /\ 
         bytes = bytes1 ++ (List.map nat_to_byte nats2) /\ 
         non_cflow_instr pfx ins = true /\
         (forall ts3 ts4,
           (length ts3 < length bytes1)%nat -> 
           bytes = ts3 ++ ts4 -> 
-          forall v0, ~ in_parser non_cflow_parser (flat_map byte_explode ts3) v0).
+          forall v0, ~ in_grammar non_cflow_grammar (flat_map byte_explode ts3) v0).
 Proof.
-  intros. subst. rewrite build_dfa_eq in H.
-  generalize (dfa_recognize_corr _ _ _ _ H (List.map byte2token bytes) 
-  (bytesLt256 _)). clear H. rewrite H0. clear H0. mysimp. destruct x0. 
+  intros. subst. rewrite make_recognizer_eq in H. unfold make_recognizer in H.
+  assert (TLT:list_all (fun t => t < num_tokens) (List.map byte2token bytes)).
+  rewrite list_all_eq. apply bytesLt256.
+  generalize 
+    (@dfa_recognize_corr _ non_cflow_grammar 400 d H (List.map byte2token bytes) TLT).
+  clear H. rewrite H0. clear H0. mysimp. destruct x0. 
   exists (List.map nat_to_byte x). exists p. exists i. 
   assert (List.map nat_to_byte (x ++ nats2) = bytes).
   rewrite <- H. apply n2bs. rewrite map_app in H3. rewrite <- H3.
   rewrite map_length. generalize (non_cflow_instr_inv H1). 
   assert (list_all (fun n => n < 256)%nat (x ++ nats2)).
-  rewrite <- H. apply (bytesLt256 bytes). generalize (list_all_app _ _ _ H4).
+  rewrite <- H. rewrite list_all_eq.
+  apply (bytesLt256 bytes). 
+  generalize (list_all_app _ _ _ H4).
   intros. destruct H5. 
   assert (flat_map byte_explode (List.map nat_to_byte x) = flat_map nat2bools x).
-  apply explode_bits. auto. rewrite H8. mysimp.
-  apply non_cflow_parser_subset. auto. intros.
+  apply explode_bits. rewrite <- list_all_eq. auto. rewrite H8.
+  assert (flat_map nat2bools x = flat_map token_id_to_chars x).
+  generalize x H5. induction x0. simpl. auto. intros.
+  replace (flat_map nat2bools (a::x0)) with ((nat2bools a) ++ (flat_map nat2bools x0)) ; 
+    auto. replace (flat_map token_id_to_chars (a :: x0)) with 
+          ((token_id_to_chars a) ++ (flat_map token_id_to_chars x0)) ; auto. 
+  destruct H9. rewrite (IHx0 H10). 
+  replace (nat2bools a) with (token_id_to_chars a) ; auto.
+  unfold token_id_to_chars. unfold nat2bools. unfold nat_explode. unfold byte_explode. 
+  assert (Word.unsigned (int8_of_nat a) = Z.of_nat a).
+  rewrite Word.unsigned_repr. auto. 
+  split. apply Zle_0_nat. unfold Word.max_unsigned. simpl. 
+  omega. rewrite H11. auto. rewrite H9. split. auto. split.
+  apply non_cflow_parser_subset. auto. split. auto. split. auto. split. auto. intros.
   specialize (H2 (List.map byte2token ts3) (List.map byte2token ts4)).
-  repeat rewrite map_length in H2. specialize (H2 H9).
-  rewrite <- map_app in H10. rewrite <- H in H10.
-  rewrite <- map_app in H2. rewrite <- H10 in H2. rewrite n2bs in H2. 
+  repeat rewrite map_length in H2. specialize (H2 H10).
+  rewrite <- map_app in H11. rewrite <- H in H11.
+  rewrite <- map_app in H2. rewrite <- H11 in H2. rewrite n2bs in H2. 
   specialize (H2 (eq_refl _)). intro. specialize (H2 v0). apply H2.
   assert (flat_map nat2bools (List.map byte2token ts3) = flat_map byte_explode ts3).
   rewrite <- explode_bits. rewrite n2bs. auto. apply (bytesLt256 ts3).
-  rewrite <- H12 in H11.  auto.
-Qed.
+  rewrite <- H13 in H12. 
+  assert (forall x, flat_map token_id_to_chars (List.map byte2token x) = 
+                    flat_map nat2bools (List.map byte2token x)).
+  induction x0. auto. replace (flat_map token_id_to_chars (List.map byte2token (a::x0)))
+  with ((token_id_to_chars (byte2token a)) ++ (flat_map token_id_to_chars (List.map byte2token x0))) ; auto.
+  replace (flat_map nat2bools (List.map byte2token (a::x0))) with
+  ((nat2bools (byte2token a)) ++ (flat_map nat2bools (List.map byte2token x0))) ; auto.
+  rewrite IHx0. replace (token_id_to_chars (byte2token a)) with (nat2bools (byte2token a)); auto.
+  unfold nat2bools, token_id_to_chars. unfold nat_explode. unfold byte_explode.
+  assert (Z.of_nat (byte2token a) = Word.unsigned (int8_of_nat (byte2token a))).
+  unfold byte2token. rewrite Zabs2Nat.id_abs.
+  rewrite Word.unsigned_repr. auto. unfold Word.unsigned. destruct a. simpl.
+  split. destruct intrange. unfold Z.abs. destruct intval ; auto. 
+  assert False. unfold Z.le in H14. unfold Z.compare in H14.
+  apply H14 ; auto. contradiction. unfold Word.max_unsigned. simpl.
+  assert ((Word.modulus 7 = 256)%Z). auto. rewrite H14 in intrange.
+  destruct intrange. destruct intval ; simpl ; auto. omega. omega. 
+  assert False. unfold Z.le in H15. unfold Z.compare in H15. apply H15. auto.
+  contradiction. rewrite <- H14. auto.
+  rewrite H14. auto.
+Qed. 
 
 (** In what follows, we need to prove that if the instruction parser
     accepts a string [s] and produces a value [v], then [v] is the 
@@ -790,25 +1177,27 @@ Qed.
 (** Simple determ holds when a parser doesn't contain [Star_p] nor any 
     [Alt_p].  We can show that these parsers produce at most one value
     (i.e., are deterministic.)  *)
-Fixpoint simple_determ t (p:parser t) : bool := 
+Fixpoint simple_determ t (p:grammar t) : bool := 
   match p with 
-    | Any_p => true
-    | Char_p _ => true
-    | Eps_p => true
-    | Zero_p _ => true
-    | Cat_p t1 t2 p1 p2 => simple_determ p1 && simple_determ p2
-    | Map_p t1 t2 f p => simple_determ p
+    | Any => true
+    | Char _ => true
+    | Eps => true
+    | Zero _ => true
+    | Cat t1 t2 p1 p2 => simple_determ p1 && simple_determ p2
+    | Map t1 t2 f p => simple_determ p
+    | Xform t1 t2 f p => simple_determ p
     | _ => false
   end.
 
-(** [simple_determ] implies a parser only accepts strings of the same size. *)
-Lemma simple_determ_same_size : forall t (p:parser t), simple_determ p = true ->
+(** [simple_determ] implies a grammar only accepts strings of the same size. *)
+Lemma simple_determ_same_size : forall t (p:grammar t), simple_determ p = true ->
   forall s1 v1 s2 v2, 
-    in_parser p s1 v1 -> 
-    in_parser p s2 v2 -> length s1 = length s2.
+    in_grammar p s1 v1 -> 
+    in_grammar p s2 v2 -> length s1 = length s2.
 Proof.
   induction p ; simpl ; intros ; try congruence ; repeat pinv ; auto.
-  repeat rewrite app_length. congruence. apply (IHp H _ _ _ _ H1 H2).
+  repeat rewrite app_length. congruence. 
+  apply (IHp H s1 x0 s2 x H0 H1).   apply (IHp H s1 x1 s2 x0 H0 H1).
 Qed. 
 
 Lemma app_inj_length : forall A (x1 x2 y1 y2:list A), 
@@ -822,125 +1211,174 @@ Proof.
   destruct IHx1. subst. auto.
 Qed.
   
-(** [simple_determ] implies a parser is deterministic. *)
-Lemma simple_determ_corr : forall t (p:parser t), 
+(** [simple_determ] implies a grammar is deterministic. *)
+Lemma simple_determ_corr : forall t (p:grammar t), 
   simple_determ p = true -> 
   forall s v1 v2,
-    in_parser p s v1 -> in_parser p s v2 -> v1 = v2.
+    in_grammar p s v1 -> in_grammar p s v2 -> v1 = v2.
 Proof.
   induction p ; simpl ; intros ; try congruence ; repeat pinv ; auto.
-  generalize (simple_determ_same_size Heqx7 H3 H2).
-  generalize (simple_determ_same_size Heqy H4 H5). intros.
-  generalize (app_inj_length _ _ _ _ H1 H H0). intros. destruct H6 ; subst.
-  specialize (IHp1 _ _ _ H2 H3). specialize (IHp2 _ _ _ H5 H4). subst. auto.
-  specialize (IHp H _ _ _ H2 H1). subst. auto.
+  generalize (simple_determ_same_size Heqx7 H0 H1).
+  generalize (simple_determ_same_size Heqy H3 H2). intros.
+  generalize (app_inj_length _ _ _ _ H5 H (eq_sym H4)). intros. destruct H6 ; subst.
+  rewrite (IHp1 _ _ _ H1 H0). rewrite (IHp2 _ _ _ H2 H3). auto.
+  rewrite (IHp H _ _ _ H1 H0). auto. rewrite (IHp H _ _ _ H1 H0) ; auto.
 Qed.
 
 (** We are going to calculate the DNF for the prefixes.  But we can only
-    do this for parsers that don't contain [Star_p]. *)
-Fixpoint star_free t (p:parser t) : bool := 
+    do this for grammars that don't contain [Star_p]. *)
+Fixpoint star_free t (p:grammar t) : bool := 
   match p with 
-    | Star_p _ _ => false
-    | Cat_p t1 t2 p1 p2 => star_free p1 && star_free p2
-    | Alt_p t p1 p2 => star_free p1 && star_free p2
-    | Map_p t1 t2 f p' => star_free p'
+    | Star _ _ => false
+    | Cat t1 t2 p1 p2 => star_free p1 && star_free p2
+    | Alt t1 t2 p1 p2 => star_free p1 && star_free p2
+    | Map t1 t2 f p' => star_free p'
+    | Xform t1 t2 f p' => star_free p'
     | _ => true
   end.
 
-(** Disjunctive normal-form for parsers.  This is not well-defined when 
-    the parser includes [Star_p]. *)
-Fixpoint dnf t (p:parser t) : list (parser t) := 
-  match p with 
-    | Alt_p t p1 p2 => (dnf p1) ++ (dnf p2)
-    | Cat_p t1 t2 p1 p2 => 
-      flat_map (fun d1 => List.map (fun d2 => Cat_p d1 d2) (dnf p2)) (dnf p1)
-    | Map_p t1 t2 f p => List.map (fun d => @Map_p t1 t2 f d) (dnf p)
-    | p => p::nil
+(** Disjunctive normal-form for grammars.  This is not well-defined when 
+    the grammar includes [Star_p]. *)
+Fixpoint dnf t (p:grammar t) : list (grammar t) := 
+  match p in grammar t return list (grammar t) with 
+    | Alt t1 t2 p1 p2 => 
+      (List.map (fun p => @Map t1 (Sum_t t1 t2) (fun x => inl x) p) (dnf p1)) ++ 
+      (List.map (fun p => @Map t2 (Sum_t t1 t2) (fun x => inr x) p) (dnf p2))
+    | Cat t1 t2 p1 p2 => 
+      flat_map (fun d1 => List.map (fun d2 => Cat d1 d2) (dnf p2)) (dnf p1)
+    | Map t1 t2 f p => List.map (fun d => @Map t1 t2 f d) (dnf p)
+    | Xform t1 t2 f p => List.map (fun d => @Xform t1 t2 f d) (dnf p)
+    | p' => p'::nil
   end.
 
+Definition in_alts_g := in_alts.
 Require Import CheckDeterministic.
 
-(** Check that a parser is determinsistic -- blow it up into its disjunctive
+(** Check that a grammar is determinsistic -- blow it up into its disjunctive
     normal form, and use [check_all_p] to ensure that there is no string in
     common. *)
-Definition check_determ t (p:parser t) : bool := 
+Definition check_determ t (p:grammar t) : bool := 
   star_free p && check_all_p' 3 (dnf p).
 
-(** Check that a list of parsers is determinsitic. *)
-Fixpoint check_determ_ps t (ps:list (parser t)) : bool := 
+(** Check that a list of grammars is determinsitic. *)
+Fixpoint check_determ_ps t (ps:list (grammar t)) : bool := 
   match ps with 
     | nil => true
     | p::ps' => check_determ p && check_determ_ps ps'
   end.
 
-(** converting a parser to DNF is equivalent to the original parser *)
-Lemma dnf_corr1 t (p:parser t) s v : 
-  in_parser p s v -> 
-  in_parser (alts (dnf p)) s v.
+(** converting a grammar to DNF is equivalent to the original grammar *)
+Lemma dnf_corr1 t (p:grammar t) s v : 
+  in_grammar p s v -> 
+  in_grammar (alts (dnf p)) s v.
 Proof.
   induction 1 ; simpl ; intros ; subst ; try (econstructor ; eauto ; fail) ; 
     repeat
     match goal with 
       | [ H : _ && _ = true |- _ ] => generalize (andb_prop _ _ H) ; clear H ; t
       | [ H : ?x = true -> _, H1 : ?x = true |- _ ] => specialize (H H1)
-      | [ |- in_parser (alts (_ ++ _)) _ _ ] => eapply in_alts_app
+      | [ |- in_grammar (alts (_ ++ _)) _ _ ] => eapply in_alts_app
       | _ => auto
     end. 
-  generalize (dnf p1) (dnf p2) IHin_parser1 IHin_parser2. 
-  induction l ; simpl ; unfold never ; intros ; repeat pinv.  
-  eapply in_alts_app. left. induction l0 ; simpl in *; unfold never in *; intros ; 
-  repeat pinv. eapply Alt_left_pi. eauto. eapply Alt_right_pi. eauto.
-  eapply in_alts_app. right. auto.
-  generalize (dnf p) IHin_parser. induction l ; simpl ; unfold never ; intros ; 
-  repeat pinv. eapply Alt_left_pi ; eauto. eapply Alt_right_pi ; eauto.
+  generalize (dnf g1) (dnf g2) IHin_grammar1 IHin_grammar2. 
+  induction l ; simpl ; intros. rewrite in_alts_g in IHin_grammar0. simpl in *.
+  pinv. eapply in_alts_app. rewrite in_alts_g in IHin_grammar0. 
+  simpl in IHin_grammar0. pinv. destruct H1. left. 
+  apply in_map_alts. econstructor ; eauto. right. eapply IHl ; eauto.
+  rewrite in_alts_g. auto. left. generalize (dnf g1) IHin_grammar. 
+  induction l ; rewrite in_alts_g ; simpl ; intros.  pinv.
+  pinv. rewrite in_alts_g. simpl. destruct H0. eapply in_alt_l.
+  econstructor ; eauto. eapply in_alt_r. rewrite in_alts_g in IHl.
+  specialize (IHl H0). rewrite in_alts_g in IHl. auto.
+  right. generalize (dnf g2) IHin_grammar. induction l ; rewrite in_alts_g ; simpl ; 
+  intros ; pinv. rewrite in_alts_g ; simpl. destruct H0. eapply in_alt_l.
+  econstructor ; eauto. eapply in_alt_r. repeat rewrite in_alts_g in IHl.
+  apply (IHl H0). rewrite in_alts_g. simpl. eapply in_alt_l. eapply InStar_cons ; eauto. 
+  generalize (dnf g) IHin_grammar. induction l ; repeat rewrite in_alts_g. simpl.
+  intros ; pinv. simpl. intros ; pinv. destruct H0. apply in_alt_l. econstructor ; eauto.
+  eapply in_alt_r. repeat rewrite in_alts_g in IHl. eauto.
+  generalize (dnf g) IHin_grammar. induction l ; repeat rewrite in_alts_g. simpl.
+  intros ; pinv. simpl. intros ; pinv. destruct H0. apply in_alt_l. econstructor ; eauto.
+  eapply in_alt_r. repeat rewrite in_alts_g in IHl. eauto.
 Qed.
 
-Lemma dnf_corr2 t (p:parser t) s v :
-  in_parser (alts (dnf p)) s v -> 
+Lemma dnf_corr2 t (p:grammar t) s v :
+  in_grammar (alts (dnf p)) s v -> 
   star_free p = true -> 
-  in_parser p s v.
+  in_grammar p s v.
 Proof.
+  intros t p s v. rewrite in_alts_g. generalize s v ; clear s v.
   induction p ; simpl ; unfold never ; intros ; repeat pinv ; eauto.
   generalize (dnf p1) (dnf p2) IHp1 IHp2 H ; clear IHp1 IHp2 H Heqx Heqy.
-  induction l ; simpl ; unfold never in * ; intros ; repeat pinv.
-  generalize (in_app_alts _ _ H). clear H ; intros. destruct H.
+  induction l ; simpl ; unfold never in * ; intros ; simpl in * ; repeat pinv. 
+  rewrite <- in_alts_g in H. 
+  generalize (in_app_alts _ _ H). repeat rewrite in_alts_g. clear H ; intros. destruct H.
   clear IHl. induction l0 ; simpl in * ; unfold never in * ; pinv.
-  destruct H. pinv. econstructor. eapply IHp1 ; eauto. eapply Alt_left_pi. eauto.
-  eapply IHp2 ; eauto. eapply Alt_left_pi. eauto. auto. auto.
-  eapply IHl0. intros. eapply IHp2. eapply Alt_right_pi. eauto. auto. auto.
-  eapply IHl. intros. eapply IHp1. eapply Alt_right_pi ; eauto. auto. 
-  eapply IHp2. auto. generalize (in_app_alts _ _ H). intros. pinv ; eauto.
-  generalize (dnf p) IHp H ; clear IHp H. induction l ; simpl ; unfold never ; 
-  intros ; repeat pinv. econstructor. eapply IHp. eapply Alt_left_pi. eauto.
-  auto. auto. eapply IHl. intros. eapply IHp. eapply Alt_right_pi ; eauto. 
-  auto. auto.
+  destruct H. pinv. econstructor ; eauto. rewrite <- in_alts_g in *.
+  rewrite <- in_map_alts in H. pinv. econstructor ; eauto. eapply IHp2 ; auto.
+  eapply in_alt_r. apply in_alts_g ; auto. eapply IHl. intros. eapply IHp1 ; eauto.
+  eapply IHp2 ; eauto. auto. rewrite <- in_alts_g in H. generalize (in_app_alts _ _ H).
+  clear H ; intros. destruct H. 
+  assert (in_grammar (Map (Sum_t t1 t2) (fun x => inl x) (alts (dnf p1))) s v).
+  generalize (dnf p1) H. induction l ; simpl ; repeat rewrite in_alts_g ; simpl ; 
+  intros ; pinv. destruct H0. pinv. econstructor ; eauto. rewrite in_alts_g. simpl.
+  eapply in_alt_l. eauto. rewrite in_alts_g in IHl. specialize (IHl H0).
+  pinv. econstructor ; eauto. rewrite in_alts_g. simpl. eapply in_alt_r. 
+  rewrite in_alts_g in H1. auto. pinv. rewrite in_alts_g in H0.
+  specialize (IHp1 _ _ H0 (eq_refl _)). eauto.
+  assert (in_grammar (Map (Sum_t t1 t2) (fun x => inr x) (alts (dnf p2))) s v).
+  generalize (dnf p2) H ; induction l ; simpl ; repeat rewrite in_alts_g ; simpl ; 
+  intros ; pinv. destruct H0. pinv. econstructor ; eauto. rewrite in_alts_g ; simpl.
+  eapply in_alt_l ; eauto. rewrite in_alts_g in IHl. specialize (IHl H0).
+  pinv. econstructor ; eauto. rewrite in_alts_g. simpl. eapply in_alt_r ; eauto.
+  apply in_alts_g. auto. pinv. eapply InAlt_r ; eauto. eapply IHp2 ; auto.
+  eapply in_alts_g. eauto.
+  assert (in_grammar (Map t2 i (alts (dnf p))) s v). 
+  generalize (dnf p) H. induction l ; simpl ; intros ; pinv. destruct H1.
+  pinv. econstructor ; eauto. rewrite in_alts_g. eapply in_alt_l. eauto.
+  specialize (IHl H1). pinv. econstructor ; eauto. rewrite in_alts_g.
+  eapply in_alt_r. eapply in_alts_g. eauto. clear H. pinv.
+  rewrite in_alts_g in H. specialize (IHp _ _ H H0). econstructor ; eauto.
+  assert (in_grammar (Xform x (alts (dnf p))) s v).
+  generalize (dnf p) H. induction l ; simpl ; intros ; pinv. 
+  destruct H1. pinv. econstructor ; eauto. rewrite in_alts_g. eapply in_alt_l ; eauto.
+  specialize (IHl H1). clear H1. pinv. econstructor ; eauto. rewrite in_alts_g ; eapply
+  in_alt_r. apply in_alts_g. eauto. pinv. rewrite in_alts_g in H1.
+  specialize (IHp _ _ H1 H0). econstructor ; eauto.
 Qed.
 
-(** All of the parsers in [ps] are [simple_determ]. *)
-Fixpoint simple_determ_list t (ps:list (parser t)) : bool := 
+(** All of the grammars in [ps] are [simple_determ]. *)
+Fixpoint simple_determ_list t (ps:list (grammar t)) : bool := 
   match ps with 
     | nil => true
     | p::ps' => simple_determ p && simple_determ_list ps'
   end.
 
-Lemma simple_determ_app t (ps1 ps2:list (parser t)) : 
+Lemma simple_determ_app t (ps1 ps2:list (grammar t)) : 
   simple_determ_list (ps1 ++ ps2) = 
   simple_determ_list ps1 && simple_determ_list ps2.
 Proof.
   induction ps1 ; simpl ; auto. intros. destruct (simple_determ a) ; simpl ; auto.
 Qed.
 
-(** All of the parsers in [dnf p] are [simple_determ] *)
-Lemma dnf_determ t (p:parser t) : 
+(** All of the grammars in [dnf p] are [simple_determ] *)
+Lemma dnf_determ t (p:grammar t) : 
   star_free p = true -> simple_determ_list (dnf p) = true.
 Proof.
   induction p ; simpl ; intros ; subst ; simpl ; repeat pinv ; auto.
   generalize (dnf p1) (dnf p2) IHp1 IHp2 ; clear IHp1 IHp2.
   induction l ; simpl ; intros ; try contradiction ; repeat pinv ; auto.
-  rewrite simple_determ_app. rewrite IHl ; auto. apply simple_andb ; auto.
+  rewrite simple_determ_app. rewrite IHl ; auto. 
+  SearchAbout (_ && _). rewrite andb_true_r.
   clear IHl. induction l0 ; simpl ; auto. rewrite Heqx0. simpl in *.
   generalize (andb_prop _ _ IHp2). t. rewrite H. rewrite IHl0 ; auto.
-  rewrite simple_determ_app. rewrite IHp1. auto.
+  rewrite simple_determ_app. generalize (dnf p1) (dnf p2) IHp1 IHp2.
+  induction l ; simpl ; intros. induction l ; simpl in * ; auto.
+  generalize (andb_prop _ _ IHp3). t. rewrite H. simpl. rewrite IHl ; auto.
+  generalize (andb_prop _ _ IHp0) ; t. rewrite H. simpl. rewrite IHl ; auto.
+  specialize (IHp H). clear H. generalize (dnf p) IHp ; clear IHp.
+  induction l ; simpl ; auto ; t. generalize (andb_prop _ _ IHp). t.
+  rewrite H. rewrite IHl ; auto.
   specialize (IHp H). clear H. generalize (dnf p) IHp ; clear IHp.
   induction l ; simpl ; auto ; t. generalize (andb_prop _ _ IHp). t.
   rewrite H. rewrite IHl ; auto.
@@ -950,13 +1388,13 @@ Qed.
    denotation of [p], then there is no prefix of [s] in the domain of the 
    denotation of [p], and that there is at most one value associated with 
    [s] in the denotation of [p]. *)
-Lemma check_determ_corr' t (p:parser t) : 
+Lemma check_determ_corr' t (p:grammar t) : 
   check_determ p = true -> 
   forall s v,
-    in_parser p s v -> 
+    in_grammar p s v -> 
     (forall s1 s2 v', 
         s = s1 ++ s2 -> 
-        in_parser p s1 v' -> s2 = nil /\ v' = v).
+        in_grammar p s1 v' -> s2 = nil /\ v' = v).
 Proof.
   unfold check_determ. intros. generalize (andb_prop _ _ H) ; clear H ; t.
   generalize (dnf_corr1 H0). intros. subst. 
@@ -976,42 +1414,60 @@ Proof.
   contradiction. 
   injection H0 ; injection H2 ; clear H0 H2 ; intros ; subst. subst. clear IHl.
   simpl in *. assert False. apply H8. exists s2. exists v.
-  apply in_alts_comm'. eapply Alt_left_pi. auto. contradiction.
+  apply in_alts_comm'. rewrite in_alts_g. apply in_alt_l. auto. contradiction.
   injection H0 ; injection H2 ; clear H0 H2 ; intros ; subst. clear IHl. subst.
-  simpl in *. assert False. apply H8. exists s2. exists v. eapply Alt_left_pi. auto.
+  simpl in *. assert False. apply H8. exists s2. exists v. rewrite in_alts_g. 
+  eapply in_alt_l. auto.
   contradiction.
   injection H0 ; injection H2 ; clear H0 H2 ; intros ; subst.
   specialize (IHl x2 x3 x4 x x0 x1 H2 (eq_refl _) H7 H5). apply IHl ; clear IHl.
-  intro. apply H8. t. exists x5. exists x6. simpl. eapply Alt_right_pi. auto.
-  intro ; t. apply H6. exists x5. exists x6. simpl. eapply Alt_right_pi. auto.
+  intro. apply H8. t. exists x5. exists x6. simpl. 
+  rewrite in_alts_g. eapply in_alt_r. rewrite <- in_alts_g. auto.
+  intro ; t. apply H6. exists x5. exists x6. simpl. rewrite in_alts_g. 
+  eapply in_alt_r. rewrite <- in_alts_g. auto.
   simpl in H. generalize (andb_prop _ _ H). t ; auto.
 Qed.
 
-(** Check that all of the instruction parsers (without the prefixes) are 
+(** Check that all of the instruction grammars (without the prefixes) are 
     deterministic.  This runs fast enough that we can afford to do this. *)
-Lemma all_parsers_determ : 
-  check_determ_ps (instr_parsers_opsize_pre ++ instr_parsers_nosize_pre) = true.
+Lemma all_grammars_determ : 
+  check_determ_ps (
+      instr_grammars_rep ++
+      instr_grammars_rep_or_repn ++
+      instr_grammars_lock_with_op_override ++
+      instr_grammars_lock_no_op_override ++
+      instr_grammars_seg_with_op_override ++
+      instr_grammars_seg_op_override ++ 
+      instr_grammars_seg_override 
+  ) = true.
 Proof.
   vm_compute. auto.
 Qed.
 
-(** This checks that when we add a prefix to a parser, that the parser 
+(** This checks that when we add a prefix to a grammar, that the grammar 
     remains deterministic.  We do so by calculating the DNF of the 
-    prefix, and pre-pending each DNF term to the parser. *)
-Definition check_pfx t1 t2 (p1:parser t1) (p2:parser t2) := 
-  check_all_p' 3 (List.map (fun d1 => Cat_p d1 p2) (dnf p1)).
+    prefix, and pre-pending each DNF term to the grammar. *)
+Definition check_pfx t1 t2 (p1:grammar t1) (p2:grammar t2) := 
+  check_all_p' 3 (List.map (fun d1 => Cat d1 p2) (dnf p1)).
 
-Fixpoint check_all_pfx t1 t2 (p1:parser t1) (p2s:list (parser t2)) := 
+Fixpoint check_all_pfx t1 t2 (p1:grammar t1) (p2s:list (grammar t2)) := 
   match p2s with 
     | nil => true
     | p2::p2s' => check_pfx p1 p2 && check_all_pfx p1 p2s'
   end.
 
-(** Check that adding all of the prefixes to the parsers keeps them
+(** Check that adding all of the prefixes to the grammars keeps them
     deterministic. *)
 Lemma check_all_prefixed_instructions : 
-  (check_all_pfx prefix_parser_nooverride instr_parsers_nosize_pre) && 
-  (check_all_pfx prefix_parser_opsize instr_parsers_opsize_pre) = true.
+  (check_all_pfx prefix_grammar_rep instr_grammars_rep) && 
+  (check_all_pfx prefix_grammar_rep_or_repn instr_grammars_rep_or_repn) &&
+  (check_all_pfx prefix_grammar_lock_with_op_override 
+                 instr_grammars_lock_with_op_override) &&
+  (check_all_pfx prefix_grammar_lock_no_op_override instr_grammars_lock_no_op_override) &&
+  (check_all_pfx prefix_grammar_seg_with_op_override 
+                 instr_grammars_seg_with_op_override) &&
+  (check_all_pfx prefix_grammar_seg_op_override instr_grammars_seg_op_override) &&
+  (check_all_pfx prefix_grammar_seg_override instr_grammars_seg_override) = true.
 Proof.
   vm_compute. auto.
 Qed.
@@ -1027,35 +1483,36 @@ Proof.
 Qed.
 
 (** This shows that if a we add a [simple_determ] prefix to a deterministic
-    parser, then at most one value is associated with a string [s] in the
-    denotation of the compound parser, and furthermore, there is no prefix
+    grammar, then at most one value is associated with a string [s] in the
+    denotation of the compound grammar, and furthermore, there is no prefix
     of [s] that is in the denotation. This basically handles one of the
     alternatives of the DNF of a prefix. *)
-Lemma simple_pfx_determ' t1 t2 (p1:parser t1) (p2:parser t2) : 
+Lemma simple_pfx_determ' t1 t2 (p1:grammar t1) (p2:grammar t2) : 
   simple_determ p1 = true -> 
   check_determ p2 = true -> 
   forall s v1,
-    in_parser (Cat_p p1 p2) s v1 -> 
+    in_grammar (Cat p1 p2) s v1 -> 
     forall s1 s2 v2,
       s = s1 ++ s2 ->
-      in_parser (Cat_p p1 p2) s1 v2 -> 
+      in_grammar (Cat p1 p2) s1 v2 -> 
       s2 = nil /\ v1 = v2.
 Proof.
   intros. generalize (simple_determ_same_size H). intros. repeat pinv.
-  rewrite app_ass in H1.
-  generalize (inj_app_length _ _ _ _ H4 H1). t. subst.
-  generalize (simple_determ_corr H). intros. rewrite (H2 _ _ _ H3 H6).
+  rewrite app_ass in H6.
+  generalize (inj_app_length _ _ _ _ H4 H6). t. subst.
+  generalize (simple_determ_corr H). intros. rewrite (H7 _ _ _ H3 H1).
   generalize (check_determ_corr' H0). intros. 
-  specialize (H8 _ _ H5 x0 s2 _ (eq_refl _) H7). t ; subst. auto.
+  specialize (H8 _ _ H2 x0 s2 _ (eq_refl _) H5). t ; subst. auto.
 Qed.
 
-Lemma in_dnf_cat t1 t2 (p1:parser t1) (p2:parser t2) s v: 
-  in_parser (Cat_p p1 p2) s v -> 
-  in_parser (alts (List.map (fun d1 => Cat_p d1 p2) (dnf p1))) s v.
+Lemma in_dnf_cat t1 t2 (p1:grammar t1) (p2:grammar t2) s v: 
+  in_grammar (Cat p1 p2) s v -> 
+  in_grammar (alts (List.map (fun d1 => Cat d1 p2) (dnf p1))) s v.
 Proof.
-  intros. pinv. generalize (dnf_corr1 H1). generalize (dnf p1). induction l ; 
-  simpl ; unfold never ; intros ; repeat pinv. econstructor. econstructor ; eauto.
-  eapply Alt_right_pi. eauto.
+  intros. pinv. generalize (dnf_corr1 H). generalize (dnf p1). intro l.
+  rewrite in_alts_g. rewrite in_alts_g. induction l ; 
+  simpl ; intros ; repeat pinv. apply in_alt_l. econstructor ; eauto.
+  apply in_alt_r. eauto.
 Qed.
 
 Lemma list_map_eq_app : forall t1 t2 (f:t1->t2) (x:list t1) (a c:list t2) (b:t2),
@@ -1071,18 +1528,18 @@ Proof.
 Qed.
 
 (** Now show that if [p1] is a star-free prefix, and [p2] is a deterministic
-    parser, then adding [p1] to [p2] yields a parser that is deterministic,
+    grammar, then adding [p1] to [p2] yields a grammar that is deterministic,
     and furthermore, if [s] is in the domain of [p1 $ p2], then there is no
     prefix of [s] that is in the domain of [p1 $ p2]. *)
-Lemma check_pfx_determ' t1 t2 (p1:parser t1) (p2:parser t2) : 
+Lemma check_pfx_determ' t1 t2 (p1:grammar t1) (p2:grammar t2) : 
   star_free p1 = true ->
   check_determ p2 = true -> 
   check_pfx p1 p2 = true -> 
   forall s v1,
-    in_parser (Cat_p p1 p2) s v1 -> 
+    in_grammar (Cat p1 p2) s v1 -> 
     forall s1 s2 v2,
       s = s1 ++ s2 -> 
-      in_parser (Cat_p p1 p2) s1 v2 -> s2 = nil /\ v1 = v2.
+      in_grammar (Cat p1 p2) s1 v2 -> s2 = nil /\ v1 = v2.
 Proof.
   intros. generalize (in_dnf_cat H2). intros. generalize (in_dnf_cat H4). intros.
   clear H2 H4. 
@@ -1094,77 +1551,109 @@ Proof.
   generalize (dnf_determ _ H). intros. rewrite H5 in *. 
   rewrite (simple_determ_app) in H3. generalize (andb_prop _ _ H3) ; clear H3 ; t.
   simpl in H6. generalize (andb_prop _ _ H6). clear H6 ; t. 
-  generalize (inv_alt_pi H12). generalize (inv_alt_pi H11). clear H11 H12. intros. 
+  generalize (inv_alt H12). generalize (inv_alt H11). clear H11 H12. intros. 
   destruct H11 ; destruct H12 ; 
     try (eapply simple_pfx_determ' ; eauto) ;
       contradiction H10 ; exists s2 ; exists v1 ; auto.
 Qed.
 
 (** Show that the prefixes used in the semantics are star-free. *)
-Lemma star_free_prefix_parser_nooverride : 
-  star_free prefix_parser_nooverride = true.
+Lemma star_free_prefix_grammar_rep : 
+  star_free prefix_grammar_rep = true.
+Proof.
+  vm_compute ; auto.
+Qed.
+
+Lemma star_free_prefix_grammar_rep_or_repn : 
+  star_free prefix_grammar_rep_or_repn = true.
+Proof.
+  vm_compute ; auto.
+Qed.
+
+Lemma star_free_prefix_grammar_lock_with_op_override : 
+  star_free prefix_grammar_lock_with_op_override = true.
+Proof.
+  vm_compute ; auto.
+Qed.
+
+Lemma star_free_prefix_grammar_lock_no_op_override : 
+  star_free prefix_grammar_lock_no_op_override = true.
+Proof.
+  vm_compute ; auto.
+Qed.
+
+Lemma star_free_prefix_grammar_seg_with_op_override : 
+  star_free prefix_grammar_seg_with_op_override = true.
+Proof.
+  vm_compute ; auto.
+Qed.
+
+Lemma star_free_prefix_grammar_seg_op_override : 
+  star_free prefix_grammar_seg_op_override = true.
+Proof.
+  vm_compute ; auto.
+Qed.
+
+Lemma star_free_prefix_grammar_seg_override : 
+  star_free prefix_grammar_seg_override = true.
 Proof.
   vm_compute. auto.
 Qed.
 
-Lemma star_free_prefix_parser_opsize : 
-  star_free prefix_parser_opsize = true.
+Lemma and_parse2rexp t (p1:grammar t) (ps:list (grammar t)) s v1 v2: 
+  in_grammar p1 s v1 -> in_grammar (alts ps) s v2 -> 
+  in_rexp (OptAnd_r (grammar2rexp p1) (alts_r (List.map (@grammar2rexp _) ps))) s.
 Proof.
-  vm_compute. auto.
+  intros. apply opt_and_r_corr. econstructor. eapply grammar2rexp_corr1 ; eauto.
+  generalize ps H0. induction ps0. simpl. rewrite in_alts_g. simpl. intros. pinv.
+  rewrite in_alts_g. simpl. intros. pv_opt. pinv. destruct H1. econstructor. 
+  eapply grammar2rexp_corr1.
+  eauto. eapply Alt_right_ri. apply IHps0. apply in_alts_g ; auto.
 Qed.
 
-Lemma and_parse2rexp t (p1:parser t) (ps:list (parser t)) s v1 v2: 
-  in_parser p1 s v1 -> in_parser (alts ps) s v2 -> 
-  in_rexp (OptAnd_r (parser2rexp p1) (alts_r (List.map (@parser2rexp _) ps))) s.
-Proof.
-  intros. apply opt_and_r_corr. econstructor. eapply parse2rexp_corr1 ; eauto.
-  generalize ps H0. induction ps0. simpl. unfold never. intros. pinv.
-  simpl. intros. pv_opt. pinv. destruct H1. econstructor. eapply parse2rexp_corr1.
-  eauto. eapply Alt_right_ri. auto.
-Qed.
-
-(** An intermediate lemma that tells us that when all of the parsers
+(** An intermediate lemma that tells us that when all of the grammars
     in [p::ps] have been shown to be disjoint, then there is no 
     string in the domain of both [p] and [ps]. *)
-Lemma check_all_p'_tail t n (p:parser t) (ps:list (parser t)) : 
+Lemma check_all_p'_tail t n (p:grammar t) (ps:list (grammar t)) : 
   check_all_p' n (p::ps) = true -> 
   check_all_p' n ps = true /\ 
-  (forall s v1, in_parser p s v1 -> 
-    forall s1 s2 v2, s = s1++s2 -> ~ in_parser (alts ps) s1 v2) /\
-  (forall s v1, in_parser (alts ps) s v1 -> 
-    forall s1 s2 v2, s = s1++s2 -> ~ in_parser p s1 v2).
+  (forall s v1, in_grammar p s v1 -> 
+    forall s1 s2 v2, s = s1++s2 -> ~ in_grammar (alts ps) s1 v2) /\
+  (forall s v1, in_grammar (alts ps) s v1 -> 
+    forall s1 s2 v2, s = s1++s2 -> ~ in_grammar p s1 v2).
 Proof.
   intros. generalize (andb_prop _ _ H). t. split. auto. clear H0.
-  replace ((fix map (l:list(parser t)) : list rexp := 
-            match l with | nil => nil | a::t => parser2rexp a :: map t end) ps) with
-  (List.map (@parser2rexp t) ps) in H1 ; auto. clear H.
+  replace ((fix map (l:list(grammar t)) : list rexp := 
+            match l with | nil => nil | a::t => grammar2rexp a :: map t end) ps) with
+  (List.map (@grammar2rexp t) ps) in H1 ; auto. clear H.
   generalize (ckzeros_corr _ _ H1). intros. split ; intros ; intro ; subst.
   contradiction H. exists (s1 ++ s2). eapply opt_and_r_corr. econstructor.
   eapply opt_cat_r_corr. econstructor. eapply in_alts.  eauto.
   eapply star_any_all. eauto. eapply opt_cat_r_corr. econstructor.
-  eapply parse2rexp_corr1. eauto. eapply (star_any_all nil). 
+  eapply grammar2rexp_corr1. eauto. eapply (star_any_all nil). 
   rewrite <- app_nil_end. auto.
   contradiction H. exists (s1 ++ s2). eapply opt_and_r_corr. econstructor.
   eapply opt_cat_r_corr. econstructor. eapply in_alts. eauto.
   eapply (star_any_all nil). rewrite <- app_nil_end. eauto. 
-  eapply opt_cat_r_corr. econstructor. eapply parse2rexp_corr1. eauto. 
+  eapply opt_cat_r_corr. econstructor. eapply grammar2rexp_corr1. eauto. 
   eapply (star_any_all s2). auto.
 Qed.
 
-Lemma in_alts_map2 t1 t2 (ps:list (parser t1)) (p2:parser t2) s v :
-  in_parser (alts (List.map (fun p1 => Cat_p p1 p2) ps)) s v -> 
-  in_parser (Cat_p (alts ps) p2) s v.
+Lemma in_alts_map2 t1 t2 (ps:list (grammar t1)) (p2:grammar t2) s v :
+  in_grammar (alts (List.map (fun p1 => Cat p1 p2) ps)) s v -> 
+  in_grammar (Cat (alts ps) p2) s v.
 Proof.
-  induction ps ; simpl ; unfold never ; intros ; repeat pinv.
-  econstructor. econstructor. eauto. eauto. auto. auto.
-  specialize (IHps _ _ _ H). repeat pinv. econstructor. eapply Alt_right_pi. 
-  eauto. eauto. eauto. auto.
+  induction ps ; simpl ; intros ; rewrite in_alts_g in H ; simpl in H ; repeat pinv.
+  econstructor. rewrite in_alts_g. simpl. apply in_alt_l. eauto. eauto. auto. auto.
+  rewrite <- in_alts_g in H.
+  specialize (IHps _ _ _ H). repeat pinv. econstructor. rewrite in_alts_g. simpl.
+  apply in_alt_r. rewrite <- in_alts_g. eauto. eauto. auto. auto.
 Qed.
 
 (** More abstraction stuff to keep Coq from unwininding the definition 
     of [check_all_p]. *)
 Module Type ABSTRACT_CHECK_ALL_P_SIG.
-  Parameter abstract_check_all_p : nat -> forall t : result, list (parser t) -> bool.
+  Parameter abstract_check_all_p : nat -> forall t , list (grammar t) -> bool.
   Parameter abstract_check_all_p_eq : 
     abstract_check_all_p = check_all_p'.
 End ABSTRACT_CHECK_ALL_P_SIG.
@@ -1175,29 +1664,27 @@ Module ABSTRACT_CHECK_ALL_P : ABSTRACT_CHECK_ALL_P_SIG.
 End ABSTRACT_CHECK_ALL_P.
 
 Import ABSTRACT_CHECK_ALL_P.
-
-(** Make the [check_all_p] for the instructions used in the parser abstract. *)
+Transparent instruction_grammar_list.
+(** Make the [check_all_p] for the instructions used in the grammar abstract. *)
 Lemma abstract_check_all_p_instructions : 
-  abstract_check_all_p 3 
-  (List.map (fun p : parser instruction_t => prefix_parser_nooverride $ p)
-    instr_parsers_nosize_pre ++
-    List.map (fun p : parser instruction_t => prefix_parser_opsize $ p)
-    instr_parsers_opsize_pre) = true.
+  abstract_check_all_p 3 instruction_grammar_list = true.
 Proof.
+  unfold instruction_grammar_list.
   generalize all_instructions_check.
-  unfold instruction_parser_list.
+  unfold instruction_grammar_list.
   rewrite <- abstract_check_all_p_eq.
   auto.
 Qed.
 
-(** This lemma tells us that if we build a parser from two prefixes
-    and two lists of parsers, such that the prefixes are star-free,
-    and the parsers have been checked to be deterministic, and the
-    concatenation of the prefixes on the parsers don't have any strings
-    in common in their domain, then the resulting mongo parser 
+(*
+(** This lemma tells us that if we build a grammar from two prefixes
+    and two lists of grammars, such that the prefixes are star-free,
+    and the grammars have been checked to be deterministic, and the
+    concatenation of the prefixes on the grammars don't have any strings
+    in common in their domain, then the resulting mongo grammar 
     is deterministic and furthermore, when [s] and [v] are in its
     denotation, then there is no prefix of [s] in the denotation. *)
-Lemma parser_determ' t1 t2 m (pfx1 pfx2:parser t1) (ps1 ps2 :list (parser t2)) : 
+Lemma grammar_determ' t1 t2 m (pfx1 pfx2:grammar t1) (ps1 ps2 :list (grammar t2)) : 
   star_free pfx1 = true -> 
   star_free pfx2 = true -> 
   check_determ_ps ps1 = true -> 
@@ -1207,10 +1694,10 @@ Lemma parser_determ' t1 t2 m (pfx1 pfx2:parser t1) (ps1 ps2 :list (parser t2)) :
   check_all_pfx pfx1 ps1 = true -> 
   check_all_pfx pfx2 ps2 = true -> 
   forall s s1 s2 v1 v2,
-    in_parser (alts ((List.map (fun p => pfx1 $ p) ps1) ++ 
+    in_grammar (alts ((List.map (fun p => pfx1 $ p) ps1) ++ 
       (List.map (fun p => pfx2 $ p) ps2))) s v1 -> 
     s = s1 ++ s2 ->
-    in_parser (alts ((List.map (fun p => pfx1 $ p) ps1) ++ 
+    in_grammar (alts ((List.map (fun p => pfx1 $ p) ps1) ++ 
       (List.map (fun p => pfx2 $ p) ps2))) s1 v2 -> s2 = nil /\ v1 = v2.
 Proof.
   intros. rewrite abstract_check_all_p_eq in H3.
@@ -1227,13 +1714,17 @@ Proof.
   destruct x5 ; destruct x8 ; simpl in *; 
     injection H9 ; clear H9 ; injection H10 ; clear H10 ;
   intros ; subst. subst. auto. assert False. clear IHps0. subst.
-  contradiction H12. exists s2. exists v1. eapply Alt_left_pi ; auto. 
+  contradiction H12. exists s2. exists v1. rewrite in_alts_g.
+  apply in_alt_l. auto.
   contradiction. assert False ; clear IHps0 ; subst. contradiction H12.
-  exists s2. exists v1. eapply in_alts_comm'.  apply Alt_left_pi. auto.
+  exists s2. exists v1. eapply in_alts_comm'.  rewrite in_alts_g. 
+  apply in_alt_l. auto.
   contradiction. subst. assert (x8 = x5 /\ x6 = x9 /\ x7 = x10).
   eapply IHps0 ; clear IHps0 ; auto. intro. contradiction H14. t.
-  exists x11. exists x12. eapply Alt_right_pi ; auto.
-  intro ; t. eapply H12. exists x11 ; exists x12 ; eapply Alt_right_pi ; auto.
+  exists x11. exists x12. rewrite in_alts_g. apply in_alt_r. rewrite <- in_alts_g.
+  auto.
+  intro ; t. eapply H12. exists x11 ; exists x12. rewrite in_alts_g. 
+  apply in_alt_r. rewrite <- in_alts_g. auto. 
   t. subst. auto.
 
   t. subst. clear H3 H6 H9 H8. 
@@ -1256,44 +1747,209 @@ Proof.
   eapply check_pfx_determ'. eapply H. eapply H7. eauto. eauto. eauto. eauto.
   eapply check_pfx_determ'. eapply H0. eapply H7. eauto. eauto. eauto. eauto.
 Qed.
+*)
 
-Lemma check_determ_ps_app : forall t (ps1 ps2:list (parser t)), 
+Lemma check_determ_ps_app : forall t (ps1 ps2:list (grammar t)), 
   check_determ_ps (ps1 ++ ps2) = true -> 
   check_determ_ps ps1 = true /\ check_determ_ps ps2 = true.
 Proof.
   induction ps1. simpl. auto. simpl. intros. 
-  generalize (andb_prop _ _ H). t. generalize (IHps1 _ H1). t. auto.
+  generalize (andb_prop _ _ H). t. generalize (IHps1 _ H1). t. 
+  rewrite H0. rewrite H2. rewrite H3. auto.
 Qed.
 
-(** A key lemma:  This tells us that the [instruction_parser] is deterministic --
+Lemma in_check_determ_ps t x (ps:list (grammar t)) : 
+  In x ps -> check_determ_ps ps = true -> check_determ x = true.
+Proof.
+  induction ps ; simpl ; t. contradiction. generalize (andb_prop _ _ H0). t.
+  destruct H. subst ; auto. apply IHps ; auto.
+Qed.
+
+Lemma instr_grammars_determ x : 
+  (In x instr_grammars_rep \/
+  In x instr_grammars_rep_or_repn \/ 
+  In x instr_grammars_lock_with_op_override \/
+  In x instr_grammars_lock_no_op_override \/
+  In x  instr_grammars_seg_with_op_override \/
+  In x instr_grammars_seg_op_override \/
+  In x instr_grammars_seg_override) -> check_determ x = true.
+Proof.
+  intros. 
+  assert (In x (instr_grammars_rep ++
+  instr_grammars_rep_or_repn ++
+  instr_grammars_lock_with_op_override ++
+  instr_grammars_lock_no_op_override ++
+  instr_grammars_seg_with_op_override ++
+  instr_grammars_seg_op_override ++
+  instr_grammars_seg_override)). 
+  destruct H. apply in_app. auto. apply in_app ; right.
+  destruct H. apply in_app. auto. apply in_app ; right.
+  destruct H. apply in_app. auto. apply in_app ; right.
+  destruct H. apply in_app. auto. apply in_app ; right.
+  destruct H. apply in_app. auto. apply in_app ; right.
+  apply in_app ; auto.
+  apply (in_check_determ_ps _ _ H0). apply all_grammars_determ.
+Qed.
+
+Lemma in_check_all_pfx t1 t2 x (pre:grammar t1) (ps:list (grammar t2)) : 
+  In x ps -> check_all_pfx pre ps = true -> check_pfx pre x = true.
+Proof.
+  induction ps ; simpl ; t. contradiction. generalize (andb_prop _ _ H0). clear H0 ; t.
+  destruct H ; subst ; auto. 
+Qed.
+
+Lemma check_all_rep x : 
+  In x instr_grammars_rep -> check_pfx prefix_grammar_rep x = true.
+Proof.
+  intros. generalize (andb_prop _ _ check_all_prefixed_instructions). t. repeat 
+  match goal with 
+    | [ H : _  && _ = true |- _ ] => generalize (andb_prop _ _ H) ; clear H ; t
+  end.
+  apply (in_check_all_pfx _ _ _ H H0).
+Qed.
+
+Lemma check_all_rep_or_repn x : 
+  In x instr_grammars_rep_or_repn -> check_pfx prefix_grammar_rep_or_repn x = true.
+Proof.
+  intros. generalize (andb_prop _ _ check_all_prefixed_instructions). t. repeat 
+  match goal with 
+    | [ H : _  && _ = true |- _ ] => generalize (andb_prop _ _ H) ; clear H ; t
+  end.
+  apply (in_check_all_pfx _ _ _ H). auto.
+Qed.
+
+Lemma check_all_lock_with_op_override x : 
+  In x instr_grammars_lock_with_op_override -> 
+  check_pfx prefix_grammar_lock_with_op_override x = true.
+Proof.
+  intros. generalize (andb_prop _ _ check_all_prefixed_instructions). t. repeat 
+  match goal with 
+    | [ H : _  && _ = true |- _ ] => generalize (andb_prop _ _ H) ; clear H ; t
+  end.
+  apply (in_check_all_pfx _ _ _ H). auto.
+Qed.
+
+Lemma check_all_lock_no_op_override x : 
+  In x instr_grammars_lock_no_op_override -> 
+  check_pfx prefix_grammar_lock_no_op_override x = true.
+Proof.
+  intros. generalize (andb_prop _ _ check_all_prefixed_instructions). t. repeat 
+  match goal with 
+    | [ H : _  && _ = true |- _ ] => generalize (andb_prop _ _ H) ; clear H ; t
+  end.
+  apply (in_check_all_pfx _ _ _ H). auto.
+Qed.
+
+Lemma check_all_seg_with_op_override x : 
+  In x instr_grammars_seg_with_op_override -> 
+  check_pfx prefix_grammar_seg_with_op_override x = true.
+Proof.
+  intros. generalize (andb_prop _ _ check_all_prefixed_instructions). t. repeat 
+  match goal with 
+    | [ H : _  && _ = true |- _ ] => generalize (andb_prop _ _ H) ; clear H ; t
+  end.
+  apply (in_check_all_pfx _ _ _ H). auto.
+Qed.
+
+Lemma check_all_seg_op_override x : 
+  In x instr_grammars_seg_op_override -> 
+  check_pfx prefix_grammar_seg_op_override x = true.
+Proof.
+  intros. generalize (andb_prop _ _ check_all_prefixed_instructions). t. repeat 
+  match goal with 
+    | [ H : _  && _ = true |- _ ] => generalize (andb_prop _ _ H) ; clear H ; t
+  end.
+  apply (in_check_all_pfx _ _ _ H). auto.
+Qed.
+
+Lemma check_all_seg_override x : 
+  In x instr_grammars_seg_override -> 
+  check_pfx prefix_grammar_seg_override x = true.
+Proof.
+  intros. generalize (andb_prop _ _ check_all_prefixed_instructions). t. repeat 
+  match goal with 
+    | [ H : _  && _ = true |- _ ] => generalize (andb_prop _ _ H) ; clear H ; t
+  end.
+  apply (in_check_all_pfx _ _ _ H). auto.
+Qed.
+
+(** A key lemma:  This tells us that the [instruction_grammar] is deterministic --
     i.e., associates at most one value with a given string.  Furthermore, it tells
-    us that if the [instruction_parser] accepts a string [s], then there is no
+    us that if the [instruction_grammar] accepts a string [s], then there is no
     prefix of [s] that is accepted.  This is crucial for showing that a shortest-
-    match strategy (used by both the DFA and the derivative-based parserin the
+    match strategy (used by both the DFA and the derivative-based grammarin the
     semantics) is complete. *)
-Lemma parser_determ : 
+Lemma grammar_determ : 
   forall s v1, 
-    in_parser instruction_parser s v1 -> 
+    in_grammar instruction_grammar s v1 -> 
     forall s1 s2 v2, 
-      s = s1 ++ s2 -> in_parser instruction_parser s1 v2 -> 
+      s = s1 ++ s2 -> in_grammar instruction_grammar s1 v2 -> 
       s2 = nil /\ v1 = v2.
 Proof.
-  unfold instruction_parser. unfold instruction_parser_list.
-  generalize (check_determ_ps_app _ _ all_parsers_determ). t.
-  generalize (andb_prop _ _ check_all_prefixed_instructions). t.
-  intros. subst.
-  eapply (@parser_determ' prefix_t instruction_t 3 prefix_parser_nooverride 
-          prefix_parser_opsize _ _
-          star_free_prefix_parser_nooverride
-          star_free_prefix_parser_opsize
-          H3 H abstract_check_all_p_instructions H4 H5). 
-  eauto. eauto. eauto.
+  unfold instruction_grammar. (* unfold instruction_grammar_list. *)
+  generalize all_instructions_check. intro.
+  generalize (check_all_p'_corr 3 instruction_grammar_list H). clear H. intros. subst.
+  generalize (H _ _ H2). generalize (H _ _ H0). clear H. t.
+  assert (x = x2 /\ x3 = x0 /\ x4 = x1).
+  generalize x2 x3 x4 H H5 H6 x x0 x1 H1 H3 H4.
+  clear x2 x3 x4 H H5 H6 x x0 x1 H1 H3 H4.  clear H2 H0.
+  generalize instruction_grammar_list. induction l.
+  simpl. intros. generalize (nil_is_nil_app_nil _ _ H). t. discriminate H2.
+  simpl in *. intros. destruct x2. simpl in H. injection H ; clear H ; intros ; subst.
+  destruct x. simpl in *. injection H1 ; clear H1 ; intros ; subst. auto.
+  simpl in *. injection H1. intros ; subst. clear H1. assert False.
+  apply H4. exists s2. exists v1. rewrite in_alts_g. simpl. apply in_alt_l. auto.
+  contradiction. simpl in H. injection H. intros. subst. clear H.
+  destruct x. simpl in H1. injection H1 ; clear H1 ; intros ; subst.
+  assert False ; [ idtac | contradiction ]. simpl in *. apply H4.
+  exists s2. exists v1. apply in_alts_comm'. rewrite in_alts_g.
+  simpl. apply in_alt_l. auto. simpl in *. injection H1. intros ; subst. clear H1.
+  specialize (fun H1 H2 => IHl _ _ _ (eq_refl _) H5 H1 _ _ _ H H3 H2).
+  assert (~ (exists (s3 : list char_p) (v' : prefix * instr),
+               in_grammar (alts (x2 ++ x4)) ((s1 ++ s2) ++ s3) v')).
+  intro. t. apply H6. exists x5. exists x6. rewrite in_alts_g.
+  apply in_alt_r. rewrite in_alts_g in H0. apply H0. specialize (IHl H0).
+  assert (~ (exists (s2 : list char_p) (v' : prefix * instr),
+           in_grammar (alts (x ++ x1)) (s1 ++ s2) v')).
+  intro. t. apply H4. exists x5. exists x6. rewrite in_alts_g. apply in_alt_r.
+  apply in_alts_g. auto. specialize (IHl H1). t. subst. auto. t. subst. clear H1.
+  assert (exists pre, exists g, x0 = (pre $ g) /\ 
+                                star_free pre = true /\ 
+                                check_determ g = true /\ 
+                                check_pfx pre g = true) ; 
+    [ idtac | t ; subst ; eapply check_pfx_determ' ; eauto].
+  generalize (splits_in x0 x2 x1). rewrite <- H. intros.
+  unfold instruction_grammar_list in H1.
+  repeat rewrite in_app in H1. 
+  repeat rewrite in_map_iff in H1.
+  Ltac foo := 
+    match goal with
+      | [ H : _ \/ _ |- _ ] => 
+        destruct H ; [t ; subst ; econstructor ; econstructor ; split ; eauto ; split | 
+                      foo ]
+      | _ => idtac
+    end.
+  foo. apply star_free_prefix_grammar_rep. split. apply instr_grammars_determ. auto.
+  apply check_all_rep ; auto.
+  apply star_free_prefix_grammar_rep_or_repn. split. apply instr_grammars_determ. auto.
+  apply check_all_rep_or_repn ; auto.
+  apply star_free_prefix_grammar_lock_with_op_override. split. 
+  apply instr_grammars_determ ; auto. apply check_all_lock_with_op_override ; auto.
+  apply star_free_prefix_grammar_lock_no_op_override. split.
+  apply instr_grammars_determ ; auto. apply check_all_lock_no_op_override ; auto.
+  apply star_free_prefix_grammar_seg_with_op_override. split.
+  apply instr_grammars_determ ; auto 10. apply check_all_seg_with_op_override ; auto.
+  apply star_free_prefix_grammar_seg_op_override. split.
+  apply instr_grammars_determ ; auto 10. apply check_all_seg_op_override ; auto.
+  t ; subst ; econstructor ; econstructor ; split ; eauto ; split.
+  apply star_free_prefix_grammar_seg_override. split.
+  apply instr_grammars_determ ; auto 10. apply check_all_seg_override ; auto.
 Qed.
-
-(** Now I want to relate the [simple_parser] to the results above.
-    Note that both the DFA and the simpler parser assume that at
+  
+(** Now I want to relate the [simple_grammar] to the results above.
+    Note that both the DFA and the simpler grammar assume that at
     least one byte is consumed.  So we have to establish that indeed,
-    the parsers require at least one byte on all paths.  While I'm
+    the grammars require at least one byte on all paths.  While I'm
     at it, I calculate the maximum number of bits on any path (but
     haven't bothered to prove it correct.) *)
 Require Import Arith.Compare_dec.
@@ -1301,30 +1957,31 @@ Require Import Arith.Compare_dec.
 Definition max(n1 n2:nat) : nat := if le_lt_dec n1 n2 then n2 else n1.
 Definition min(n1 n2:nat) : nat := if le_lt_dec n1 n2 then n1 else n2.
 
-(** Maximum number of bits consumed by a parser.  Undefined if the
-    parser includes [Star_p]. *)
-Fixpoint max_bit_count t (p:parser t) : option nat := 
+(** Maximum number of bits consumed by a grammar.  Undefined if the
+    grammar includes [Star_p]. *)
+Fixpoint max_bit_count t (p:grammar t) : option nat := 
   match p with 
-    | Eps_p => Some 0
-    | Zero_p _ => Some 0
-    | Char_p _ => Some 1
-    | Any_p => Some 1
-    | Cat_p _ _ p1 p2 => 
+    | Eps => Some 0
+    | Zero _ => Some 0
+    | Char _ => Some 1
+    | Any => Some 1
+    | Cat _ _ p1 p2 => 
       match max_bit_count p1, max_bit_count p2 with
         | Some n1, Some n2 => Some (n1 + n2)
         | _,_ => None
       end
-    | Map_p _ _ _ p => max_bit_count p
-    | Alt_p _ p1 p2 => 
+    | Map _ _ _ p => max_bit_count p
+    | Xform _ _ _ p => max_bit_count p
+    | Alt _ _ p1 p2 => 
       match max_bit_count p1, max_bit_count p2 with
         | Some n1, Some n2 => Some (max n1 n2)
         | _,_ => None
       end
-    | Star_p _ _ => None
+    | Star _ _ => None
   end%nat.
 
-Lemma max_count_corr : forall t (p: parser t) s v,
-  in_parser p s v -> 
+Lemma max_count_corr : forall t (p: grammar t) s v,
+  in_grammar p s v -> 
   match max_bit_count p with 
     | None => True
     | Some n => length s <= n
@@ -1339,42 +1996,41 @@ Proof.
       end ; try omega; auto; try (rewrite app_length; omega).
 Qed.
 
-Eval vm_compute in (max_bit_count instruction_parser).
-
 Lemma max_instruction_bits: 
-  max_bit_count instruction_parser = Some 104.
+  max_bit_count instruction_grammar = Some 104.
 Proof.
   vm_compute; auto.
 Qed.
 
-(** Minimum number of bits consumed by the parser.  This is undefined
-    when the parser is [Zero_p].  Or rather, we use [None] to represent
+(** Minimum number of bits consumed by the grammar.  This is undefined
+    when the grammar is [Zero_p].  Or rather, we use [None] to represent
     "minimum infinity" to get this to work out properly. *)
-Fixpoint min_bit_count t (p:parser t) : option nat := 
+Fixpoint min_bit_count t (p:grammar t) : option nat := 
   match p with 
-    | Eps_p => Some 0
-    | Zero_p _ => None
-    | Char_p _ => Some 1
-    | Any_p => Some 1
-    | Cat_p _ _ p1 p2 => 
+    | Eps => Some 0
+    | Zero _ => None
+    | Char _ => Some 1
+    | Any => Some 1
+    | Cat _ _ p1 p2 => 
       match min_bit_count p1, min_bit_count p2 with
         | Some n1, Some n2 => Some (n1 + n2)
         | _,_ => None
       end
-    | Map_p _ _ _ p => min_bit_count p
-    | Alt_p _ p1 p2 => 
+    | Map _ _ _ p => min_bit_count p
+    | Xform _ _ _ p => min_bit_count p
+    | Alt _ _ p1 p2 => 
       match min_bit_count p1, min_bit_count p2 with
         | Some n1, Some n2 => Some (min n1 n2)
         | Some n1, None => Some n1
         | None, Some n1 => Some n1
         | _, _ => None
       end
-    | Star_p _ _ => Some 0
+    | Star _ _ => Some 0
   end%nat.
 
 (** If [s] is in the domain of [p], then [length s] is at least [min_bit_count p]. *)
-Lemma min_count_corr : forall t (p:parser t) s v,
-  in_parser p s v -> 
+Lemma min_count_corr : forall t (p:grammar t) s v,
+  in_grammar p s v -> 
   match min_bit_count p with 
     | None => False
     | Some n => length s >= n
@@ -1390,35 +2046,206 @@ Proof.
   rewrite app_length. omega.
 Qed.
 
-(** The [instruction_parser] always consumes at least 8 bits.  *)
+(** The [instruction_grammar] always consumes at least 8 bits.  *)
 Lemma min_instruction_bits : 
-  min_bit_count instruction_parser = Some 8.
+  min_bit_count instruction_grammar = Some 8.
 Proof.
   vm_compute ; auto.
 Qed.
 
 (** Probably goes in the Parser file.  In fact, this whole file would be
-    much simpler if I could just calculate derivatives directly on parsers,
+    much simpler if I could just calculate derivatives directly on grammars,
     instead of having to convert them to regexps.  *)
-Lemma in_derivs_app t (x1 x2:list char_p) (c:ctxt_t) (r:regexp t) (v:result_m t): 
-  wf_regexp c r -> 
-  in_regexp c (deriv_parse' (deriv_parse' r x1) x2) nil v -> 
-  in_regexp c r (x1 ++ x2) v.
+Ltac pinvopt := 
+  match goal with 
+    | [ H : in_grammar (OptAlt _ _) _ _ |- _ ] => rewrite <- opt_alt_corr in H
+    | [ H : in_grammar (OptCat _ _) _ _ |- _ ] => rewrite <- opt_cat_corr in H
+    | [ H : in_grammar (OptMap _ _ _) _ _ |- _] => rewrite <- opt_map_corr in H
+    | [ H : in_grammar (OptXform _ _) _ _ |- _] => rewrite <- opt_xform_corr in H
+    | [ |- in_grammar (OptAlt _ _) _ _ ] => rewrite <- opt_alt_corr
+    | [ |- in_grammar (OptCat _ _) _ _ ] => rewrite <- opt_cat_corr
+    | [ |- in_grammar (OptMap _ _ _) _ _ ] => rewrite <- opt_map_corr
+    | [ |- in_grammar (OptXform _ _) _ _ ] => rewrite <- opt_xform_corr
+    | _ => pinv
+  end.
+
+Lemma null_emp t (g:grammar t) cs v : 
+  in_grammar (null g) cs v -> cs = nil.
 Proof.
-  induction x1. simpl. intros. eapply Deriv'1. auto. auto.
-  intros. simpl. eapply Deriv2. auto. eapply IHx1. eapply wf_deriv. eauto.
-  eauto.
+  induction g ; simpl ; intros ; repeat pinvopt ; eauto.  
+  rewrite (IHg1 _ _ H) ; rewrite (IHg2 _ _ H0). auto.
+Qed.
+
+Lemma null_corr t (g:grammar t) cs v : 
+  in_grammar (null g) cs v -> in_grammar g nil v.
+Proof.
+  induction g ; simpl ; intros ; repeat pinvopt ; eauto.
+Qed.
+
+Lemma star_inv t (g:grammar t) s v : 
+  in_grammar (Star g) s v -> 
+  ((s = nil /\ v = nil) \/ 
+       (exists s1, exists s2, exists v1:interp t, exists v2:interp (List_t t),
+         s1 <> nil /\ s = s1 ++ s2 /\ v = v1::v2 /\ 
+         in_grammar g s1 v1 /\ in_grammar (Star g) s2 v2)).
+Proof.
+  intros. inversion H. subst. left ; auto. 
+  repeat 
+  match goal with 
+    | [ H : existT ?f ?t ?x = existT ?f ?t ?y |- _ ] => 
+      generalize (inj_pairT2 _ f t x y H) ; clear H
+  end. intros ; subst ; auto.
+  right.
+  repeat 
+  match goal with 
+    | [ H : existT ?f ?t ?x = existT ?f ?t ?y |- _ ] => 
+      generalize (inj_pairT2 _ f t x y H) ; clear H
+  end. intros ; subst. exists s1. exists s2. exists v1. exists v2. auto.
+Qed.
+
+Lemma null_corr' t (g:grammar t) v : 
+  in_grammar g nil v -> in_grammar (null g) nil v.
+Proof.
+  induction g ; intros ; simpl ; auto ; repeat pinvopt ; try discriminate H ; eauto.
+  generalize (nil_is_nil_app_nil _ _ H1). t. subst. rewrite H1. econstructor ; eauto.
+  econstructor ; eauto. generalize (star_inv H). intros. destruct H0 ; t.
+  subst ; auto. generalize (nil_is_nil_app_nil _ _ H1). t ; subst. 
+  congruence.
+Qed.
+
+Lemma deriv_corr t (g:grammar t) c v cs : 
+  in_grammar (deriv g c) cs v <-> in_grammar g (c::cs) v.
+Proof.
+  induction g ; simpl ; intros ; split ; intros ; repeat pinvopt ; eauto.
+  discriminate H. destruct (char_dec c0 c) ; subst ; repeat pinv ; eauto.
+  destruct (char_dec c c) ; try congruence. econstructor ; eauto. 
+  econstructor ; eauto. apply IHg1 ; eauto. auto. auto.
+  generalize (null_emp _ H). generalize (null_corr _ H). intros.
+  econstructor. eauto. apply IHg2 ; eauto. subst ; auto. auto. 
+  destruct x. simpl in *. subst. specialize (IHg2 c x2 cs).
+  econstructor ; eauto. pinvopt. eapply InAlt_r. pinvopt.
+  econstructor. eapply null_corr'. eauto. eapply IHg2. eauto. auto.
+  eauto. eauto. auto. simpl in H1 ; injection H1 ; clear H1 ; t ; subst.
+  econstructor. pinvopt. eapply InAlt_l. pinvopt. econstructor.
+  apply IHg1 ; eauto. eauto. auto. eauto. eauto. eauto.
+  eapply InAlt_l. eapply IHg1 ; eauto. auto.
+  eapply InAlt_r ; eauto. eapply IHg2 ; eauto.
+  eapply InAlt_l ; eauto. eapply IHg1 ; eauto. eapply InAlt_r ; eauto.
+  eapply IHg2 ; eauto. eapply InStar_cons. specialize (IHg c x2 x0).
+  eapply IHg. eauto. eauto. congruence. auto. auto.
+  generalize (star_inv H). clear H. t. destruct H ; t. congruence. subst.
+  destruct x ; try congruence. simpl in H0 ; injection H0 ; intros ; subst ;
+  clear H0. econstructor. pinvopt. econstructor. eapply IHg ; eauto.
+  eauto. auto. eauto. auto. econstructor. eapply IHg ; eauto. auto.
+  econstructor. eapply IHg ; eauto. auto. econstructor ; eauto.
+  eapply IHg ; eauto. econstructor ; eauto ; eapply IHg ; eauto.
 Qed.  
 
+Fixpoint derivs t (g:grammar t) (cs : list char_p) : grammar t := 
+  match cs with 
+    | nil => g
+    | c::cs' => derivs (deriv g c) cs'
+  end.
+
+Lemma derivs_corr t v cs2 cs1 (g:grammar t) : 
+  in_grammar (derivs g cs1) cs2 v <-> in_grammar g (cs1 ++ cs2) v.
+Proof.
+  induction cs1 ; simpl ; intros ; split ; intros ; auto.
+  eapply deriv_corr. eapply IHcs1. auto. eapply IHcs1.
+  eapply deriv_corr. auto.
+Qed.
+
+Lemma in_derivs_app t (x1 x2:list char_p) (r:grammar t) (v:interp t): 
+  in_grammar (derivs (derivs r x1) x2) nil v -> 
+  in_grammar r (x1 ++ x2) v.
+Proof.
+  intros. eapply derivs_corr. generalize (derivs r x1) H ; clear H ; intros.
+  replace (x2) with (x2 ++ nil). apply derivs_corr. auto. rewrite app_nil_end.
+  auto.
+Qed.  
+
+Fixpoint extract_nil t (g:grammar t) : list (interp t) := 
+  match g in grammar t return list (interp t) with
+    | Eps => tt::nil
+    | Zero t => nil
+    | Char c => nil
+    | Any => nil
+    | Cat t1 t2 g1 g2 => cross_prod (extract_nil g1) (extract_nil g2)
+    | Alt t1 t2 g1 g2 => 
+      (List.map (fun x => inl _ x) (extract_nil g1)) ++ 
+      (List.map (fun x => inr _ x) (extract_nil g2))
+    | Star t g => nil::nil
+    | Map t1 t2 f g => List.map f (extract_nil g)
+    | Xform t1 t2 x g => List.map (xinterp x) (extract_nil g)
+  end.                                                     
+
+Lemma extract_nil_corr t (g:grammar t) v :
+  in_grammar g nil v <-> In v (extract_nil g).
+Proof.  
+  induction g; simpl ; intros ; split ; intro ; repeat pinvopt ; auto ; 
+  try (congruence || contradiction).
+  generalize (nil_is_nil_app_nil _ _ H1). clear H1 ; t. subst.
+  specialize (IHg1 x1). specialize (IHg2 x2). destruct IHg1. destruct IHg2.
+  clear H2 H4. specialize (H1 H). specialize (H3 H0). clear H H0.
+  generalize H1 H3 ; clear H1 H3. generalize (extract_nil g1) (extract_nil g2).
+  clear g1 g2. induction l ; simpl ; intros ; auto. destruct H1.
+  subst. apply in_app. left. induction l0 ; simpl in *. auto.
+  destruct H3. subst. left ; auto. specialize (IHl0 H). auto. 
+  apply in_app ; right. auto. destruct v as [x1 x2].
+  specialize (IHg1 x1). specialize (IHg2 x2). destruct IHg1. destruct IHg2.
+  clear H0 H2. replace (@nil char_p) with (@nil char_p ++ nil).
+  econstructor ; eauto. apply H1. generalize (extract_nil g1) H.
+  induction l ; simpl ; intros ; auto. rewrite in_app in H0. destruct H0.
+  left. generalize (extract_nil g2) H0. induction l0 ; simpl ; intros ; 
+  try contradiction. destruct H2 ; auto. injection H2 ; intros ; subst ; auto.
+  right ; auto. apply H3. generalize (extract_nil g1) (extract_nil g2) H.
+  induction l ; simpl ; intros ; try contradiction. rewrite in_app in H0.
+  destruct H0. generalize H0 ; clear H0. induction l0 ; simpl ; intros ;
+  try contradiction. destruct H0. left. injection H0 ; intros ; subst ; auto.
+  right. auto. auto. auto. specialize (IHg1 x). destruct IHg1.
+  specialize (H0 H). rewrite in_app. left. generalize (extract_nil g1) H0.
+  induction l ; simpl ; intros ; try contradiction. destruct H2 ; [ left ; subst ; auto 
+  | right ]. auto.
+  specialize (IHg2 x). destruct IHg2. specialize (H0 H). apply in_app.
+  right. generalize (extract_nil g2) H0. induction l ; simpl ; intros ;  
+  try contradiction. destruct H2 ; [left ; subst ; auto | right ; auto].
+  rewrite in_app in H. destruct v. eapply InAlt_l ; eauto. 
+  destruct H. specialize (IHg1 i). destruct IHg1. apply H1. clear H0 H1 IHg2.
+  generalize (extract_nil g1) H. induction l ; simpl ; intros ; try contradiction.
+  destruct H0 ; auto. injection H0 ; intros ; subst ; auto. assert False.
+  generalize (extract_nil g2) H. induction l ; simpl ; intros ; auto.
+  destruct H0 ; auto. discriminate. contradiction. clear IHg1. specialize (IHg2 i).
+  destruct IHg2. eapply InAlt_r ; eauto. apply H1. clear H0 H1. destruct H.
+  assert False. generalize (extract_nil g1) H. induction l ; simpl ; intros ; auto. 
+  destruct H0 ; auto. discriminate. contradiction.
+  generalize (extract_nil g2) H. induction l ; simpl ; intros ; try contradiction.
+  destruct H0. injection H0 ; intros ; subst. left ; auto. right ; auto.
+  generalize (star_inv H). clear H. t. destruct H ; t ; subst ; auto.
+  generalize (nil_is_nil_app_nil _ _ H0). t ; subst. contradiction.
+  specialize (IHg x). destruct IHg. apply in_map. auto.
+  assert (exists x, v = i x /\ In x (extract_nil g)). 
+  generalize (extract_nil) H. 
+  induction l ; simpl ; t ; try contradiction. destruct H0 ; eauto. 
+  specialize (IHl H0). t. subst. eauto. t. subst.
+  specialize (IHg x). destruct IHg. specialize (H2 H1).  
+  econstructor ; eauto.
+  specialize (IHg x0). destruct IHg. apply in_map. eauto.
+  assert (exists z, v = xinterp x z /\ In z (extract_nil g)).
+  generalize (extract_nil g) H. induction l ; simpl ; t. contradiction.
+  destruct H0 ; eauto. specialize (IHl H0). t. eauto. t. subst.
+  econstructor ; eauto. apply IHg. eauto.
+Qed.
+
+(*
 (** If [apply_null] on [derivs p cs] is [nil], then there's no value associated
    with [cs] in the denotation of [p]. *)
 Lemma apply_null_nil : 
-  forall (c:ctxt_t) t (p:parser t) (r:regexp t) cs,
+  forall (c:ctxt_t) t (p:grammar t) (r:regexp t) cs,
     c = snd (parser2regexp p) ->
     r = deriv_parse' (fst (parser2regexp p)) cs ->
     forall (H:wf_regexp c r),
     apply_null c r H = nil -> 
-    forall v, ~ in_parser p cs v.
+    forall v, ~ in_grammar p cs v.
 Proof.
   intros c t p r cs H1 H2. rewrite H1. rewrite H2. intros. intro.
   assert (in_regexp (snd (parser2regexp p)) (fst (parser2regexp p)) cs v).
@@ -1456,6 +2283,7 @@ Proof.
   assert (wf_derivs c (a::cs1) r H = wf_derivs c cs1 (deriv r a) (wf_deriv c r a H)).
   apply Coqlib.proof_irrelevance. rewrite H1. auto.
 Qed.
+*)
 
 (** A surprisingly tricky little lemma used below. *)
 Lemma foo_app A (x s1 s2 s3:list A) (v:A) : 
@@ -1477,6 +2305,7 @@ Proof.
   intros. subst. auto.
 Qed.
 
+(*
 (** This lemma establishes a relationship between a parser [p] and the
     execution of the [simple_parse'] loop.  In particular, if we are
     in the loop processing [derivs p bytes1] and trying to process [bytes2],
@@ -1509,15 +2338,15 @@ Lemma simple_parse'_corr2 :
   | None => 
     forall s1 s2 v, 
       s1 ++ s2 = bytes1 ++ bytes2 -> 
-      ~ in_parser p (flat_map byte_explode s1) v
+      ~ in_grammar p (flat_map byte_explode s1) v
   | Some (v,bytes3) => 
     exists bytes4,
       bytes2 = bytes4 ++ bytes3 /\ 
-      in_parser p (flat_map byte_explode (bytes1 ++ bytes4)) v /\
+      in_grammar p (flat_map byte_explode (bytes1 ++ bytes4)) v /\
       (forall bytes5 bytes6,
         bytes2 = bytes5 ++ bytes6 -> 
         length bytes5 < length bytes4 -> 
-        forall v, ~ in_parser p (flat_map byte_explode (bytes1 ++ bytes5)) v)
+        forall v, ~ in_grammar p (flat_map byte_explode (bytes1 ++ bytes5)) v)
   end.
 Proof.
   Opaque byte_explode.
@@ -1610,23 +2439,48 @@ Proof.
             (fst (parser2regexp p)) (p2r_wf p initial_ctxt) = inst_regexp_wf0).
   apply Coqlib.proof_irrelevance. rewrite <- H. auto.
 Qed.
+*)
+
+Lemma min_none : 
+  forall t (g:grammar t),
+    min_bit_count g = None -> extract_nil g = nil.
+Proof.
+  induction g ; simpl ; intros ; try congruence.
+  destruct (min_bit_count g1) ; try congruence ; destruct (min_bit_count g2) ;  
+  try congruence. rewrite IHg2. generalize (extract_nil g1). induction l ; auto. auto.
+  rewrite IHg1 ; auto. rewrite IHg1 ; auto. destruct (min_bit_count g1) ; 
+  destruct (min_bit_count g2) ; try congruence. rewrite IHg1 ; auto ; rewrite IHg2 ; auto.
+  rewrite IHg ; auto. rewrite IHg ; auto.
+Qed.
 
 (** If the [min_bit_count] of [p] is greater than 0, then there's no 
     way that [apply_null] will succeed. *)
 Lemma min_count_not_null : 
-  forall n t (p:parser t),
+  forall t (p:grammar t) n,
     min_bit_count p = Some (S n) -> 
-    apply_null (snd (parser2regexp p)) (fst (parser2regexp p)) 
-    (p2r_wf p initial_ctxt) = nil.
+    extract_nil p = nil.
 Proof.
-  intros.
-  generalize (@ApplyNull2  (snd (parser2regexp p)) _ (fst (parser2regexp p))
-  (p2r_wf _ _)). destruct (apply_null (snd (parser2regexp p)) (fst (parser2regexp p))
-  (p2r_wf p initial_ctxt)). auto. intros. specialize (H0 r). assert (In r (r::l)).
-  left ; auto. specialize (H0 H1). assert (in_parser p nil r). eapply r2p_ok. eauto. 
-  generalize (min_count_corr H2).  rewrite H. simpl. intros. assert False. omega.
-  contradiction.
+  induction p ; simpl ; intros ; try congruence.
+  remember (min_bit_count p1) as e1. remember (min_bit_count p2) as e2.
+  destruct e1 ; try congruence. destruct e2 ; try congruence.
+  destruct n0 ; destruct n1 ; simpl in * ; try congruence. 
+  specialize (IHp2 _ (eq_refl _)). 
+  rewrite IHp2. generalize (extract_nil p1). induction l ; simpl ; auto.
+  specialize (IHp1 _ (eq_refl _)). rewrite IHp1. auto.
+  specialize (IHp1 _ (eq_refl _)). rewrite IHp1. auto.
+  remember (min_bit_count p1) as e1. remember (min_bit_count p2) as e2. 
+  destruct e1 ; destruct e2 ; try congruence.
+  unfold min in H. destruct (le_lt_dec n0 n1) ; injection H ; intros ; subst.
+  specialize (IHp1 _ (eq_refl _)). rewrite IHp1.
+  destruct n1. assert False. omega. contradiction. specialize (IHp2 _ (eq_refl _)).
+  rewrite IHp2. auto. rewrite (IHp2 _ (eq_refl _)).
+  destruct n0. assert False. omega. contradiction. rewrite (IHp1 _ (eq_refl _)). auto.
+  injection H ; intros ; subst. rewrite (IHp1 _ (eq_refl _)). simpl. rewrite min_none ;
+  auto. erewrite IHp2 ; eauto. rewrite min_none ; auto. erewrite IHp ; eauto.
+  erewrite IHp ; eauto.
 Qed.
+
+(*XXXXXXXXX*)
 
 (** Finally, the connection that directly ties execution of the DFA for
     the [non_cflow] parser to the [simple_parse] above.  This says that
@@ -1773,7 +2627,7 @@ Qed.
 (** Show that the instruction we get out of the [dir_cflow] parsers satisfies
     the [dir_cflow_instr] predicate. *)
 Lemma dir_cflow_instr_inv (ins:instr) (s:list char_p) : 
-  in_parser (alts dir_cflow) s ins -> 
+  in_grammar (alts dir_cflow) s ins -> 
   dir_cflow_instr (mkPrefix None None false false) ins = true.
 Proof.
   unfold dir_cflow. simpl ; 
@@ -1783,12 +2637,12 @@ Qed.
 
 (** Show that the [dir_cflow] parsers are sub-parsers of the [instruction_parser]. *)
 Lemma dir_cflow_parser_subset : 
-  forall s v, in_parser (alts dir_cflow) s v -> 
-    in_parser instruction_parser s (mkPrefix None None false false, v).
+  forall s v, in_grammar (alts dir_cflow) s v -> 
+    in_grammar instruction_parser s (mkPrefix None None false false, v).
 Proof.
   intros. replace s with (nil ++ s) ; auto. 
   remember (mkPrefix None None false false) as p.
-  assert (in_parser prefix_parser_nooverride nil p). 
+  assert (in_grammar prefix_parser_nooverride nil p). 
   unfold prefix_parser_nooverride. unfold option_perm2. subst.
   repeat econstructor. clear Heqp. unfold dir_cflow in H. simpl in H.
   Transparent instruction_parser.
@@ -1797,21 +2651,21 @@ Proof.
   econstructor ; eauto. clear H0. repeat pinv ; unfold instr_parsers_nosize_pre ; simpl.
   repeat 
   match goal with 
-    | [ |- in_parser (JMP_p |+| _) _ _ ] => eapply Alt_left_pi
-    | [ |- in_parser (_ |+| _) _ _ ] => eapply Alt_right_pi
+    | [ |- in_grammar (JMP_p |+| _) _ _ ] => eapply Alt_left_pi
+    | [ |- in_grammar (_ |+| _) _ _ ] => eapply Alt_right_pi
   end.
   unfold dir_near_JMP_p, JMP_p in *. pinv. destruct H.
   eapply Alt_left_pi. auto. eapply Alt_right_pi. eapply Alt_left_pi. auto.
   repeat 
   match goal with 
-    | [ |- in_parser (Jcc_p |+| _) _ _ ] => eapply Alt_left_pi
-    | [ |- in_parser (_ |+| _) _ _ ] => eapply Alt_right_pi
+    | [ |- in_grammar (Jcc_p |+| _) _ _ ] => eapply Alt_left_pi
+    | [ |- in_grammar (_ |+| _) _ _ ] => eapply Alt_right_pi
   end.
   unfold dir_near_Jcc_p, Jcc_p in *. auto.
   repeat 
   match goal with 
-    | [ |- in_parser (CALL_p |+| _) _ _ ] => eapply Alt_left_pi
-    | [ |- in_parser (_ |+| _) _ _ ] => eapply Alt_right_pi
+    | [ |- in_grammar (CALL_p |+| _) _ _ ] => eapply Alt_left_pi
+    | [ |- in_grammar (_ |+| _) _ _ ] => eapply Alt_right_pi
   end.
   unfold dir_near_CALL_p, CALL_p in *. eapply Alt_left_pi. auto.
   unfold never in *. pinv.
@@ -1828,15 +2682,15 @@ Lemma dir_cflow_dfa_corr1 :
     forall (bytes:list int8) (n:nat) (nats2:list nat),
       dfa_recognize 256 d (List.map byte2token bytes) = Some (n,nats2) -> 
       exists bytes1, exists pfx:prefix, exists ins:instr, 
-        in_parser (alts dir_cflow) (flat_map byte_explode bytes1) ins /\ 
-        in_parser instruction_parser (flat_map byte_explode bytes1) (pfx,ins) /\ 
+        in_grammar (alts dir_cflow) (flat_map byte_explode bytes1) ins /\ 
+        in_grammar instruction_parser (flat_map byte_explode bytes1) (pfx,ins) /\ 
         n = length bytes1 /\ 
         bytes = bytes1 ++ (List.map nat_to_byte nats2) /\ 
         dir_cflow_instr pfx ins = true /\
         (forall ts3 ts4,
           (length ts3 < length bytes1)%nat -> 
           bytes = ts3 ++ ts4 -> 
-          forall v0, ~ in_parser (alts dir_cflow) (flat_map byte_explode ts3) v0).
+          forall v0, ~ in_grammar (alts dir_cflow) (flat_map byte_explode ts3) v0).
 Proof.
   intros. subst. rewrite build_dfa_eq in H.
   generalize (dfa_recognize_corr _ _ _ _ H (List.map byte2token bytes)
