x86model/RockSalt/VerifierDFA.v
@@ -16,6 +16,7 @@
 *)
 Require Import Coqlib.
 Require Import Parser.
+Require Import Recognizer.
 Require Import Ascii.
 Require Import String.
 Require Import List.
@@ -39,6 +40,7 @@ Definition logChunkSize := 5%nat.
 Definition chunkSize := two_power_nat logChunkSize.
 Notation int8_of_nat n := (@repr 7 (Z_of_nat n)).
 Definition safeMask := shl (Word.mone 7) (int8_of_nat logChunkSize).
+Local Open Scope Z_scope.
 
 Fixpoint int2bools_aux (bs : Z -> bool) (n: nat) : list bool :=
   match n with
@@ -53,61 +55,142 @@ Definition nat2bools(n:nat) : list bool :=
   let bs := Word.bits_of_Z 8 (Z_of_nat n) in
     ((bs 7)::(bs 6)::(bs 5)::(bs 4)::(bs 3)::(bs 2)::(bs 1)::(bs 0)::nil)%Z.
 
-(* Definition make_dfa t (p:grammar t) := build_dfa 256 nat2bools 400 (par2rec p). *)
-(* Implicit Arguments make_dfa [t]. *)
+Definition make_dfa t (p:grammar t) := build_dfa 400 (par2rec p).
+Implicit Arguments make_dfa [t].
 
-(** Subset of the parsers that don't do control-flow, and do not allow the
-    operand size override prefix. *)
-Definition non_cflow_instrs_nosize_pre : list (grammar instruction_t) := 
-  instr_grammars_lock_no_op_override ++
-  instr_grammars_seg_override.
+(** We mirror the definitions in Decode but only for valid, non-control-flow
+    instructions below.  Instructions that are commented out are presumed *not* 
+    valid.  I've been a little conservative and ruled out many systems level
+    instructions, such as INS, OUTS, LODS, etc.  Still, we really ought to 
+    audit this list carefully.
+*)
 
-(** Subset of the parsers that don't do control-flow, but allow the
-    operand size override prefix *)
-Definition non_cflow_instrs_opsize_pre : list (grammar instruction_t) := 
-  instr_grammars_lock_with_op_override ++
-  instr_grammars_seg_with_op_override ++
+(* this set of instructions can take prefixes in prefix_grammar_rep;
+     that is, in lock_or_rep, only rep can be used;
+     we put RET in this category because it turns out many binaries use
+     the "rep ret" sequence to avoid branch prediction panelty in AMD processors;
+     intel processor seems to just ignore the rep prefix *)
+Definition valid_instr_grammars_rep :=
+    (*INS_p :: OUTS_p :: *) MOVS_p :: (* LODS_p ::*) STOS_p :: (*RET_p ::*) nil.
+
+(* this set of instructions can take prefixes in prefix_grammar_repn;
+      that is, in lock_or_rep, only repn can be used *)
+Definition valid_instr_grammars_rep_or_repn := 
+  instr_grammars_rep_or_repn.
+
+(* this set of instructions can take prefixes in 
+     prefix_grammar_lock_with_op_override;
+     that is, in lock_or_rep, only lock can be used;
+     and op_override prefix *must* be used *)
+Definition valid_instr_grammars_lock_with_op_override := 
+  instr_grammars_lock_with_op_override.
+
+(* this set of instructions can take prefixes in 
+     prefix_grammar_lock_no_op_override;
+     that is, in lock_or_rep, only lock can be used;
+     and op_override prefix *must not* be used *)
+Definition valid_instr_grammars_lock_no_op_override := 
+  instr_grammars_lock_no_op_override.
+
+(* this set of instructions can take prefixes in 
+     prefix_grammar_seg_op_override;
+     that is, it cannot take a lock_or_rep prefix, but can
+     optionally take segment or op override prefix *)
+Definition valid_instr_grammars_seg_op_override := 
   instr_grammars_seg_op_override.
 
-(** Subset of the parsers that don't do control-flow and which allow
-   the rep prefix - some of these are allowed to have 16 bit mode
-   in NaCl, but to be safe we'll not add those in unless we get a
-   failing test case. *)
-Definition non_cflow_instrs_rep_pre : list (grammar instruction_t) :=
-  CMPS_p :: MOVS_p :: STOS_p :: nil.
+(* this set of instructions can take only the seg_override prefix *)
+Definition valid_instr_grammars_seg_override := 
+    AAA_p :: AAD_p :: AAM_p :: AAS_p :: CMP_p false ::
+    (* ARPL_p :: *) BOUND_p :: BSF_p :: BSR_p :: BSWAP_p :: BT_p :: 
+    (* CALL_p :: *) CLC_p :: CLD_p :: CLI_p :: CLTS_p :: CMC_p :: CPUID_p :: DAA_p :: DAS_p ::
+    HLT_p :: IMUL_p false :: (* IN_p :: INTn_p :: INT_p :: INTO_p :: INVD_p :: INVLPG_p :: IRET_p :: Jcc_p :: JCXZ_p :: JMP_p :: *)
+    LAHF_p :: LAR_p :: (* LDS_p :: *) LEA_p :: LEAVE_p :: (* LES_p :: LFS_p :: LGDT_p ::*) LGS_p :: (* LIDT_p :: LLDT_p :: LMSW_p :: 
+    LOOP_p :: LOOPZ_p :: LOOPNZ_p :: LSL_p :: LSS_p :: LTR_p :: *) MOV_p false :: MOVCR_p :: MOVDR_p :: 
+    MOVSR_p :: MOVBE_p ::  (* OUT_p :: *) POP_p :: (* POPSR_p :: *) POPA_p :: POPF_p ::
+    PUSH_p :: PUSHSR_p :: PUSHA_p :: PUSHF_p :: RCL_p :: RCR_p :: (* RDMSR_p :: *) RDPMC_p :: RDTSC_p :: RDTSCP_p :: 
+    (* RSM_p :: *) SAHF_p :: SETcc_p :: (* SGDT_p :: SIDT_p :: *) SLDT_p :: SMSW_p :: STC_p :: STD_p :: (* STI_p :: *)
+    STR_p :: TEST_p false :: (* UD2_p :: VERR_p :: VERW_p :: *) WBINVD_p :: (* WRMSR_p :: XLAT_p :: *) F2XM1_p ::
+    FABS_p :: FADD_p :: FADDP_p :: FBLD_p :: FBSTP_p :: FCHS_p :: FCMOVcc_p :: FCOM_p :: FCOMP_p :: FCOMPP_p :: FCOMIP_p :: FCOS_p :: FDECSTP_p ::
+    FDIV_p :: FDIVP_p :: FDIVR_p :: FDIVRP_p :: FFREE_p :: FIADD_p :: FICOM_p :: FICOMP_p :: FIDIV_p :: FIDIVR_p :: FILD_p :: FIMUL_p :: FINCSTP_p
+    :: FIST_p :: FISTP_p :: FISUB_p :: FISUBR_p :: FLD_p :: FLD1_p :: FLDCW_p :: FLDENV_p :: FLDL2E_p :: FLDL2T_p :: FLDLG2_p :: FLDLN2_p
+    :: FLDPI_p :: FLDZ_p :: FMUL_p :: FMULP_p :: FNCLEX_p :: FNINIT_p :: FNOP_p :: FNSAVE_p :: FNSTCW_p :: FNSTSW_p :: FPATAN_p :: FPREM_p :: FPREM1_p :: FPTAN_p :: FRNDINT_p :: FRSTOR_p :: (* FSAVE_p :: *) 
+    FSCALE_p :: 
+    FSIN_p :: FSINCOS_p :: FSQRT_p :: FST_p :: (* FSTCW_p :: *) FSTENV_p :: FSTP_p :: FSUB_p :: FSUBP_p :: FSUBR_p :: FSUBRP_p ::FTST_p ::
+    FUCOM_p :: FUCOMP_p :: FUCOMPP_p :: FUCOMI_p :: FUCOMIP_p :: FXAM_p :: FXCH_p :: FXTRACT_p :: FYL2X_p :: FYL2XP1_p :: FWAIT_p :: 
+    EMMS_p :: MOVD_p :: MOVQ_p :: PACKSSDW_p :: PACKSSWB_p :: PACKUSWB_p :: PADD_p :: PADDS_p :: PADDUS_p :: PAND_p :: PANDN_p :: PCMPEQ_p :: PCMPGT_p :: 
+    PMADDWD_p :: PMULHUW_p :: PMULHW_p :: PMULLW_p :: POR_p :: PSLL_p :: PSRA_p :: PSRL_p :: PSUB_p :: PSUBS_p :: PSUBUS_p :: PUNPCKH_p :: PUNPCKL_p :: PXOR_p :: 
+    ADDPS_p :: ADDSS_p :: ANDNPS_p :: ANDPS_p :: CMPPS_p :: CMPSS_p :: COMISS_p :: CVTPI2PS_p :: CVTPS2PI_p :: CVTSI2SS_p :: CVTSS2SI_p :: CVTTPS2PI_p :: CVTTSS2SI_p ::
+    DIVPS_p :: DIVSS_p :: LDMXCSR_p :: MAXPS_p :: MAXSS_p :: MINPS_p :: MINSS_p :: MOVAPS_p :: MOVHLPS_p :: MOVLPS_p :: MOVMSKPS_p :: MOVSS_p :: MOVUPS_p :: MULPS_p ::
+    MULSS_p :: ORPS_p :: RCPPS_p :: RCPSS_p :: RSQRTPS_p :: RSQRTSS_p :: SHUFPS_p :: SQRTPS_p :: SQRTSS_p :: STMXCSR_p :: SUBPS_p :: SUBSS_p :: UCOMISS_p :: UNPCKHPS_p ::
+    UNPCKLPS_p :: XORPS_p :: PAVGB_p :: PEXTRW_p :: PINSRW_p :: PMAXSW_p :: PMAXUB_p :: PMINSW_p :: PMINUB_p :: PMOVMSKB_p :: PSADBW_p :: PSHUFW_p :: MASKMOVQ_p ::
+    MOVNTPS_p :: MOVNTQ_p :: PREFETCHT0_p :: PREFETCHT1_p :: PREFETCHT2_p :: PREFETCHNTA_p :: SFENCE_p :: nil.
 
-(** Prefixes allowed for non-control-flow operations that support an
-    operand size override.  We could possibly add in the lock and 
-    repeat prefixes, but I'm keeping things simple for now.  We cannot
-    allow the segment override prefix for NaCL. *)
-Definition valid_prefix_parser_opsize := 
-  op_override_p @ (fun p => mkPrefix None None p false %% prefix_t).
+Definition gs_segment_override_p : grammar segment_register_t := 
+"0110" $$ bits "0101" @ (fun _ => GS %% segment_register_t).
 
-(** Prefixes allowed for non-control-flow operations that do not support
-    an operand size override.  We could possibly add in the lock and
-    repeat prefixes, but I'm keeping things simple for now. We cannot
-    allows the segment override prefix for NaCL, except for GS *)
-Definition valid_prefix_parser_nooverride := 
-  Eps @ (fun p => (mkPrefix None None false false) %% prefix_t) |+|
-  ("0110" $$ bits "0101" @ (fun p => (mkPrefix None (Some GS) false false) %% prefix_t)).
+Definition valid_prefix_grammar_rep := 
+  option_perm3 rep_p gs_segment_override_p op_override_p @ 
+               (fun p => match p with (l, (s, op)) => 
+                                      mkPrefix l s (opt2b op false) false %% prefix_t
+                         end).
 
-(** We're only allowing rep for now - no lock - these are just the string ops. *)
-Definition valid_prefix_parser_rep :=
-  Eps @ (fun p => (mkPrefix None None false false) %% prefix_t) |+|
-  ("1111" $$ bits "0011" @ (fun _ => (mkPrefix (Some rep) None false false) %% prefix_t)).
+Definition valid_prefix_grammar_rep_or_repn :=
+    option_perm3 rep_or_repn_p gs_segment_override_p op_override_p @
+      (fun p => match p with (l, (s, op)) =>
+                  mkPrefix l s (opt2b op false) false %% prefix_t end).
 
+Definition valid_prefix_grammar_lock_with_op_override :=
+    option_perm3_variation lock_p gs_segment_override_p op_override_p @
+     (fun p => match p with (l, (s, op)) =>
+                 mkPrefix l s op false %% prefix_t end).
 
-(** The list of valid prefix and instruction parsers for non-control-flow
+Definition valid_prefix_grammar_lock_no_op_override :=
+    option_perm2 lock_p gs_segment_override_p @
+     (fun p => match p with (l, s) =>
+                 mkPrefix l s false false %% prefix_t end).
+
+Definition valid_prefix_grammar_seg_with_op_override := 
+    option_perm2_variation gs_segment_override_p op_override_p @
+     (fun p => match p with (s, op) =>
+                 mkPrefix None s op false %% prefix_t end).
+
+Definition valid_instr_grammars_seg_with_op_override := 
+  instr_grammars_seg_with_op_override.
+
+Definition valid_prefix_grammar_seg_op_override :=
+    option_perm2 gs_segment_override_p op_override_p @
+     (fun p => match p with (s, op) =>
+                 mkPrefix None s (opt2b op false) false %% prefix_t end).
+
+Definition valid_prefix_grammar_seg_override :=
+    option_perm gs_segment_override_p @
+     (fun s => mkPrefix None s false false %% prefix_t).
+
+(** The list of valid prefix and instruction grammars for non-control-flow
     operations. *)
-Definition non_cflow_parser_list := 
-  (List.map (fun (p:grammar instruction_t) => valid_prefix_parser_nooverride $ p) 
-    non_cflow_instrs_nosize_pre) ++
-  (List.map (fun (p:grammar instruction_t) => valid_prefix_parser_opsize $ p)
-    non_cflow_instrs_opsize_pre) ++
-  (List.map (fun (p:grammar instruction_t) => valid_prefix_parser_rep $ p)
-    non_cflow_instrs_rep_pre).
+Definition non_cflow_grammar_list := 
+  (List.map (fun (p:grammar instruction_t) => valid_prefix_grammar_rep $ p) 
+            valid_instr_grammars_rep) ++
+  (List.map (fun (p:grammar instruction_t) => valid_prefix_grammar_rep_or_repn $ p)
+            valid_instr_grammars_rep_or_repn) ++
+  (List.map (fun (p:grammar instruction_t) => 
+               valid_prefix_grammar_lock_with_op_override $ p)
+            valid_instr_grammars_lock_with_op_override) ++
+  (List.map (fun (p:grammar instruction_t) => 
+               valid_prefix_grammar_lock_no_op_override $ p)
+            valid_instr_grammars_lock_no_op_override) ++
+  (List.map (fun (p:grammar instruction_t) => 
+               valid_prefix_grammar_seg_with_op_override $ p)
+      valid_instr_grammars_seg_with_op_override) ++
+  (List.map (fun (p:grammar instruction_t) => 
+               valid_prefix_grammar_seg_op_override $ p)
+      valid_instr_grammars_seg_op_override) ++
+  (List.map (fun (p:grammar instruction_t) =>
+               valid_prefix_grammar_seg_override $ p)
+      valid_instr_grammars_seg_override).
 
-Definition non_cflow_parser := alts non_cflow_parser_list.
+Definition non_cflow_grammar := alts non_cflow_grammar_list.
 
 (* Direct jumps. Destinations will be checked to see if 
    they are known, valid starts of instructions. *)
@@ -144,7 +227,7 @@ Definition register_to_Z (r: register) :=
     | EBP => 5
     | ESI => 6
     | EDI => 7
-  end.
+  end%nat.
 
 (* Lemma register_to_Z_identity1: forall r:register, Z_to_register (register_to_Z r) = r. *)
 (* Proof. destruct r; auto. *)
@@ -200,6 +283,21 @@ Definition nacljmp_mask : list (grammar (Pair_t instruction_t instruction_t)) :=
   nacljmp_p EAX :: nacljmp_p ECX :: nacljmp_p EDX :: nacljmp_p EBX ::
   nacljmp_p EBP :: nacljmp_p ESI :: nacljmp_p EDI :: nil.
 
+Fixpoint parseloop ps bytes := 
+  match bytes with 
+    | nil => None
+    | b::bs => match parse_byte ps b with 
+                 | (ps', nil) => parseloop ps' bs
+                 (* JGM: FIX!  What to do with prefix? *)
+                 | (ps', (pfx,JMP true false (Imm_op disp) sel)::_) => 
+                   match bs with 
+                     | nil => Some disp
+                     | _ => None
+                   end
+                 | (ps', _) => None
+               end
+  end.
+
 (** Next, we define a boolean-valued test that tells whether an instruction
     is a valid non-control-flow instruction.  We should have the property
     that the [non_cflow_grammar] only builds instructions that satisfy this
@@ -209,6 +307,18 @@ Definition nacljmp_mask : list (grammar (Pair_t instruction_t instruction_t)) :=
 Definition no_imm_op(op1:operand) : bool := 
   match op1 with 
     | Imm_op _ => false
+    | _ => true
+  end.
+
+Definition no_mmx_imm_op(op1:mmx_operand) : bool := 
+  match op1 with 
+    | MMX_Imm_op _ => false
+    | _ => true
+  end.
+
+Definition no_sse_imm_op(op1:sse_operand) : bool := 
+  match op1 with 
+    | SSE_Imm_op _ => false
     | _ => true
   end.
 
@@ -222,6 +332,13 @@ Definition no_prefix (p : prefix) : bool :=
   match lock_rep p, seg_override p, op_override p, addr_override p with
     | None, None, false, false => true
     | _, _, _, _ => false
+  end.
+
+Definition only_seg_or_op (p : prefix) : bool := 
+  match lock_rep p, seg_override p, op_override p, addr_override p with
+      | None, (Some GS), _, false => true
+      | None, None, _, false => true
+      | _, _, _, _ => false
   end.
 
 Definition only_gs_seg_override (p:prefix) : bool := 
@@ -238,80 +355,363 @@ Definition only_lock_or_rep (p: prefix) : bool :=
     | _,_,_,_ => false
   end.
 
-Definition either_prefix (p:prefix) := 
-  only_op_override p || only_gs_seg_override p.
+Definition lock_or_gs (p:prefix) : bool := 
+  match lock_rep p, seg_override p, op_override p, addr_override p with
+    | _, Some GS, false, false => true
+    | _, None, false, false => true
+    | _, _, _, _ => false
+  end.
 
+Definition rep_or_gs_or_op_prefix (p:prefix) := 
+  negb (addr_override p) &&  
+  match lock_rep p with 
+    | None => true
+    | Some rep => true
+    | _ => false
+  end &&
+  match seg_override p with 
+    | None => true
+    | Some GS => true
+    | _ => false
+  end.
+
+Definition rep_or_repn_or_gs_or_op_prefix (p:prefix) := 
+  negb (addr_override p) && 
+  match lock_rep p with 
+    | None => true
+    | Some rep => true
+    | Some repn => true
+    | _ => false
+  end && 
+  match seg_override p with 
+    | None => true
+    | Some GS => true
+    | _ => false
+  end.
+
+Definition lock_or_gs_with_op (p:prefix) := 
+  match lock_rep p, seg_override p, op_override p, addr_override p with
+    | _, None, true, false => true
+    | _, Some GS, true, false => true
+    | _, _, _, _ => false
+  end.
+
+Definition lock_or_gs_without_op (p:prefix) := 
+  match lock_rep p, seg_override p, op_override p, addr_override p with
+    | _, None, false, false => true
+    | _, Some GS, false, false => true
+    | _, _, _, _ => false
+  end.
+                  
 Definition non_cflow_instr (pfx:prefix) (ins:instr) : bool := 
   match ins with 
+    (* valid_instr_grammars_rep *)
+    | MOVS w => rep_or_gs_or_op_prefix pfx
+    | STOS w => rep_or_gs_or_op_prefix pfx
+    (* valid_instr_grammars_rep_or_repn *)
+    | CMPS w => rep_or_repn_or_gs_or_op_prefix pfx
+    | SCAS w => rep_or_repn_or_gs_or_op_prefix pfx
+    (* valid_instr_grammars_lock_with_op_override *)
+    | ADD w op1 op2 => 
+      (* I'm not sure what to do here -- we use the lock_or_gs_with_op prefix
+         with the (ADD_p true) parser, and without for the (ADD_p false) parser.
+         The ADD_p true parser accepts halfword immediates and then 
+         sign extends them into a word, whereas the ADD_p false parser accepts a word,
+         so the information is lost as to whether we had a half-word or word.
+         So for now, I'm just going to assume that a prefix with or without
+         the operand is okay.   The situation is similar for other kinds
+         of operations such as ADC, AND, OR, SBB, SUB, and XOR. *)
+      no_imm_op op1 && (lock_or_gs_with_op pfx || lock_or_gs_without_op pfx)
+    | ADC w op1 op2 => 
+      no_imm_op op1 && (lock_or_gs_with_op pfx || lock_or_gs_without_op pfx)
+    | AND w op1 op2 => 
+      no_imm_op op1 && (lock_or_gs_with_op pfx || lock_or_gs_without_op pfx)
+    | NEG w op1 => 
+      no_imm_op op1 && (lock_or_gs_with_op pfx || lock_or_gs_without_op pfx)
+    | NOT w op1 => 
+      no_imm_op op1 && (lock_or_gs_with_op pfx || lock_or_gs_without_op pfx)
+    | OR w op1 op2 => 
+      no_imm_op op1 && (lock_or_gs_with_op pfx || lock_or_gs_without_op pfx)
+    | SBB w op1 op2 => 
+      no_imm_op op1 && (lock_or_gs_with_op pfx || lock_or_gs_without_op pfx)
+    | SUB w op1 op2 => 
+      no_imm_op op1 && (lock_or_gs_with_op pfx || lock_or_gs_without_op pfx)
+    | XOR w op1 op2 => 
+      no_imm_op op1 && (lock_or_gs_with_op pfx || lock_or_gs_without_op pfx)
+    | XCHG w op1 op2 => 
+      no_imm_op op1 && no_imm_op op2 && (lock_or_gs_with_op pfx || lock_or_gs_without_op pfx)
+    (* valid_instr_grammars_lock_no_op_override *)
+    (* covered by above: 
+    | ADD false op1 op2 => lock_or_gs_without_op pfx && no_imm_op op1
+    | ADC false op1 op2 => lock_or_gs_without_op pfx && no_imm_op op1
+    | AND false op1 op2 => lock_or_gs_without_op pfx && no_imm_op op1
+    *)
+    | BTC op1 op2 => lock_or_gs_without_op pfx && no_imm_op op1
+    | BTR op1 op2 => lock_or_gs_without_op pfx && no_imm_op op1
+    | BTS op1 op2 => lock_or_gs_without_op pfx && no_imm_op op1
+    | CMPXCHG w op1 op2 => lock_or_gs_without_op pfx && no_imm_op op1
+    | DEC w op1 => lock_or_gs_without_op pfx && no_imm_op op1
+    | INC w op1 => lock_or_gs_without_op pfx && no_imm_op op1
+    (* covered by above:                                         
+    | OR false op1 op2 => lock_or_gs_without_op pfx && no_imm_op op1
+    | SBB false op1 op2 => lock_or_gs_without_op pfx && no_imm_op op1
+    | SUB false op1 op2 => lock_or_gs_without_op pfx && no_imm_op op1
+    | XOR false op1 op2 => lock_or_gs_without_op pfx && no_imm_op op1
+    *)
+    | XADD w op1 op2 => lock_or_gs_without_op pfx && no_imm_op op1 && no_imm_op op2
+    (* valid_instr_grammars_only_seg_or_op_override *)
+    (* Similar issue with ADD above for CMP, IMUL, MOV, and TEST. *)
+    | CMP w op1 op2 => only_seg_or_op pfx 
+    | IMUL w op1 opopt iopt => only_seg_or_op pfx
+    | MOV w op1 op2 => only_seg_or_op pfx && no_imm_op op1
+    | TEST w op1 op2 => only_seg_or_op pfx
+    (* valid_instr_grammars_seg_op_override *) 
+    | CDQ => only_seg_or_op pfx 
+    | CMOVcc ct op1 op2 =>  only_seg_or_op pfx && no_imm_op op1
+    | CWDE => only_seg_or_op pfx
+    | DIV w op1 => only_seg_or_op pfx && no_imm_op op1
+    | IDIV w op1 => only_seg_or_op pfx && no_imm_op op1
+    | MOVSX w op1 op2 => only_seg_or_op pfx && no_imm_op op1
+    | MOVZX w op1 op2 => only_seg_or_op pfx && no_imm_op op1
+    | MUL w op1 => only_seg_or_op pfx && no_imm_op op1
+    | NOP op1 => only_seg_or_op pfx && no_imm_op op1
+    | ROL w op1 ri => only_seg_or_op pfx && no_imm_op op1
+    | ROR w op1 ri => only_seg_or_op pfx && no_imm_op op1
+    | SAR w op1 ri => only_seg_or_op pfx && no_imm_op op1
+    | SHL w op1 ri => only_seg_or_op pfx && no_imm_op op1
+    | SHLD op1 r ri => only_seg_or_op pfx && no_imm_op op1
+    | SHR w op1 ri => only_seg_or_op pfx && no_imm_op op1
+    | SHRD op1 op2 ri => only_seg_or_op pfx && no_imm_op op1
+    (* valid_instr_grammars_seg_override -- just gs segment override *)
     | AAA => only_gs_seg_override pfx
     | AAD => only_gs_seg_override pfx
     | AAM => only_gs_seg_override pfx
     | AAS => only_gs_seg_override pfx
-    | ADC w op1 op2 => either_prefix pfx && no_imm_op op1
-    | ADD w op1 op2 => either_prefix pfx && no_imm_op op1
-    | AND w op1 op2 => either_prefix pfx && no_imm_op op1
-    | CMP w op1 op2 => either_prefix pfx
-    | OR w op1 op2 => either_prefix pfx && no_imm_op op1
-    | SBB w op1 op2 => either_prefix pfx && no_imm_op op1
-    | SUB w op1 op2 => either_prefix pfx && no_imm_op op1
-    | XOR w op1 op2 => either_prefix pfx && no_imm_op op1
+    (* | CMP false op1 op2 => only_gs_seg_override pfx *)
+    | BOUND op1 op2 => only_gs_seg_override pfx && no_imm_op op1
     | BSF op1 op2 => only_gs_seg_override pfx && no_imm_op op1
-    | BSR op1 op2 => only_gs_seg_override pfx && no_imm_op op1 
+    | BSR op1 op2 => only_gs_seg_override pfx && no_imm_op op1
     | BSWAP r => only_gs_seg_override pfx
     | BT op1 op2 => only_gs_seg_override pfx && no_imm_op op1
-    | BTC op1 op2 => only_gs_seg_override pfx  && no_imm_op op1
-    | BTR op1 op2 => only_gs_seg_override pfx && no_imm_op op1
-    | BTS op1 op2 => only_gs_seg_override pfx  && no_imm_op op1
-    | CDQ => either_prefix pfx
-    | CLC => only_gs_seg_override pfx 
+    | CLC => only_gs_seg_override pfx
     | CLD => only_gs_seg_override pfx
-    | CMOVcc ct op1 op2 => only_gs_seg_override pfx && no_imm_op op1
-    | CMC => only_gs_seg_override pfx 
-    | CMPXCHG w op1 op2 => only_gs_seg_override pfx && no_imm_op op1
-    | CWDE => either_prefix pfx
+    | CLI => only_gs_seg_override pfx
+    | CLTS => only_gs_seg_override pfx
+    | CMC => only_gs_seg_override pfx
+    | CPUID => only_gs_seg_override pfx
     | DAA => only_gs_seg_override pfx
     | DAS => only_gs_seg_override pfx
-    | DEC w op1 => only_gs_seg_override pfx && no_imm_op op1
-    | DIV w op1 => either_prefix pfx && no_imm_op op1
     | HLT => only_gs_seg_override pfx
-    | IDIV w op1 => either_prefix pfx && no_imm_op op1
-    | IMUL w op1 opopt2 iopt3 => either_prefix pfx && no_imm_op op1
-    | INC w op1 => only_gs_seg_override pfx && no_imm_op op1
+    (* | IMUL false op1 opopt iopt => only_gs_seg_override pfx (* FIX? *) *)
     | LAHF => only_gs_seg_override pfx
+    | LAR op1 op2 => only_gs_seg_override pfx && no_imm_op op1
+    (* JGM:  The parser doesn't rule out other kinds of operands, so I'm
+       generalizing this to allow for it.  Note, however, that the machine
+       should trap if there isn't an address operand. 
     | LEA op1 (Address_op a) => only_gs_seg_override pfx && no_imm_op op1
+    *)
+    | LEA op1 op2 => only_gs_seg_override pfx && no_imm_op op1
     | LEAVE => only_gs_seg_override pfx
-    | MOV w op1 op2 => either_prefix pfx && no_imm_op op1
-    | MOVSX w op1 op2 => either_prefix pfx && no_imm_op op1
-    | MOVZX w op1 op2 => either_prefix pfx && no_imm_op op1
-    | MUL w op1 => either_prefix pfx && no_imm_op op1
-    | NEG w op1 => either_prefix pfx && no_imm_op op1
-    | NOT w op1 => either_prefix pfx && no_imm_op op1
+    | LGS op1 op2 => only_gs_seg_override pfx && no_imm_op op1
+    (* | MOV false op1 op2 => only_seg_or_op pfx && no_imm_op op1 *)
+    | MOVCR direction cr r => only_gs_seg_override pfx
+    | MOVDR direction dr r => only_gs_seg_override pfx
+    | MOVSR direction sr r => only_gs_seg_override pfx
+    | MOVBE op1 op2 => only_gs_seg_override pfx && no_imm_op op1
     | POP op1 => only_gs_seg_override pfx && no_imm_op op1
     | POPA => only_gs_seg_override pfx  
+    | POPF => only_gs_seg_override pfx  
     | PUSH w op1 => only_gs_seg_override pfx
     | PUSHA => only_gs_seg_override pfx 
+    | PUSHSR sr => only_gs_seg_override pfx  
+    | PUSHF => only_gs_seg_override pfx  
     | RCL w op1 ri => only_gs_seg_override pfx && no_imm_op op1
     | RCR w op1 ri => only_gs_seg_override pfx && no_imm_op op1
-    | ROL w op1 ri => only_gs_seg_override pfx && no_imm_op op1
-    | ROR w op1 ri => only_gs_seg_override pfx && no_imm_op op1
+    | RDMSR => only_gs_seg_override pfx  
+    | RDPMC => only_gs_seg_override pfx  
+    | RDTSC => only_gs_seg_override pfx  
+    | RDTSCP => only_gs_seg_override pfx  
+    | RSM => only_gs_seg_override pfx  
     | SAHF => only_gs_seg_override pfx
-    | SAR w op1 ri => either_prefix pfx && no_imm_op op1
     | SETcc ct op1 => only_gs_seg_override pfx && no_imm_op op1
-    | SHL w op1 ri => either_prefix pfx && no_imm_op op1
-    | SHLD op1 r ri => either_prefix pfx && no_imm_op op1
-    | SHR w op1 ri => either_prefix pfx && no_imm_op op1
-    | SHRD op1 r ri => either_prefix pfx && no_imm_op op1
+    | SGDT op1 => only_gs_seg_override pfx 
+    | SIDT op1 => only_gs_seg_override pfx 
+    | SLDT op1 => only_gs_seg_override pfx 
+    | SMSW op1 => only_gs_seg_override pfx 
     | STC => only_gs_seg_override pfx 
     | STD => only_gs_seg_override pfx 
-    | TEST w op1 op2 => either_prefix pfx
-    | XADD w op1 op2 => only_gs_seg_override pfx && no_imm_op op1 && no_imm_op op2
-    | XCHG w op1 op2 => either_prefix pfx && no_imm_op op1 && no_imm_op op2
-    | CMPS w => only_lock_or_rep pfx
-    | MOVS w => only_lock_or_rep pfx
-    | STOS w => only_lock_or_rep pfx
+    | STI => only_gs_seg_override pfx 
+    | STR op1 => only_gs_seg_override pfx 
+    (* | TEST false op1 op2 => only_gs_seg_override pfx *)
+    | WBINVD => only_gs_seg_override pfx 
+    | F2XM1 => only_gs_seg_override pfx 
+    | FABS => only_gs_seg_override pfx 
+    | FADD zerod op1 => only_gs_seg_override pfx 
+    | FADDP op1 => only_gs_seg_override pfx 
+    | FBLD op1 => only_gs_seg_override pfx 
+    | FBSTP op1 => only_gs_seg_override pfx 
+    | FCHS => only_gs_seg_override pfx 
+    | FCMOVcc ct op1 => only_gs_seg_override pfx 
+    | FCOM op1 => only_gs_seg_override pfx 
+    | FCOMP op1 => only_gs_seg_override pfx 
+    | FCOMPP => only_gs_seg_override pfx 
+    | FCOMIP op1 => only_gs_seg_override pfx 
+    | FCOS => only_gs_seg_override pfx 
+    | FDECSTP => only_gs_seg_override pfx 
+    | FDIV zerod op1 => only_gs_seg_override pfx 
+    | FDIVP op1 => only_gs_seg_override pfx 
+    | FDIVR zerod op1 => only_gs_seg_override pfx 
+    | FDIVRP op1 => only_gs_seg_override pfx 
+    | FFREE op1 => only_gs_seg_override pfx 
+    | FIADD op1 => only_gs_seg_override pfx 
+    | FICOM op1 => only_gs_seg_override pfx 
+    | FICOMP op1 => only_gs_seg_override pfx 
+    | FIDIV op1 => only_gs_seg_override pfx 
+    | FIDIVR op1 => only_gs_seg_override pfx 
+    | FILD op1 => only_gs_seg_override pfx 
+    | FIMUL op1 => only_gs_seg_override pfx 
+    | FINCSTP => only_gs_seg_override pfx 
+    | FIST op1 => only_gs_seg_override pfx 
+    | FISTP op1 => only_gs_seg_override pfx 
+    | FISUB op1 => only_gs_seg_override pfx 
+    | FISUBR op1 => only_gs_seg_override pfx 
+    | FLD op1 => only_gs_seg_override pfx 
+    | FLD1 => only_gs_seg_override pfx 
+    | FLDCW op1 => only_gs_seg_override pfx 
+    | FLDENV op1 => only_gs_seg_override pfx 
+    | FLDL2E => only_gs_seg_override pfx 
+    | FLDL2T => only_gs_seg_override pfx 
+    | FLDLG2 => only_gs_seg_override pfx 
+    | FLDLN2 => only_gs_seg_override pfx 
+    | FLDPI => only_gs_seg_override pfx 
+    | FLDZ => only_gs_seg_override pfx 
+    | FMUL zerod op1 => only_gs_seg_override pfx 
+    | FMULP op1 => only_gs_seg_override pfx
+    | FNCLEX => only_gs_seg_override pfx 
+    | FNINIT => only_gs_seg_override pfx 
+    | FNOP => only_gs_seg_override pfx 
+    | FNSAVE op1 => only_gs_seg_override pfx 
+    | FNSTCW op1 => only_gs_seg_override pfx 
+    | FNSTSW op1 => only_gs_seg_override pfx 
+    | FPATAN => only_gs_seg_override pfx 
+    | FPREM => only_gs_seg_override pfx 
+    | FPREM1 => only_gs_seg_override pfx 
+    | FPTAN => only_gs_seg_override pfx
+    | FRNDINT => only_gs_seg_override pfx 
+    | FRSTOR op1 => only_gs_seg_override pfx 
+    | FSCALE => only_gs_seg_override pfx 
+    | FSIN => only_gs_seg_override pfx 
+    | FSINCOS => only_gs_seg_override pfx 
+    | FSQRT => only_gs_seg_override pfx 
+    | FST op1 => only_gs_seg_override pfx 
+    | FSTENV op1 => only_gs_seg_override pfx 
+    | FSTP op1 => only_gs_seg_override pfx 
+    | FSUB zerod op1 => only_gs_seg_override pfx 
+    | FSUBP op1 => only_gs_seg_override pfx 
+    | FSUBR zerod op1 => only_gs_seg_override pfx 
+    | FSUBRP op1 => only_gs_seg_override pfx 
+    | FTST => only_gs_seg_override pfx 
+    | FUCOM op1 => only_gs_seg_override pfx 
+    | FUCOMP op1 => only_gs_seg_override pfx 
+    | FUCOMPP => only_gs_seg_override pfx 
+    | FUCOMI op1 => only_gs_seg_override pfx 
+    | FUCOMIP op1 => only_gs_seg_override pfx 
+    | FXAM => only_gs_seg_override pfx 
+    | FXCH op1 => only_gs_seg_override pfx 
+    | FXTRACT => only_gs_seg_override pfx 
+    | FYL2X => only_gs_seg_override pfx 
+    | FYL2XP1 => only_gs_seg_override pfx 
+    | FWAIT => only_gs_seg_override pfx 
+    | EMMS => only_gs_seg_override pfx 
+    | MOVD op1 op2 => only_gs_seg_override pfx && no_mmx_imm_op op1
+    | MOVQ op1 op2 => only_gs_seg_override pfx && no_mmx_imm_op op1
+    | PACKSSDW op1 op2 => only_gs_seg_override pfx && no_mmx_imm_op op1
+    | PACKSSWB op1 op2 => only_gs_seg_override pfx && no_mmx_imm_op op1
+    | PACKUSWB op1 op2 => only_gs_seg_override pfx && no_mmx_imm_op op1
+    | PADD gg op1 op2 => only_gs_seg_override pfx && no_mmx_imm_op op1
+    | PADDS gg op1 op2 => only_gs_seg_override pfx && no_mmx_imm_op op1
+    | PADDUS gg op1 op2 => only_gs_seg_override pfx && no_mmx_imm_op op1
+    | PAND op1 op2 => only_gs_seg_override pfx && no_mmx_imm_op op1
+    | PANDN op1 op2 => only_gs_seg_override pfx && no_mmx_imm_op op1
+    | PCMPEQ gg op1 op2 => only_gs_seg_override pfx && no_mmx_imm_op op1
+    | PCMPGT gg op1 op2 => only_gs_seg_override pfx && no_mmx_imm_op op1
+    | PMADDWD op1 op2 => only_gs_seg_override pfx && no_mmx_imm_op op1
+    | PMULHUW op1 op2 => only_gs_seg_override pfx && no_mmx_imm_op op1
+    | PMULHW op1 op2 => only_gs_seg_override pfx && no_mmx_imm_op op1
+    | PMULLW op1 op2 => only_gs_seg_override pfx && no_mmx_imm_op op1
+    | POR op1 op2 => only_gs_seg_override pfx && no_mmx_imm_op op1
+    | PSLL gg op1 op2 => only_gs_seg_override pfx && no_mmx_imm_op op1
+    | PSRA gg op1 op2 => only_gs_seg_override pfx && no_mmx_imm_op op1
+    | PSRL gg op1 op2 => only_gs_seg_override pfx && no_mmx_imm_op op1
+    | PSUB gg op1 op2 => only_gs_seg_override pfx && no_mmx_imm_op op1
+    | PSUBS gg op1 op2 => only_gs_seg_override pfx && no_mmx_imm_op op1
+    | PSUBUS gg op1 op2 => only_gs_seg_override pfx && no_mmx_imm_op op1
+    | PUNPCKH gg op1 op2 => only_gs_seg_override pfx && no_mmx_imm_op op1
+    | PUNPCKL gg op1 op2 => only_gs_seg_override pfx && no_mmx_imm_op op1
+    | PXOR op1 op2 => only_gs_seg_override pfx && no_mmx_imm_op op1
+    | ADDPS op1 op2 => only_gs_seg_override pfx && no_sse_imm_op op1
+    | ADDSS op1 op2 => only_gs_seg_override pfx && no_sse_imm_op op1
+    | ANDNPS op1 op2 => only_gs_seg_override pfx && no_sse_imm_op op1
+    | ANDPS op1 op2 => only_gs_seg_override pfx && no_sse_imm_op op1
+    | CMPPS op1 op2 imm => only_gs_seg_override pfx && no_sse_imm_op op1
+    | CMPSS op1 op2 imm => only_gs_seg_override pfx && no_sse_imm_op op1
+    | COMISS op1 op2 => only_gs_seg_override pfx && no_sse_imm_op op1
+    | CVTPI2PS op1 op2 => only_gs_seg_override pfx && no_sse_imm_op op1
+    | CVTPS2PI op1 op2 => only_gs_seg_override pfx && no_sse_imm_op op1
+    | CVTSI2SS op1 op2 => only_gs_seg_override pfx && no_sse_imm_op op1
+    | CVTSS2SI op1 op2 => only_gs_seg_override pfx && no_sse_imm_op op1
+    | CVTTPS2PI op1 op2 => only_gs_seg_override pfx && no_sse_imm_op op1
+    | CVTTSS2SI op1 op2 => only_gs_seg_override pfx && no_sse_imm_op op1
+    | DIVPS op1 op2 => only_gs_seg_override pfx && no_sse_imm_op op1
+    | DIVSS op1 op2 => only_gs_seg_override pfx && no_sse_imm_op op1
+    | LDMXCSR op1 => only_gs_seg_override pfx 
+    | MAXPS op1 op2 => only_gs_seg_override pfx && no_sse_imm_op op1
+    | MAXSS op1 op2 => only_gs_seg_override pfx && no_sse_imm_op op1
+    | MINPS op1 op2 => only_gs_seg_override pfx && no_sse_imm_op op1
+    | MINSS op1 op2 => only_gs_seg_override pfx && no_sse_imm_op op1
+    | MOVAPS op1 op2 => only_gs_seg_override pfx && no_sse_imm_op op1
+    | MOVHLPS op1 op2 => only_gs_seg_override pfx && no_sse_imm_op op1
+    | MOVLPS op1 op2 => only_gs_seg_override pfx && no_sse_imm_op op1
+    | MOVMSKPS op1 op2 => only_gs_seg_override pfx && no_sse_imm_op op1
+    | MOVSS op1 op2 => only_gs_seg_override pfx && no_sse_imm_op op1
+    | MOVUPS op1 op2 => only_gs_seg_override pfx && no_sse_imm_op op1
+    | MULPS op1 op2 => only_gs_seg_override pfx && no_sse_imm_op op1
+    | MULSS op1 op2 => only_gs_seg_override pfx && no_sse_imm_op op1
+    | ORPS op1 op2 => only_gs_seg_override pfx && no_sse_imm_op op1
+    | RCPPS op1 op2 => only_gs_seg_override pfx && no_sse_imm_op op1
+    | RCPSS op1 op2 => only_gs_seg_override pfx && no_sse_imm_op op1
+    | RSQRTPS op1 op2 => only_gs_seg_override pfx && no_sse_imm_op op1
+    | RSQRTSS op1 op2 => only_gs_seg_override pfx && no_sse_imm_op op1
+    | SHUFPS op1 op2 imm => only_gs_seg_override pfx && no_sse_imm_op op1
+    | SQRTPS op1 op2 => only_gs_seg_override pfx && no_sse_imm_op op1
+    | SQRTSS op1 op2 => only_gs_seg_override pfx && no_sse_imm_op op1
+    | STMXCSR op1 => only_gs_seg_override pfx
+    | SUBPS op1 op2 => only_gs_seg_override pfx && no_sse_imm_op op1
+    | SUBSS op1 op2 => only_gs_seg_override pfx && no_sse_imm_op op1
+    | UCOMISS op1 op2 => only_gs_seg_override pfx && no_sse_imm_op op1
+    | UNPCKHPS op1 op2 => only_gs_seg_override pfx && no_sse_imm_op op1
+    | UNPCKLPS op1 op2 => only_gs_seg_override pfx && no_sse_imm_op op1
+    | XORPS op1 op2 => only_gs_seg_override pfx && no_sse_imm_op op1
+    | PAVGB op1 op2 => only_gs_seg_override pfx && no_sse_imm_op op1
+    | PEXTRW op1 op2 imm => only_gs_seg_override pfx && no_sse_imm_op op1
+    | PINSRW op1 op2 imm => only_gs_seg_override pfx && no_sse_imm_op op1
+    | PMAXSW op1 op2 => only_gs_seg_override pfx && no_sse_imm_op op1
+    | PMAXUB op1 op2 => only_gs_seg_override pfx && no_sse_imm_op op1
+    | PMINSW op1 op2 => only_gs_seg_override pfx && no_sse_imm_op op1
+    | PMINUB op1 op2 => only_gs_seg_override pfx && no_sse_imm_op op1
+    | PMOVMSKB op1 op2 => only_gs_seg_override pfx && no_sse_imm_op op1
+    | PSADBW op1 op2 => only_gs_seg_override pfx && no_sse_imm_op op1
+    | PSHUFW op1 op2 imm => only_gs_seg_override pfx && no_sse_imm_op op1
+    | MASKMOVQ op1 op2 => only_gs_seg_override pfx && no_sse_imm_op op1
+    | MOVNTPS op1 op2 => only_gs_seg_override pfx && no_sse_imm_op op1
+    | MOVNTQ op1 op2 => only_gs_seg_override pfx && no_sse_imm_op op1
+    | PREFETCHT0 op1 => only_gs_seg_override pfx 
+    | PREFETCHT1 op1 => only_gs_seg_override pfx 
+    | PREFETCHT2 op1 => only_gs_seg_override pfx 
+    | PREFETCHNTA op1 => only_gs_seg_override pfx 
+    | SFENCE => only_gs_seg_override pfx 
     | _ => false
   end.
-
 
 (** We rule out JMPs and CALLs that are far (i.e., not near), that
     are absolute instead of relative, that don't have an immediate
@@ -342,8 +742,10 @@ Definition nacljmp_mask_instr (pfx1:prefix) (ins1:instr) (pfx2:prefix) (ins2:ins
     | _ => false
   end.
 
+Definition make_recognizer t (g:grammar t) := 
+  Recognizer.build_dfa 400 (par2rec g).
 
-(* Definition dfas := (make_dfa non_cflow_grammar, make_dfa (alts dir_cflow), make_dfa (alts nacljmp_mask)). *)
+Definition dfas := (make_recognizer non_cflow_grammar, make_recognizer (alts dir_cflow), make_recognizer (alts nacljmp_mask)).
 (* Extraction "tables.ml" dfas.*)
 
 
